<?xml version="1.0"?>
<rdf:RDF xmlns="http://humanbehaviourchange.org/ontology/bcto.owl#"
     xml:base="http://humanbehaviourchange.org/ontology/bcto.owl"
     xmlns:dc="http://purl.org/dc/elements/1.1/"
     xmlns:obo="http://purl.obolibrary.org/obo/"
     xmlns:owl="http://www.w3.org/2002/07/owl#"
     xmlns:rdf="http://www.w3.org/1999/02/22-rdf-syntax-ns#"
     xmlns:xml="http://www.w3.org/XML/1998/namespace"
     xmlns:xsd="http://www.w3.org/2001/XMLSchema#"
     xmlns:foaf="http://xmlns.com/foaf/0.1/"
     xmlns:rdfs="http://www.w3.org/2000/01/rdf-schema#"
     xmlns:sssom="https://w3id.org/sssom/"
     xmlns:terms="http://purl.org/dc/terms/"
     xmlns:schema="https://schema.org/"
     xmlns:Property="https://www.wikidata.org/wiki/Property:"
     xmlns:oboInOwl="http://www.geneontology.org/formats/oboInOwl#"
     xmlns:owlready_ontology="http://www.lesfleursdunormal.fr/static/_downloads/owlready_ontology.owl#">
    <owl:Ontology rdf:about="http://humanbehaviourchange.org/ontology/bcto.owl">
        <owl:imports rdf:resource="http://humanbehaviourchange.org/ontology/bcio_external.owl"/>
        <owl:imports rdf:resource="http://humanbehaviourchange.org/ontology/bcio_upper_level.owl"/>
    </owl:Ontology>
    


    <!-- 
    ///////////////////////////////////////////////////////////////////////////////////////
    //
    // Classes
    //
    ///////////////////////////////////////////////////////////////////////////////////////
     -->

    


    <!-- http://humanbehaviourchange.org/ontology/BCIO_007001 -->

    <owl:Class rdf:about="http://humanbehaviourchange.org/ontology/BCIO_007001">
        <rdfs:subClassOf rdf:resource="http://humanbehaviourchange.org/ontology/BCIO_033000"/>
        <obo:IAO_0000114>Published</obo:IAO_0000114>
        <obo:IAO_0000115>A behaviour change technique that sets or changes goals.</obo:IAO_0000115>
        <rdfs:comment>A goal is a cognitive representation of an end state towards which one is striving.</rdfs:comment>
        <rdfs:label>goal directed BCT</rdfs:label>
    </owl:Class>
    


    <!-- http://humanbehaviourchange.org/ontology/BCIO_007002 -->

    <owl:Class rdf:about="http://humanbehaviourchange.org/ontology/BCIO_007002">
        <rdfs:subClassOf rdf:resource="http://humanbehaviourchange.org/ontology/BCIO_007001"/>
        <obo:IAO_0000114>Published</obo:IAO_0000114>
        <obo:IAO_0000115>A goal directed BCT that sets goals.</obo:IAO_0000115>
        <rdfs:comment>A goal is a cognitive representation of an end state towards which one is striving. The goal could be set for the self or another person.</rdfs:comment>
        <rdfs:label>goal setting BCT</rdfs:label>
    </owl:Class>
    


    <!-- http://humanbehaviourchange.org/ontology/BCIO_007003 -->

    <owl:Class rdf:about="http://humanbehaviourchange.org/ontology/BCIO_007003">
        <rdfs:subClassOf rdf:resource="http://humanbehaviourchange.org/ontology/BCIO_007002"/>
        <obo:IAO_0000114>Published</obo:IAO_0000114>
        <obo:IAO_0000115>A goal setting BCT that sets a goal for the behaviour to be achieved.</obo:IAO_0000115>
        <rdfs:comment> if goal is a behavioural outcome, code &apos;set outcome goal BCT&apos;</rdfs:comment>
        <rdfs:comment> if goal unspecified code &apos;goal setting BCT&apos;</rdfs:comment>
        <rdfs:comment> if the goal defines a specific context, frequency, duration or intensity for the behaviour, also code &apos;action planning BCT&apos;.</rdfs:comment>
        <rdfs:comment>A goal is a cognitive representation of an end state towards which one is striving. The goal could be set for the self or another person. Only code if there is sufficient evidence that the goal is set as part of intervention</rdfs:comment>
        <rdfs:label>set behaviour goal BCT</rdfs:label>
    </owl:Class>
    


    <!-- http://humanbehaviourchange.org/ontology/BCIO_007004 -->

    <owl:Class rdf:about="http://humanbehaviourchange.org/ontology/BCIO_007004">
        <rdfs:subClassOf rdf:resource="http://humanbehaviourchange.org/ontology/BCIO_007002"/>
        <obo:IAO_0000114>Published</obo:IAO_0000114>
        <obo:IAO_0000115>A goal setting BCT that involves the intervention source agreeing with the person on a behavioural goal.</obo:IAO_0000115>
        <rdfs:comment>A goal is a cognitive representation of an end state towards which one is striving.</rdfs:comment>
        <rdfs:label>agree behaviour goal BCT</rdfs:label>
    </owl:Class>
    


    <!-- http://humanbehaviourchange.org/ontology/BCIO_007005 -->

    <owl:Class rdf:about="http://humanbehaviourchange.org/ontology/BCIO_007005">
        <rdfs:subClassOf rdf:resource="http://humanbehaviourchange.org/ontology/BCIO_007002"/>
        <obo:IAO_0000114>Published</obo:IAO_0000114>
        <obo:IAO_0000115>A goal setting BCT in which the goal is a positive outcome of performing the behaviour.</obo:IAO_0000115>
        <rdfs:comment> if goal is a behaviour, code &apos;set behaviour goal BCT&apos;</rdfs:comment>
        <rdfs:comment> if goal unspecified code &apos;goal setting BCT&apos;.</rdfs:comment>
        <rdfs:comment>A goal is a cognitive representation of an end state towards which one is striving. The goal could be set for the self or another person. Only code guidelines if set as a goal in an intervention context</rdfs:comment>
        <rdfs:label>set outcome goal BCT</rdfs:label>
    </owl:Class>
    


    <!-- http://humanbehaviourchange.org/ontology/BCIO_007006 -->

    <owl:Class rdf:about="http://humanbehaviourchange.org/ontology/BCIO_007006">
        <rdfs:subClassOf rdf:resource="http://humanbehaviourchange.org/ontology/BCIO_007002"/>
        <obo:IAO_0000114>Published</obo:IAO_0000114>
        <obo:IAO_0000115>A goal setting BCT that involves the intervention source agreeing with the person on a goal which is a positive outcome of performing the behaviour.</obo:IAO_0000115>
        <obo:IAO_0000118>objective setting</obo:IAO_0000118>
        <rdfs:comment>A goal is a cognitive representation of an end state towards which one is striving.</rdfs:comment>
        <rdfs:label>agree outcome goal BCT</rdfs:label>
    </owl:Class>
    


    <!-- http://humanbehaviourchange.org/ontology/BCIO_007008 -->

    <owl:Class rdf:about="http://humanbehaviourchange.org/ontology/BCIO_007008">
        <rdfs:subClassOf rdf:resource="http://humanbehaviourchange.org/ontology/BCIO_007001"/>
        <obo:IAO_0000114>Published</obo:IAO_0000114>
        <obo:IAO_0000115>A goal directed BCT in which the person analyses factors influencing the behaviour and generates, selects, or reviews strategies to increase facilitators and overcome barriers.</obo:IAO_0000115>
        <obo:IAO_0000118>relapse prevention, coping planning, problem solving</obo:IAO_0000118>
        <rdfs:comment>Barrier identification without strategies to increase facilitators is not sufficient.</rdfs:comment>
        <rdfs:label>goal strategising BCT</rdfs:label>
    </owl:Class>
    


    <!-- http://humanbehaviourchange.org/ontology/BCIO_007010 -->

    <owl:Class rdf:about="http://humanbehaviourchange.org/ontology/BCIO_007010">
        <rdfs:subClassOf rdf:resource="http://humanbehaviourchange.org/ontology/BCIO_007001"/>
        <obo:IAO_0000114>Published</obo:IAO_0000114>
        <obo:IAO_0000115>A goal directed BCT that involves making a detailed plan for the performance of the behaviour, which must include at least one of context, frequency, duration or intensity.</obo:IAO_0000115>
        <rdfs:comment>Evidence of action planning does not necessarily imply goal setting, only code latter if sufficient evidence.</rdfs:comment>
        <rdfs:label>action planning BCT</rdfs:label>
    </owl:Class>
    


    <!-- http://humanbehaviourchange.org/ontology/BCIO_007011 -->

    <owl:Class rdf:about="http://humanbehaviourchange.org/ontology/BCIO_007011">
        <rdfs:subClassOf rdf:resource="http://humanbehaviourchange.org/ontology/BCIO_007001"/>
        <obo:IAO_0000114>Published</obo:IAO_0000114>
        <obo:IAO_0000115>A goal directed BCT that reviews a behavioural goal and considers modifying the goal in light of progress toward the goal.</obo:IAO_0000115>
        <rdfs:comment> if discrepancy created consider also &apos;attend to discrepancy between current behaviour and goal BCT&apos;</rdfs:comment>
        <rdfs:comment> if goal unspecified, code &apos;review outcome goal BCT&apos;</rdfs:comment>
        <rdfs:comment> if modifying the plan to achieve the goal consider also &apos;review behaviour goal plan BCT&apos;.</rdfs:comment>
        <rdfs:comment>A goal is a cognitive representation of an end state towards which one is striving. If goal specified in terms of behaviour, code this class</rdfs:comment>
        <rdfs:label>review behaviour goal BCT</rdfs:label>
    </owl:Class>
    


    <!-- http://humanbehaviourchange.org/ontology/BCIO_007012 -->

    <owl:Class rdf:about="http://humanbehaviourchange.org/ontology/BCIO_007012">
        <rdfs:subClassOf rdf:resource="http://humanbehaviourchange.org/ontology/BCIO_007001"/>
        <obo:IAO_0000114>Published</obo:IAO_0000114>
        <obo:IAO_0000115>A goal directed BCT that draws attention to discrepancies between a person&apos;s current behaviour and the person&apos;s outcome goal, behavioural goal or action plan.</obo:IAO_0000115>
        <rdfs:comment> if feedback provided, also code &apos;provide feedback BCT&apos; or one of its child classes.</rdfs:comment>
        <rdfs:comment>If discomfort is created only code &apos;draw attention to incompatible beliefs BCT&apos; and not this class. If goals are modified, also code &apos;review behaviour goal BCT&apos; and/or &apos;review outcome goal BCT&apos;</rdfs:comment>
        <rdfs:label>attend to discrepancy between current behaviour and goal BCT</rdfs:label>
    </owl:Class>
    


    <!-- http://humanbehaviourchange.org/ontology/BCIO_007013 -->

    <owl:Class rdf:about="http://humanbehaviourchange.org/ontology/BCIO_007013">
        <rdfs:subClassOf rdf:resource="http://humanbehaviourchange.org/ontology/BCIO_007001"/>
        <obo:IAO_0000114>Published</obo:IAO_0000114>
        <obo:IAO_0000115>A goal directed BCT that reviews an outcome goal and considers modifying the goal in light of achievement.</obo:IAO_0000115>
        <rdfs:comment> if discrepancy created consider also &apos;attend to discrepancy between current behaviour and goal BCT&apos;.</rdfs:comment>
        <rdfs:comment> if goal unspecified, code this class</rdfs:comment>
        <rdfs:comment>A goal is a cognitive representation of an end state towards which one is striving. If goal specified in terms of behaviour, code &apos;review behaviour goal BCT&apos;</rdfs:comment>
        <rdfs:label>review outcome goal BCT</rdfs:label>
    </owl:Class>
    


    <!-- http://humanbehaviourchange.org/ontology/BCIO_007014 -->

    <owl:Class rdf:about="http://humanbehaviourchange.org/ontology/BCIO_007014">
        <rdfs:subClassOf rdf:resource="http://humanbehaviourchange.org/ontology/BCIO_007001"/>
        <obo:IAO_0000114>Published</obo:IAO_0000114>
        <obo:IAO_0000115>A goal directed BCT that creates a written specification of the behaviour to be performed, agreed on by the person, and witnessed by another person.</obo:IAO_0000115>
        <obo:IAO_0000118>behavioural contract</obo:IAO_0000118>
        <rdfs:comment>The person witnessing the agreement can be the intervention source or another person who is present at the time. Also code &apos;set behaviour goal BCT&apos;.</rdfs:comment>
        <rdfs:label>create behavioural contract BCT</rdfs:label>
    </owl:Class>
    


    <!-- http://humanbehaviourchange.org/ontology/BCIO_007015 -->

    <owl:Class rdf:about="http://humanbehaviourchange.org/ontology/BCIO_007015">
        <rdfs:subClassOf rdf:resource="http://humanbehaviourchange.org/ontology/BCIO_007001"/>
        <obo:IAO_0000114>Published</obo:IAO_0000114>
        <obo:IAO_0000115>A goal directed BCT that asks the person to affirm or reaffirm statements indicating commitment to change the behaviour.</obo:IAO_0000115>
        <obo:IAO_0000118>commitment</obo:IAO_0000118>
        <rdfs:comment>If defined in terms of the behaviour to be achieved also code &apos;set behaviour goal BCT&apos;.</rdfs:comment>
        <rdfs:label>affirm commitment BCT</rdfs:label>
    </owl:Class>
    


    <!-- http://humanbehaviourchange.org/ontology/BCIO_007016 -->

    <owl:Class rdf:about="http://humanbehaviourchange.org/ontology/BCIO_007016">
        <rdfs:subClassOf rdf:resource="http://humanbehaviourchange.org/ontology/BCIO_007001"/>
        <obo:IAO_0000114>Published</obo:IAO_0000114>
        <obo:IAO_0000115>A goal directed BCT that advises the person to adopt more than one goal in a situation where the goals facilitate each other.</obo:IAO_0000115>
        <obo:IAO_0000118>goal facilitation</obo:IAO_0000118>
        <rdfs:label>advise goal integration BCT</rdfs:label>
    </owl:Class>
    


    <!-- http://humanbehaviourchange.org/ontology/BCIO_007017 -->

    <owl:Class rdf:about="http://humanbehaviourchange.org/ontology/BCIO_007017">
        <rdfs:subClassOf rdf:resource="http://humanbehaviourchange.org/ontology/BCIO_033000"/>
        <obo:IAO_0000114>Published</obo:IAO_0000114>
        <obo:IAO_0000115>A behaviour change technique that involves gathering or using information about performance.</obo:IAO_0000115>
        <rdfs:label>monitoring BCT</rdfs:label>
    </owl:Class>
    


    <!-- http://humanbehaviourchange.org/ontology/BCIO_007018 -->

    <owl:Class rdf:about="http://humanbehaviourchange.org/ontology/BCIO_007018">
        <rdfs:subClassOf rdf:resource="http://humanbehaviourchange.org/ontology/BCIO_007017"/>
        <obo:IAO_0000114>Published</obo:IAO_0000114>
        <obo:IAO_0000115>A monitoring BCT that observes current performance of the behaviour with the person’s knowledge but without providing feedback about their behaviour.</obo:IAO_0000115>
        <obo:IAO_0000118>observation, performance monitoring</obo:IAO_0000118>
        <rdfs:comment> if feedback given, code only &apos;provide feedback on behaviour BCT&apos; and not this class</rdfs:comment>
        <rdfs:comment> if observing outcomes code &apos;observe outcome of behaviour without feedback BCT&apos;.</rdfs:comment>
        <rdfs:comment>The monitoring agent can be a human or a technical device. If observation is part of a data collection procedure rather than a strategy aimed at changing behaviour, do not code</rdfs:comment>
        <rdfs:label>observe behaviour without feedback BCT</rdfs:label>
    </owl:Class>
    


    <!-- http://humanbehaviourchange.org/ontology/BCIO_007019 -->

    <owl:Class rdf:about="http://humanbehaviourchange.org/ontology/BCIO_007019">
        <rdfs:subClassOf rdf:resource="http://humanbehaviourchange.org/ontology/BCIO_007017"/>
        <obo:IAO_0000114>Published</obo:IAO_0000114>
        <obo:IAO_0000115>A monitoring BCT that records current performance of the behaviour with the person’s knowledge but without providing feedback about their behaviour.</obo:IAO_0000115>
        <obo:IAO_0000118>monitoring</obo:IAO_0000118>
        <rdfs:comment> if feedback given, code only &apos;provide feedback on behaviour BCT&apos; and not this class</rdfs:comment>
        <rdfs:comment> if recording outcomes code &apos;record outcome of behaviour without feedback BCT&apos;.</rdfs:comment>
        <rdfs:comment>The monitoring agent can be a human or a technical device. If recording is part of a data collection procedure rather than a strategy aimed at changing behaviour, do not code</rdfs:comment>
        <rdfs:label>record behaviour without feedback BCT</rdfs:label>
    </owl:Class>
    


    <!-- http://humanbehaviourchange.org/ontology/BCIO_007020 -->

    <owl:Class rdf:about="http://humanbehaviourchange.org/ontology/BCIO_007020">
        <rdfs:subClassOf rdf:resource="http://humanbehaviourchange.org/ontology/BCIO_007017"/>
        <obo:IAO_0000114>Published</obo:IAO_0000114>
        <obo:IAO_0000115>A monitoring BCT that observes an outcome of performing the behaviour with the person’s knowledge but without providing feedback about the outcome.</obo:IAO_0000115>
        <rdfs:comment> if feedback given, code only &apos;provide feedback on outcome of behaviour BCT&apos; and not this class</rdfs:comment>
        <rdfs:comment> if observing behaviour code &apos;observe behaviour without feedback BCT&apos;.</rdfs:comment>
        <rdfs:comment>The monitoring agent can be a human or a technical device. If recording is part of a data collection procedure rather than a strategy aimed at changing behaviour, do not code</rdfs:comment>
        <rdfs:label>observe outcome of behaviour without feedback BCT</rdfs:label>
    </owl:Class>
    


    <!-- http://humanbehaviourchange.org/ontology/BCIO_007021 -->

    <owl:Class rdf:about="http://humanbehaviourchange.org/ontology/BCIO_007021">
        <rdfs:subClassOf rdf:resource="http://humanbehaviourchange.org/ontology/BCIO_007017"/>
        <obo:IAO_0000114>Published</obo:IAO_0000114>
        <obo:IAO_0000115>A monitoring BCT that records an outcome of performing the behaviour with the person&apos;s knowledge but without providing feedback about the outcome.</obo:IAO_0000115>
        <rdfs:comment> if feedback given, code only &apos;provide feedback on outcome of behaviour BCT&apos; and not this class</rdfs:comment>
        <rdfs:comment> if recording behaviour code &apos;record behaviour without feedback BCT&apos;.</rdfs:comment>
        <rdfs:comment>The monitoring agent can be a human or a technical device. If recording is part of a data collection procedure rather than a strategy aimed at changing behaviour, do not code</rdfs:comment>
        <rdfs:label>record outcome of behaviour without feedback BCT</rdfs:label>
    </owl:Class>
    


    <!-- http://humanbehaviourchange.org/ontology/BCIO_007022 -->

    <owl:Class rdf:about="http://humanbehaviourchange.org/ontology/BCIO_007022">
        <rdfs:subClassOf rdf:resource="http://humanbehaviourchange.org/ontology/BCIO_007017"/>
        <obo:IAO_0000114>Published</obo:IAO_0000114>
        <obo:IAO_0000115>A monitoring BCT in which feedback about the behaviour is provided.</obo:IAO_0000115>
        <obo:IAO_0000118>feedback, behavioural feedback</obo:IAO_0000118>
        <rdfs:comment>Feedback is provision of data about some aspect of behaviour without an evaluation (positive or negative). Where feedback includes reward or punishment, see behavioural consequence BCT, outcome consequence BCT and their child classes. If there is no clear evidence that feedback was given, code &apos;observe behaviour without feedback BCT&apos; or &apos;record behaviour without feedback BCT&apos;.</rdfs:comment>
        <rdfs:label>provide feedback BCT</rdfs:label>
    </owl:Class>
    


    <!-- http://humanbehaviourchange.org/ontology/BCIO_007023 -->

    <owl:Class rdf:about="http://humanbehaviourchange.org/ontology/BCIO_007023">
        <rdfs:subClassOf rdf:resource="http://humanbehaviourchange.org/ontology/BCIO_007022"/>
        <obo:IAO_0000114>Published</obo:IAO_0000114>
        <obo:IAO_0000115>A provide feedback BCT that provides information about the person&apos;s previous performance of the behaviour.</obo:IAO_0000115>
        <rdfs:label>provide feedback on behaviour BCT</rdfs:label>
    </owl:Class>
    


    <!-- http://humanbehaviourchange.org/ontology/BCIO_007024 -->

    <owl:Class rdf:about="http://humanbehaviourchange.org/ontology/BCIO_007024">
        <rdfs:subClassOf rdf:resource="http://humanbehaviourchange.org/ontology/BCIO_007017"/>
        <obo:IAO_0000114>Published</obo:IAO_0000114>
        <obo:IAO_0000115>A monitoring BCT in which the person uses a method to monitor and record their behaviour.</obo:IAO_0000115>
        <obo:IAO_0000118>self-monitoring</obo:IAO_0000118>
        <rdfs:comment> if self-monitoring of outcome of behaviour, code &apos;self-monitor outcome of behaviour BCT&apos;.</rdfs:comment>
        <rdfs:comment>If monitoring is part of a data collection procedure rather than a strategy aimed at changing behaviour, do not code</rdfs:comment>
        <rdfs:label>self-monitor behaviour BCT</rdfs:label>
    </owl:Class>
    


    <!-- http://humanbehaviourchange.org/ontology/BCIO_007025 -->

    <owl:Class rdf:about="http://humanbehaviourchange.org/ontology/BCIO_007025">
        <rdfs:subClassOf rdf:resource="http://humanbehaviourchange.org/ontology/BCIO_007017"/>
        <obo:IAO_0000114>Published</obo:IAO_0000114>
        <obo:IAO_0000115>A monitoring BCT in which the person uses a method to monitor and record an outcome of their behaviour.</obo:IAO_0000115>
        <rdfs:comment> if self-monitoring behaviour, code &apos;self-monitor behaviour BCT&apos;.</rdfs:comment>
        <rdfs:comment>If monitoring is part of a data collection procedure rather than a strategy aimed at changing behaviour, do not code</rdfs:comment>
        <rdfs:label>self-monitor outcome of behaviour BCT</rdfs:label>
    </owl:Class>
    


    <!-- http://humanbehaviourchange.org/ontology/BCIO_007026 -->

    <owl:Class rdf:about="http://humanbehaviourchange.org/ontology/BCIO_007026">
        <rdfs:subClassOf rdf:resource="http://humanbehaviourchange.org/ontology/BCIO_007022"/>
        <obo:IAO_0000112>Using a pedometer to keep track of number of steps taken in a day.</obo:IAO_0000112>
        <obo:IAO_0000114>Published</obo:IAO_0000114>
        <obo:IAO_0000115>A provide feedback BCT that provides information about the functioning or state of the person&apos;s body, based on information collected by an external monitoring device.</obo:IAO_0000115>
        <obo:IAO_0000118>biofeedback</obo:IAO_0000118>
        <rdfs:label>provide biofeedback BCT</rdfs:label>
    </owl:Class>
    


    <!-- http://humanbehaviourchange.org/ontology/BCIO_007027 -->

    <owl:Class rdf:about="http://humanbehaviourchange.org/ontology/BCIO_007027">
        <rdfs:subClassOf rdf:resource="http://humanbehaviourchange.org/ontology/BCIO_007022"/>
        <obo:IAO_0000114>Published</obo:IAO_0000114>
        <obo:IAO_0000115>A provide feedback BCT that provides information about an outcome of the person&apos;s previous performance of the behaviour.</obo:IAO_0000115>
        <rdfs:label>provide feedback on outcome of behaviour BCT</rdfs:label>
    </owl:Class>
    


    <!-- http://humanbehaviourchange.org/ontology/BCIO_007028 -->

    <owl:Class rdf:about="http://humanbehaviourchange.org/ontology/BCIO_007028">
        <rdfs:subClassOf rdf:resource="http://humanbehaviourchange.org/ontology/BCIO_033000"/>
        <obo:IAO_0000114>Published</obo:IAO_0000114>
        <obo:IAO_0000115>A behaviour change technique that involves taking steps to secure or deliver the support or aid of another person.</obo:IAO_0000115>
        <rdfs:comment>Attending a group class and/or mention of ‘follow-up’ does not necessarily apply this BCT, support must be explicitly mentioned.</rdfs:comment>
        <rdfs:label>social support BCT</rdfs:label>
    </owl:Class>
    


    <!-- http://humanbehaviourchange.org/ontology/BCIO_007029 -->

    <owl:Class rdf:about="http://humanbehaviourchange.org/ontology/BCIO_007029">
        <rdfs:subClassOf rdf:resource="http://humanbehaviourchange.org/ontology/BCIO_007028"/>
        <obo:IAO_0000114>Published</obo:IAO_0000114>
        <obo:IAO_0000115>A social support BCT that involves advising the person to seek support from another person.</obo:IAO_0000115>
        <rdfs:comment>Where an &quot;advise to seek support BCT&quot; is used together with an &quot;arrange support BCT,&quot; this constitutes connecting to social support as used in social prescribing. Attending a group class and/or mention of ‘follow-up’ does not necessarily apply this BCT, support must be explicitly mentioned</rdfs:comment>
        <rdfs:label>advise to seek support BCT</rdfs:label>
    </owl:Class>
    


    <!-- http://humanbehaviourchange.org/ontology/BCIO_007030 -->

    <owl:Class rdf:about="http://humanbehaviourchange.org/ontology/BCIO_007030">
        <rdfs:subClassOf rdf:resource="http://humanbehaviourchange.org/ontology/BCIO_007029"/>
        <obo:IAO_0000114>Published</obo:IAO_0000114>
        <obo:IAO_0000115>An advise to seek support BCT that suggests the person try to obtain support from another in terms of tangible aid.</obo:IAO_0000115>
        <rdfs:label>advise to seek instrumental support BCT</rdfs:label>
    </owl:Class>
    


    <!-- http://humanbehaviourchange.org/ontology/BCIO_007031 -->

    <owl:Class rdf:about="http://humanbehaviourchange.org/ontology/BCIO_007031">
        <rdfs:subClassOf rdf:resource="http://humanbehaviourchange.org/ontology/BCIO_007029"/>
        <obo:IAO_0000114>Published</obo:IAO_0000114>
        <obo:IAO_0000115>An advise to seek support BCT that suggests the person try to obtain support from another in terms of expressing concern, caring and empathy.</obo:IAO_0000115>
        <rdfs:label>advise to seek emotional support BCT</rdfs:label>
    </owl:Class>
    


    <!-- http://humanbehaviourchange.org/ontology/BCIO_007032 -->

    <owl:Class rdf:about="http://humanbehaviourchange.org/ontology/BCIO_007032">
        <rdfs:subClassOf rdf:resource="http://humanbehaviourchange.org/ontology/BCIO_007029"/>
        <obo:IAO_0000114>Published</obo:IAO_0000114>
        <obo:IAO_0000115>An advise to seek support BCT that suggests the person try to obtain support from another in terms of advice, suggestions and information.</obo:IAO_0000115>
        <rdfs:label>advise to seek informational support BCT</rdfs:label>
    </owl:Class>
    


    <!-- http://humanbehaviourchange.org/ontology/BCIO_007033 -->

    <owl:Class rdf:about="http://humanbehaviourchange.org/ontology/BCIO_007033">
        <rdfs:subClassOf rdf:resource="http://humanbehaviourchange.org/ontology/BCIO_007029"/>
        <obo:IAO_0000114>Published</obo:IAO_0000114>
        <obo:IAO_0000115>An advise to seek support BCT that suggests the person try to obtain support from another in terms of information that will aid the person in evaluating themself or the situation.</obo:IAO_0000115>
        <rdfs:label>advise to seek appraisal support BCT</rdfs:label>
    </owl:Class>
    


    <!-- http://humanbehaviourchange.org/ontology/BCIO_007034 -->

    <owl:Class rdf:about="http://humanbehaviourchange.org/ontology/BCIO_007034">
        <rdfs:subClassOf rdf:resource="http://humanbehaviourchange.org/ontology/BCIO_007028"/>
        <obo:IAO_0000114>Published</obo:IAO_0000114>
        <obo:IAO_0000115>A social support BCT that organises support from another for the person.</obo:IAO_0000115>
        <rdfs:comment>Where an &quot;arrange support BCT&quot; is used together with an &quot;advise to seek support BCT&quot;, this constitutes &quot;connecting to support&quot; as used in social prescribing. Attending a group class and/or mention of ‘follow-up’ does not necessarily apply this BCT, support must be explicitly mentioned</rdfs:comment>
        <rdfs:label>arrange support BCT</rdfs:label>
    </owl:Class>
    


    <!-- http://humanbehaviourchange.org/ontology/BCIO_007035 -->

    <owl:Class rdf:about="http://humanbehaviourchange.org/ontology/BCIO_007035">
        <rdfs:subClassOf rdf:resource="http://humanbehaviourchange.org/ontology/BCIO_007034"/>
        <obo:IAO_0000114>Published</obo:IAO_0000114>
        <obo:IAO_0000115>An arrange support BCT that organises support from another in terms of tangible aid.</obo:IAO_0000115>
        <rdfs:label>arrange instrumental support BCT</rdfs:label>
    </owl:Class>
    


    <!-- http://humanbehaviourchange.org/ontology/BCIO_007036 -->

    <owl:Class rdf:about="http://humanbehaviourchange.org/ontology/BCIO_007036">
        <rdfs:subClassOf rdf:resource="http://humanbehaviourchange.org/ontology/BCIO_007034"/>
        <obo:IAO_0000114>Published</obo:IAO_0000114>
        <obo:IAO_0000115>An arrange support BCT that organises support from another in terms of expressing concern, caring and empathy.</obo:IAO_0000115>
        <rdfs:label>arrange emotional support BCT</rdfs:label>
    </owl:Class>
    


    <!-- http://humanbehaviourchange.org/ontology/BCIO_007037 -->

    <owl:Class rdf:about="http://humanbehaviourchange.org/ontology/BCIO_007037">
        <rdfs:subClassOf rdf:resource="http://humanbehaviourchange.org/ontology/BCIO_007034"/>
        <obo:IAO_0000114>Published</obo:IAO_0000114>
        <obo:IAO_0000115>An arrange support BCT that organises support from another in terms of advice, suggestions and information.</obo:IAO_0000115>
        <rdfs:label>arrange informational support BCT</rdfs:label>
    </owl:Class>
    


    <!-- http://humanbehaviourchange.org/ontology/BCIO_007038 -->

    <owl:Class rdf:about="http://humanbehaviourchange.org/ontology/BCIO_007038">
        <rdfs:subClassOf rdf:resource="http://humanbehaviourchange.org/ontology/BCIO_007034"/>
        <obo:IAO_0000114>Published</obo:IAO_0000114>
        <obo:IAO_0000115>An arrange support BCT that organises support from another in terms of information that will aid the person in evaluating themself or the situation.</obo:IAO_0000115>
        <rdfs:label>arrange appraisal support BCT</rdfs:label>
    </owl:Class>
    


    <!-- http://humanbehaviourchange.org/ontology/BCIO_007039 -->

    <owl:Class rdf:about="http://humanbehaviourchange.org/ontology/BCIO_007039">
        <rdfs:subClassOf rdf:resource="http://humanbehaviourchange.org/ontology/BCIO_007028"/>
        <obo:IAO_0000114>Published</obo:IAO_0000114>
        <obo:IAO_0000115>A social support BCT that directly provides support to the person.</obo:IAO_0000115>
        <obo:IAO_0000118>social support</obo:IAO_0000118>
        <rdfs:comment>Attending a group class and/or mention of ‘follow-up’ does not necessarily apply this BCT, support must be explicitly mentioned</rdfs:comment>
        <rdfs:label>deliver support BCT</rdfs:label>
    </owl:Class>
    


    <!-- http://humanbehaviourchange.org/ontology/BCIO_007040 -->

    <owl:Class rdf:about="http://humanbehaviourchange.org/ontology/BCIO_007040">
        <rdfs:subClassOf rdf:resource="http://humanbehaviourchange.org/ontology/BCIO_007039"/>
        <obo:IAO_0000114>Published</obo:IAO_0000114>
        <obo:IAO_0000115>A deliver support BCT that provides tangible aid.</obo:IAO_0000115>
        <obo:IAO_0000118>instrumental social support, practical social support</obo:IAO_0000118>
        <rdfs:label>deliver instrumental support BCT</rdfs:label>
    </owl:Class>
    


    <!-- http://humanbehaviourchange.org/ontology/BCIO_007041 -->

    <owl:Class rdf:about="http://humanbehaviourchange.org/ontology/BCIO_007041">
        <rdfs:subClassOf rdf:resource="http://humanbehaviourchange.org/ontology/BCIO_007039"/>
        <obo:IAO_0000114>Published</obo:IAO_0000114>
        <obo:IAO_0000115>A deliver support BCT that provides expressions of concern, caring and empathy.</obo:IAO_0000115>
        <obo:IAO_0000118>emotional social support</obo:IAO_0000118>
        <rdfs:label>deliver emotional support BCT</rdfs:label>
    </owl:Class>
    


    <!-- http://humanbehaviourchange.org/ontology/BCIO_007042 -->

    <owl:Class rdf:about="http://humanbehaviourchange.org/ontology/BCIO_007042">
        <rdfs:subClassOf rdf:resource="http://humanbehaviourchange.org/ontology/BCIO_007039"/>
        <obo:IAO_0000114>Published</obo:IAO_0000114>
        <obo:IAO_0000115>A deliver support BCT that provides advice, suggestions and information.</obo:IAO_0000115>
        <obo:IAO_0000118>information social support</obo:IAO_0000118>
        <rdfs:label>deliver informational support BCT</rdfs:label>
    </owl:Class>
    


    <!-- http://humanbehaviourchange.org/ontology/BCIO_007043 -->

    <owl:Class rdf:about="http://humanbehaviourchange.org/ontology/BCIO_007043">
        <rdfs:subClassOf rdf:resource="http://humanbehaviourchange.org/ontology/BCIO_007039"/>
        <obo:IAO_0000114>Published</obo:IAO_0000114>
        <obo:IAO_0000115>A deliver support BCT that provides information that will aid the person in evaluating themself or the situation.</obo:IAO_0000115>
        <obo:IAO_0000118>appraisal social support</obo:IAO_0000118>
        <rdfs:label>deliver appraisal support BCT</rdfs:label>
    </owl:Class>
    


    <!-- http://humanbehaviourchange.org/ontology/BCIO_007050 -->

    <owl:Class rdf:about="http://humanbehaviourchange.org/ontology/BCIO_007050">
        <rdfs:subClassOf rdf:resource="http://humanbehaviourchange.org/ontology/BCIO_033000"/>
        <obo:IAO_0000114>Published</obo:IAO_0000114>
        <obo:IAO_0000115>A behaviour change technique that provides guidance regarding how to perform the behaviour.</obo:IAO_0000115>
        <rdfs:label>guide how to perform behaviour BCT</rdfs:label>
    </owl:Class>
    


    <!-- http://humanbehaviourchange.org/ontology/BCIO_007051 -->

    <owl:Class rdf:about="http://humanbehaviourchange.org/ontology/BCIO_007051">
        <rdfs:subClassOf rdf:resource="http://humanbehaviourchange.org/ontology/BCIO_007050"/>
        <obo:IAO_0000114>Published</obo:IAO_0000114>
        <obo:IAO_0000115>A guide how to perform behaviour BCT that involves reaching consensus on how to perform the behaviour.</obo:IAO_0000115>
        <rdfs:label>agree on how to perform behaviour BCT</rdfs:label>
    </owl:Class>
    


    <!-- http://humanbehaviourchange.org/ontology/BCIO_007052 -->

    <owl:Class rdf:about="http://humanbehaviourchange.org/ontology/BCIO_007052">
        <rdfs:subClassOf rdf:resource="http://humanbehaviourchange.org/ontology/BCIO_007302"/>
        <obo:IAO_0000114>Published</obo:IAO_0000114>
        <obo:IAO_0000115>A suggest different perspective on behaviour BCT that involves providing factual information to the person regarding triggers or influences that precede the initiation of the behaviour.</obo:IAO_0000115>
        <obo:IAO_0000118>trigger recognition, understanding of antecedents</obo:IAO_0000118>
        <rdfs:label>inform about antecedents BCT</rdfs:label>
    </owl:Class>
    


    <!-- http://humanbehaviourchange.org/ontology/BCIO_007053 -->

    <owl:Class rdf:about="http://humanbehaviourchange.org/ontology/BCIO_007053">
        <rdfs:subClassOf rdf:resource="http://humanbehaviourchange.org/ontology/BCIO_007302"/>
        <obo:IAO_0000114>Published</obo:IAO_0000114>
        <obo:IAO_0000115>A suggest different perspective on behaviour BCT that involves eliciting the person&apos;s beliefs about, and suggesting alternative beliefs about, the causes of the behaviour.</obo:IAO_0000115>
        <obo:IAO_0000118>re-attribution</obo:IAO_0000118>
        <rdfs:label>re-attribute cause BCT</rdfs:label>
    </owl:Class>
    


    <!-- http://humanbehaviourchange.org/ontology/BCIO_007054 -->

    <owl:Class rdf:about="http://humanbehaviourchange.org/ontology/BCIO_007054">
        <rdfs:subClassOf rdf:resource="http://humanbehaviourchange.org/ontology/BCIO_033000"/>
        <obo:IAO_0000114>Published</obo:IAO_0000114>
        <obo:IAO_0000115>A behaviour change technique that advises on how to identify and test hypotheses about the behaviour, its causes and consequences.</obo:IAO_0000115>
        <obo:IAO_0000118>behavioural experiment</obo:IAO_0000118>
        <rdfs:label>conduct a behavioural experiment BCT</rdfs:label>
    </owl:Class>
    


    <!-- http://humanbehaviourchange.org/ontology/BCIO_007055 -->

    <owl:Class rdf:about="http://humanbehaviourchange.org/ontology/BCIO_007055">
        <rdfs:subClassOf rdf:resource="http://humanbehaviourchange.org/ontology/BCIO_007050"/>
        <obo:IAO_0000114>Published</obo:IAO_0000114>
        <obo:IAO_0000115>A guide how to perform behaviour BCT that provides an observable sample of the performance of the behaviour for the person to aspire to or imitate.</obo:IAO_0000115>
        <obo:IAO_0000118>modelling, observational learning</obo:IAO_0000118>
        <rdfs:comment> If provided with instructions on how to perform, also code &apos;instruct how to perform behaviour BCT&apos;.</rdfs:comment>
        <rdfs:comment>If advised to practice, also code &apos;practise behaviour BCT&apos;</rdfs:comment>
        <rdfs:label>demonstrate the behaviour BCT</rdfs:label>
    </owl:Class>
    


    <!-- http://humanbehaviourchange.org/ontology/BCIO_007056 -->

    <owl:Class rdf:about="http://humanbehaviourchange.org/ontology/BCIO_007056">
        <rdfs:subClassOf rdf:resource="http://humanbehaviourchange.org/ontology/BCIO_007302"/>
        <obo:IAO_0000114>Published</obo:IAO_0000114>
        <obo:IAO_0000115>A suggest different perspective on behaviour BCT that involves reattributing a person&apos;s successes to internal, stable or global factors or failures to external, unstable or specific factors.</obo:IAO_0000115>
        <obo:IAO_0000118>cognitive re-structuring, re-attribution</obo:IAO_0000118>
        <rdfs:label>reframe past behaviour BCT</rdfs:label>
    </owl:Class>
    


    <!-- http://humanbehaviourchange.org/ontology/BCIO_007057 -->

    <owl:Class rdf:about="http://humanbehaviourchange.org/ontology/BCIO_007057">
        <rdfs:subClassOf rdf:resource="http://humanbehaviourchange.org/ontology/BCIO_007302"/>
        <obo:IAO_0000114>Published</obo:IAO_0000114>
        <obo:IAO_0000115>A suggest different perspective on behaviour BCT that draws the person&apos;s attention to the discrepancies between current or past behaviour and self-identity.</obo:IAO_0000115>
        <obo:IAO_0000118>cognitive dissonance</obo:IAO_0000118>
        <rdfs:label>draw attention to incompatible beliefs BCT</rdfs:label>
    </owl:Class>
    


    <!-- http://humanbehaviourchange.org/ontology/BCIO_007058 -->

    <owl:Class rdf:about="http://humanbehaviourchange.org/ontology/BCIO_007058">
        <rdfs:subClassOf rdf:resource="http://humanbehaviourchange.org/ontology/BCIO_007050"/>
        <obo:IAO_0000114>Published</obo:IAO_0000114>
        <obo:IAO_0000115>A guide how to perform behaviour BCT that involves telling the person how to perform the behaviour.</obo:IAO_0000115>
        <obo:IAO_0000118>skills training, instruction</obo:IAO_0000118>
        <rdfs:comment>When the person attends classes such as exercise or cookery, code &apos;instruct how to perform behaviour BCT&apos;, &apos;practise behaviour BCT&apos;, and &apos;demonstrate the behaviour BCT&apos;.</rdfs:comment>
        <rdfs:label>instruct how to perform a behaviour BCT</rdfs:label>
    </owl:Class>
    


    <!-- http://humanbehaviourchange.org/ontology/BCIO_007060 -->

    <owl:Class rdf:about="http://humanbehaviourchange.org/ontology/BCIO_007060">
        <rdfs:subClassOf rdf:resource="http://humanbehaviourchange.org/ontology/BCIO_007239"/>
        <obo:IAO_0000114>Published</obo:IAO_0000114>
        <obo:IAO_0000115>A prompt thinking related to successful performance BCT that reminds the person of their skills and abilities that are relevant to the performance of the behaviour.</obo:IAO_0000115>
        <rdfs:label>remind about personal capability BCT</rdfs:label>
    </owl:Class>
    


    <!-- http://humanbehaviourchange.org/ontology/BCIO_007061 -->

    <owl:Class rdf:about="http://humanbehaviourchange.org/ontology/BCIO_007061">
        <rdfs:subClassOf rdf:resource="http://humanbehaviourchange.org/ontology/BCIO_007001"/>
        <obo:IAO_0000114>Published</obo:IAO_0000114>
        <obo:IAO_0000115>A goal directed BCT that advises the person to plan a way of performing the behaviour that is pleasurable or satisfying.</obo:IAO_0000115>
        <rdfs:label>plan inclusion of enjoyment BCT</rdfs:label>
    </owl:Class>
    


    <!-- http://humanbehaviourchange.org/ontology/BCIO_007062 -->

    <owl:Class rdf:about="http://humanbehaviourchange.org/ontology/BCIO_007062">
        <rdfs:subClassOf rdf:resource="http://humanbehaviourchange.org/ontology/BCIO_033000"/>
        <obo:IAO_0000114>Published</obo:IAO_0000114>
        <obo:IAO_0000115>A behaviour change technique that draws attention to consequences of the behaviour in the normal course of events.</obo:IAO_0000115>
        <rdfs:label>increase awareness of consequences BCT</rdfs:label>
    </owl:Class>
    


    <!-- http://humanbehaviourchange.org/ontology/BCIO_007063 -->

    <owl:Class rdf:about="http://humanbehaviourchange.org/ontology/BCIO_007063">
        <rdfs:subClassOf rdf:resource="http://humanbehaviourchange.org/ontology/BCIO_007062"/>
        <obo:IAO_0000114>Published</obo:IAO_0000114>
        <obo:IAO_0000115>An increase awareness of consequences BCT that provides information about the physical or mental health consequences of performing or not performing the behaviour.</obo:IAO_0000115>
        <obo:IAO_0000118>consequences for well-being, health effects, wellness outcomes</obo:IAO_0000118>
        <rdfs:comment> emphasising importance of consequences is not sufficient.</rdfs:comment>
        <rdfs:comment>Consequences can be for any target, not just the recipient(s) of the intervention</rdfs:comment>
        <rdfs:label>inform about health consequences BCT</rdfs:label>
    </owl:Class>
    


    <!-- http://humanbehaviourchange.org/ontology/BCIO_007064 -->

    <owl:Class rdf:about="http://humanbehaviourchange.org/ontology/BCIO_007064">
        <rdfs:subClassOf rdf:resource="http://humanbehaviourchange.org/ontology/BCIO_007062"/>
        <obo:IAO_0000114>Published</obo:IAO_0000114>
        <obo:IAO_0000115>An increase awareness of consequences BCT that provides information about the social consequences of performing or not performing the behaviour.</obo:IAO_0000115>
        <obo:IAO_0000118>social effects, community repercussions</obo:IAO_0000118>
        <rdfs:comment> emphasising importance of consequences is not sufficient.</rdfs:comment>
        <rdfs:comment>Consequences can be for any target, not just the recipient(s) of the intervention</rdfs:comment>
        <rdfs:label>inform about social consequences BCT</rdfs:label>
    </owl:Class>
    


    <!-- http://humanbehaviourchange.org/ontology/BCIO_007065 -->

    <owl:Class rdf:about="http://humanbehaviourchange.org/ontology/BCIO_007065">
        <rdfs:subClassOf rdf:resource="http://humanbehaviourchange.org/ontology/BCIO_007062"/>
        <obo:IAO_0000114>Published</obo:IAO_0000114>
        <obo:IAO_0000115>An increase awareness of consequences BCT that provides information about the emotional consequences of performing or not performing the behaviour.</obo:IAO_0000115>
        <obo:IAO_0000118>affective outcomes, emotional effects, consequences on emotions</obo:IAO_0000118>
        <rdfs:comment> emphasising importance of consequences is not sufficient. Consequences can be related to emotional health disorders (e.g. depression, anxiety) and/or states of mind (e.g. low mood, stress).</rdfs:comment>
        <rdfs:comment>Consequences can be for any target, not just the recipient(s) of the intervention</rdfs:comment>
        <rdfs:label>inform about emotional consequences BCT</rdfs:label>
    </owl:Class>
    


    <!-- http://humanbehaviourchange.org/ontology/BCIO_007066 -->

    <owl:Class rdf:about="http://humanbehaviourchange.org/ontology/BCIO_007066">
        <rdfs:subClassOf rdf:resource="http://humanbehaviourchange.org/ontology/BCIO_007017"/>
        <obo:IAO_0000114>Published</obo:IAO_0000114>
        <obo:IAO_0000115>A monitoring BCT that involves the person assessing their emotions after performing the behaviour.</obo:IAO_0000115>
        <rdfs:label>monitor emotional consequences BCT</rdfs:label>
    </owl:Class>
    


    <!-- http://humanbehaviourchange.org/ontology/BCIO_007067 -->

    <owl:Class rdf:about="http://humanbehaviourchange.org/ontology/BCIO_007067">
        <rdfs:subClassOf rdf:resource="http://humanbehaviourchange.org/ontology/BCIO_007065"/>
        <obo:IAO_0000114>Published</obo:IAO_0000114>
        <obo:IAO_0000115>An inform about emotional consequences BCT that focuses on expectations of remorse after performing or not performing the behaviour.</obo:IAO_0000115>
        <rdfs:comment>If suggests adoption of a perspective or new perspective in order to change cognitions also code &apos;suggest different perspective on behaviour BCT&apos; or one of its child classes</rdfs:comment>
        <rdfs:label>induce anticipated regret BCT</rdfs:label>
    </owl:Class>
    


    <!-- http://humanbehaviourchange.org/ontology/BCIO_007068 -->

    <owl:Class rdf:about="http://humanbehaviourchange.org/ontology/BCIO_007068">
        <rdfs:subClassOf rdf:resource="http://humanbehaviourchange.org/ontology/BCIO_007062"/>
        <obo:IAO_0000114>Published</obo:IAO_0000114>
        <obo:IAO_0000115>An awareness of consequences BCT that changes behaviour by the source emphasising the consequences of performing a behaviour to the person in a way that makes them memorable.</obo:IAO_0000115>
        <obo:IAO_0000118>significance of outcomes, importance of consequences, relevance of results</obo:IAO_0000118>
        <rdfs:comment>Consider also coding one of &quot;inform about health consequences&quot;, &quot;inform about emotional consequences&quot;,  &quot;inform about social consequences&quot;, or their child classes</rdfs:comment>
        <rdfs:label>increase salience of consequences BCT</rdfs:label>
    </owl:Class>
    


    <!-- http://humanbehaviourchange.org/ontology/BCIO_007069 -->

    <owl:Class rdf:about="http://humanbehaviourchange.org/ontology/BCIO_007069">
        <rdfs:subClassOf rdf:resource="http://humanbehaviourchange.org/ontology/BCIO_007062"/>
        <obo:IAO_0000114>Published</obo:IAO_0000114>
        <obo:IAO_0000115>An increase awareness of consequences BCT that advises identification and comparison of the positive and negative consequences of performing or not performing the behaviour.</obo:IAO_0000115>
        <obo:IAO_0000118>decisional balance, weighing pros and cons</obo:IAO_0000118>
        <rdfs:label>consider pros and cons BCT</rdfs:label>
    </owl:Class>
    


    <!-- http://humanbehaviourchange.org/ontology/BCIO_007070 -->

    <owl:Class rdf:about="http://humanbehaviourchange.org/ontology/BCIO_007070">
        <rdfs:subClassOf rdf:resource="http://humanbehaviourchange.org/ontology/BCIO_007062"/>
        <obo:IAO_0000114>Published</obo:IAO_0000114>
        <obo:IAO_0000115>An increase awareness of consequences BCT that guides the person to imagine and compare the consequences of performing and not performing the behaviour.</obo:IAO_0000115>
        <obo:IAO_0000118>imagining future results</obo:IAO_0000118>
        <rdfs:label>prompt comparative imagining of future outcomes BCT</rdfs:label>
    </owl:Class>
    


    <!-- http://humanbehaviourchange.org/ontology/BCIO_007072 -->

    <owl:Class rdf:about="http://humanbehaviourchange.org/ontology/BCIO_007072">
        <rdfs:subClassOf rdf:resource="http://humanbehaviourchange.org/ontology/BCIO_033000"/>
        <obo:IAO_0000114>Published</obo:IAO_0000114>
        <obo:IAO_0000115>A behaviour change technique that increases awareness of what other people think, do, or feel.</obo:IAO_0000115>
        <rdfs:label>awareness of other peoples thoughts, feelings and actions BCT</rdfs:label>
    </owl:Class>
    


    <!-- http://humanbehaviourchange.org/ontology/BCIO_007073 -->

    <owl:Class rdf:about="http://humanbehaviourchange.org/ontology/BCIO_007073">
        <rdfs:subClassOf rdf:resource="http://humanbehaviourchange.org/ontology/BCIO_007072"/>
        <obo:IAO_0000114>Published</obo:IAO_0000114>
        <obo:IAO_0000115>An awareness of other people&apos;s thoughts, feelings and actions BCT that draws attention to other people&apos;s behaviour and compares it with the person&apos;s own behaviour.</obo:IAO_0000115>
        <obo:IAO_0000118>social comparison</obo:IAO_0000118>
        <rdfs:comment>Being in a group setting does not necessarily mean that social comparison is actually taking place</rdfs:comment>
        <rdfs:label>prompt social comparison BCT</rdfs:label>
    </owl:Class>
    


    <!-- http://humanbehaviourchange.org/ontology/BCIO_007074 -->

    <owl:Class rdf:about="http://humanbehaviourchange.org/ontology/BCIO_007074">
        <rdfs:subClassOf rdf:resource="http://humanbehaviourchange.org/ontology/BCIO_007072"/>
        <obo:IAO_0000114>Published</obo:IAO_0000114>
        <obo:IAO_0000115>An awareness of other people&apos;s thoughts, feelings and actions BCT that increases awareness of whether others will like, approve, dislike, or disapprove of the behaviour.</obo:IAO_0000115>
        <rdfs:label>increase awareness of others approval BCT</rdfs:label>
    </owl:Class>
    


    <!-- http://humanbehaviourchange.org/ontology/BCIO_007075 -->

    <owl:Class rdf:about="http://humanbehaviourchange.org/ontology/BCIO_007075">
        <rdfs:subClassOf rdf:resource="http://humanbehaviourchange.org/ontology/BCIO_007072"/>
        <obo:IAO_0000114>Published</obo:IAO_0000114>
        <obo:IAO_0000115>An awareness of other people&apos;s thoughts, feelings and actions BCT that presents information from a credible person or organisation to influence the behaviour.</obo:IAO_0000115>
        <rdfs:comment>Code this BCT if influence generally agreed on as credible e.g., health professionals, celebrities or words used to indicate expertise or leader in field and if the communication has the aim of persuading</rdfs:comment>
        <rdfs:label>present information from credible influence BCT</rdfs:label>
    </owl:Class>
    


    <!-- http://humanbehaviourchange.org/ontology/BCIO_007076 -->

    <owl:Class rdf:about="http://humanbehaviourchange.org/ontology/BCIO_007076">
        <rdfs:subClassOf rdf:resource="http://humanbehaviourchange.org/ontology/BCIO_007072"/>
        <obo:IAO_0000114>Published</obo:IAO_0000114>
        <obo:IAO_0000115>An awareness of other people&apos;s thoughts, feelings and actions BCT that involves sharing a view about what behaviour the person should do.</obo:IAO_0000115>
        <obo:IAO_0000118>encourage to change behaviour</obo:IAO_0000118>
        <rdfs:comment>An example of the &quot;suggest to change behaviour BCT&quot; would be saying to someone: &quot;I think you should do this behaviour&quot; whereas an example of the &quot;Tell to change behaviour BCT&quot; is saying &quot;Do this behaviour&quot;. This class includes &quot;strongly encourage&quot;.</rdfs:comment>
        <rdfs:label>suggest to change behaviour BCT</rdfs:label>
    </owl:Class>
    


    <!-- http://humanbehaviourchange.org/ontology/BCIO_007077 -->

    <owl:Class rdf:about="http://humanbehaviourchange.org/ontology/BCIO_007077">
        <rdfs:subClassOf rdf:resource="http://humanbehaviourchange.org/ontology/BCIO_007072"/>
        <obo:IAO_0000114>Published</obo:IAO_0000114>
        <obo:IAO_0000115>An awareness of other people&apos;s thoughts, feelings and actions BCT that involves telling the person to perform the behaviour.</obo:IAO_0000115>
        <obo:IAO_0000118>instruct, command</obo:IAO_0000118>
        <rdfs:comment>An example of the &quot;Tell to change behaviour BCT&quot; is saying &quot;Do this behaviour&quot; whereas an example of the &quot;suggest to change behaviour BCT&quot; would be saying to someone: &quot;I think you should do this behaviour.&quot;</rdfs:comment>
        <rdfs:label>tell to change behaviour BCT</rdfs:label>
    </owl:Class>
    


    <!-- http://humanbehaviourchange.org/ontology/BCIO_007078 -->

    <owl:Class rdf:about="http://humanbehaviourchange.org/ontology/BCIO_007078">
        <rdfs:subClassOf rdf:resource="http://humanbehaviourchange.org/ontology/BCIO_007072"/>
        <obo:IAO_0000114>Published</obo:IAO_0000114>
        <obo:IAO_0000115>An awareness of other people&apos;s thoughts, feelings and actions BCT that makes an emotional or earnest appeal to change the person&apos;s behaviour.</obo:IAO_0000115>
        <rdfs:label>implore to change behaviour BCT</rdfs:label>
    </owl:Class>
    


    <!-- http://humanbehaviourchange.org/ontology/BCIO_007079 -->

    <owl:Class rdf:about="http://humanbehaviourchange.org/ontology/BCIO_007079">
        <rdfs:subClassOf rdf:resource="http://humanbehaviourchange.org/ontology/BCIO_007090"/>
        <obo:IAO_0000114>Published</obo:IAO_0000114>
        <obo:IAO_0000115>An associative learning BCT that involves creating, strengthening or reducing an association between the behaviour and an environmental trigger.</obo:IAO_0000115>
        <rdfs:label>alter external stimulus BCT</rdfs:label>
    </owl:Class>
    


    <!-- http://humanbehaviourchange.org/ontology/BCIO_007080 -->

    <owl:Class rdf:about="http://humanbehaviourchange.org/ontology/BCIO_007080">
        <rdfs:subClassOf rdf:resource="http://humanbehaviourchange.org/ontology/BCIO_007079"/>
        <obo:IAO_0000114>Published</obo:IAO_0000114>
        <obo:IAO_0000115>An alter external stimulus BCT that involves introducing an external stimulus to facilitate the behaviour for which an intention has previously been formed.</obo:IAO_0000115>
        <obo:IAO_0000118>prompts</obo:IAO_0000118>
        <rdfs:comment>When a stimulus is linked to a specific action in an if-then plan including one or more of frequency, duration or intensity also code &apos;action planning BCT&apos;</rdfs:comment>
        <rdfs:label>prompt intended action BCT</rdfs:label>
    </owl:Class>
    


    <!-- http://humanbehaviourchange.org/ontology/BCIO_007081 -->

    <owl:Class rdf:about="http://humanbehaviourchange.org/ontology/BCIO_007081">
        <rdfs:subClassOf rdf:resource="http://humanbehaviourchange.org/ontology/BCIO_007079"/>
        <obo:IAO_0000114>Published</obo:IAO_0000114>
        <obo:IAO_0000115>An alter external stimulus BCT that introduces external information that is already associated with the behaviour in order to elicit that behaviour.</obo:IAO_0000115>
        <obo:IAO_0000118>cues</obo:IAO_0000118>
        <rdfs:comment>When a stimulus is linked to a specific action in an if-then plan including one or more of frequency, duration or intensity also code &apos;action planning BCT&apos;</rdfs:comment>
        <rdfs:label>cue BCT</rdfs:label>
    </owl:Class>
    


    <!-- http://humanbehaviourchange.org/ontology/BCIO_007082 -->

    <owl:Class rdf:about="http://humanbehaviourchange.org/ontology/BCIO_007082">
        <rdfs:subClassOf rdf:resource="http://humanbehaviourchange.org/ontology/BCIO_007079"/>
        <obo:IAO_0000114>Published</obo:IAO_0000114>
        <obo:IAO_0000115>An alter external stimulus BCT that identifies an external stimulus that reliably signals that reward will follow the behaviour.</obo:IAO_0000115>
        <obo:IAO_0000118>discriminative stimulus for reward</obo:IAO_0000118>
        <rdfs:label>cue signalling reward BCT</rdfs:label>
    </owl:Class>
    


    <!-- http://humanbehaviourchange.org/ontology/BCIO_007084 -->

    <owl:Class rdf:about="http://humanbehaviourchange.org/ontology/BCIO_007084">
        <rdfs:subClassOf rdf:resource="http://humanbehaviourchange.org/ontology/BCIO_007079"/>
        <obo:IAO_0000114>Published</obo:IAO_0000114>
        <obo:IAO_0000115>An alter external stimulus BCT in which cues for the behaviour are presented less frequently.</obo:IAO_0000115>
        <obo:IAO_0000118>fading</obo:IAO_0000118>
        <rdfs:comment>The reduction in frequency of cue presentation can be gradual or rapid. This BCT is concerned with reducing the frequency of cue presentation. In contrast, in &quot;reduce exposure to cues for the behaviour BCT&quot;, the cue frequency may remain unchanged but the person&apos;s exposure to the presentation of the cue is reduced.</rdfs:comment>
        <rdfs:label>reduce cue frequency BCTs</rdfs:label>
    </owl:Class>
    


    <!-- http://humanbehaviourchange.org/ontology/BCIO_007085 -->

    <owl:Class rdf:about="http://humanbehaviourchange.org/ontology/BCIO_007085">
        <rdfs:subClassOf rdf:resource="http://humanbehaviourchange.org/ontology/BCIO_007079"/>
        <obo:IAO_0000114>Published</obo:IAO_0000114>
        <obo:IAO_0000115>An alter external stimulus BCT that sustains the person&apos;s exposure to a stimulus associated with the behaviour.</obo:IAO_0000115>
        <obo:IAO_0000118>exposure</obo:IAO_0000118>
        <rdfs:label>expose to stimulus BCT</rdfs:label>
    </owl:Class>
    


    <!-- http://humanbehaviourchange.org/ontology/BCIO_007087 -->

    <owl:Class rdf:about="http://humanbehaviourchange.org/ontology/BCIO_007087">
        <rdfs:subClassOf rdf:resource="http://humanbehaviourchange.org/ontology/BCIO_007085"/>
        <obo:IAO_0000114>Published</obo:IAO_0000114>
        <obo:IAO_0000115>An expose to stimulus BCT that provides sustained exposure to a stimulus to reduce or extinguish an unwanted behaviour.</obo:IAO_0000115>
        <rdfs:label>arrange satiation BCT</rdfs:label>
    </owl:Class>
    


    <!-- http://humanbehaviourchange.org/ontology/BCIO_007089 -->

    <owl:Class rdf:about="http://humanbehaviourchange.org/ontology/BCIO_007089">
        <rdfs:subClassOf rdf:resource="http://humanbehaviourchange.org/ontology/BCIO_007085"/>
        <obo:IAO_0000114>Published</obo:IAO_0000114>
        <obo:IAO_0000115>An expose to stimulus BCT that gradually exposes the person to an aversive stimulus while also engaging them in a relaxation process to reduce the response to that stimulus.</obo:IAO_0000115>
        <rdfs:label>systematically desensitise BCT</rdfs:label>
    </owl:Class>
    


    <!-- http://humanbehaviourchange.org/ontology/BCIO_007090 -->

    <owl:Class rdf:about="http://humanbehaviourchange.org/ontology/BCIO_007090">
        <rdfs:subClassOf rdf:resource="http://humanbehaviourchange.org/ontology/BCIO_033000"/>
        <obo:IAO_0000114>Published</obo:IAO_0000114>
        <obo:IAO_0000115>A behaviour change technique that involves repeated pairing of a stimulus with another stimulus or with a behavioural outcome.</obo:IAO_0000115>
        <obo:IAO_0000118>Classical conditioning, Pavlovian conditioning</obo:IAO_0000118>
        <rdfs:comment>When this BCT involves reward or punishment, consider &apos;behavioural consequence BCT&apos; and its child classes</rdfs:comment>
        <rdfs:label>associative learning BCT</rdfs:label>
    </owl:Class>
    


    <!-- http://humanbehaviourchange.org/ontology/BCIO_007091 -->

    <owl:Class rdf:about="http://humanbehaviourchange.org/ontology/BCIO_007091">
        <rdfs:subClassOf rdf:resource="http://humanbehaviourchange.org/ontology/BCIO_007090"/>
        <obo:IAO_0000114>Published</obo:IAO_0000114>
        <obo:IAO_0000115>An associative learning BCT that involves repeated pairing of a neutral stimulus with a stimulus that already elicits the behaviour until the neutral stimulus elicits the behaviour.</obo:IAO_0000115>
        <obo:IAO_0000118>Classical conditioning, Pavlovian conditioning</obo:IAO_0000118>
        <rdfs:label>associative learning to elicit behaviour BCT</rdfs:label>
    </owl:Class>
    


    <!-- http://humanbehaviourchange.org/ontology/BCIO_007092 -->

    <owl:Class rdf:about="http://humanbehaviourchange.org/ontology/BCIO_007092">
        <rdfs:subClassOf rdf:resource="http://humanbehaviourchange.org/ontology/BCIO_007090"/>
        <obo:IAO_0000114>Published</obo:IAO_0000114>
        <obo:IAO_0000115>An associative learning BCT that stops the presentation of a reward for the behaviour.</obo:IAO_0000115>
        <obo:IAO_0000118>extinction, elimination of reinforcement</obo:IAO_0000118>
        <rdfs:label>associative learning to extinguish behaviour BCT</rdfs:label>
    </owl:Class>
    


    <!-- http://humanbehaviourchange.org/ontology/BCIO_007094 -->

    <owl:Class rdf:about="http://humanbehaviourchange.org/ontology/BCIO_007094">
        <rdfs:subClassOf rdf:resource="http://humanbehaviourchange.org/ontology/BCIO_007168"/>
        <obo:IAO_0000114>Published</obo:IAO_0000114>
        <obo:IAO_0000115>An advise specific behaviour BCT that advises repetition of the behaviour in a way that has the function of increasing the skill in performing the behaviour.</obo:IAO_0000115>
        <obo:IAO_0000118>skill practise, rehearsal</obo:IAO_0000118>
        <rdfs:comment>If aiming to associate performance with the context, also code &apos;context-specific repetition of behaviour BCT&apos;</rdfs:comment>
        <rdfs:label>practise behaviour BCT</rdfs:label>
    </owl:Class>
    


    <!-- http://humanbehaviourchange.org/ontology/BCIO_007095 -->

    <owl:Class rdf:about="http://humanbehaviourchange.org/ontology/BCIO_007095">
        <rdfs:subClassOf rdf:resource="http://humanbehaviourchange.org/ontology/BCIO_007168"/>
        <obo:IAO_0000114>Published</obo:IAO_0000114>
        <obo:IAO_0000115>An advise specific behaviour BCT that advises the person to replace the unwanted behaviour with another behaviour.</obo:IAO_0000115>
        <obo:IAO_0000118>behaviour replacement, alternative response</obo:IAO_0000118>
        <rdfs:comment>If this occurs regularly, also code &apos;context-specific repetition of alternative behaviour BCT&apos;</rdfs:comment>
        <rdfs:label>substitute behaviour BCT</rdfs:label>
    </owl:Class>
    


    <!-- http://humanbehaviourchange.org/ontology/BCIO_007096 -->

    <owl:Class rdf:about="http://humanbehaviourchange.org/ontology/BCIO_007096">
        <rdfs:subClassOf rdf:resource="http://humanbehaviourchange.org/ontology/BCIO_007168"/>
        <obo:IAO_0000114>Published</obo:IAO_0000114>
        <obo:IAO_0000115>An advise specific behaviour BCT that advises the person to repeat the behaviour in the same context.</obo:IAO_0000115>
        <obo:IAO_0000118>habit formation, habit development</obo:IAO_0000118>
        <rdfs:comment>For the purposes of this BCT, preceding behaviour can be considered part of the context. Also code &apos;practise behaviour BCT&apos;</rdfs:comment>
        <rdfs:label>context-specific repetition of behaviour BCT</rdfs:label>
    </owl:Class>
    


    <!-- http://humanbehaviourchange.org/ontology/BCIO_007097 -->

    <owl:Class rdf:about="http://humanbehaviourchange.org/ontology/BCIO_007097">
        <rdfs:subClassOf rdf:resource="http://humanbehaviourchange.org/ontology/BCIO_007168"/>
        <obo:IAO_0000114>Published</obo:IAO_0000114>
        <obo:IAO_0000115>An advise specific behaviour BCT that advises the person to repeat an alternative behaviour consistently in a context that previously elicited an unwanted behaviour.</obo:IAO_0000115>
        <obo:IAO_0000118>habit reversal, breaking a habit, habit elimination</obo:IAO_0000118>
        <rdfs:comment>For the purposes of this BCT, preceding behaviour can be considered part of the context. Also code &apos;substitute behaviour BCT&apos;</rdfs:comment>
        <rdfs:label>context-specific repetition of alternative behaviour BCT</rdfs:label>
    </owl:Class>
    


    <!-- http://humanbehaviourchange.org/ontology/BCIO_007098 -->

    <owl:Class rdf:about="http://humanbehaviourchange.org/ontology/BCIO_007098">
        <rdfs:subClassOf rdf:resource="http://humanbehaviourchange.org/ontology/BCIO_007168"/>
        <obo:IAO_0000114>Published</obo:IAO_0000114>
        <obo:IAO_0000115>An advise specific behaviour BCT that advises the person to repeat a wanted behaviour in an exaggerated way following performance of an unwanted behaviour.</obo:IAO_0000115>
        <obo:IAO_0000118>overcorrection, remedial overcompensation</obo:IAO_0000118>
        <rdfs:label>overcorrect unwanted behaviour BCT</rdfs:label>
    </owl:Class>
    


    <!-- http://humanbehaviourchange.org/ontology/BCIO_007099 -->

    <owl:Class rdf:about="http://humanbehaviourchange.org/ontology/BCIO_007099">
        <rdfs:subClassOf rdf:resource="http://humanbehaviourchange.org/ontology/BCIO_007168"/>
        <obo:IAO_0000114>Published</obo:IAO_0000114>
        <obo:IAO_0000115>An advise specific behaviour BCT that advises the person to perform the behaviour which is already performed in a particular context, in a similar context.</obo:IAO_0000115>
        <obo:IAO_0000118>universalisation of behaviour</obo:IAO_0000118>
        <rdfs:label>generalise behaviour BCT</rdfs:label>
    </owl:Class>
    


    <!-- http://humanbehaviourchange.org/ontology/BCIO_007100 -->

    <owl:Class rdf:about="http://humanbehaviourchange.org/ontology/BCIO_007100">
        <rdfs:subClassOf rdf:resource="http://humanbehaviourchange.org/ontology/BCIO_007001"/>
        <obo:IAO_0000114>Published</obo:IAO_0000114>
        <obo:IAO_0000115>A goal directed BCT that sets easy-to-perform tasks for the person, making them increasingly difficult, but achievable, until the behaviour is performed.</obo:IAO_0000115>
        <obo:IAO_0000118>graded tasks</obo:IAO_0000118>
        <rdfs:label>set graded tasks BCT</rdfs:label>
    </owl:Class>
    


    <!-- http://humanbehaviourchange.org/ontology/BCIO_007101 -->

    <owl:Class rdf:about="http://humanbehaviourchange.org/ontology/BCIO_007101">
        <rdfs:subClassOf rdf:resource="http://humanbehaviourchange.org/ontology/BCIO_033000"/>
        <obo:IAO_0000114>Published</obo:IAO_0000114>
        <obo:IAO_0000115>A behaviour change technique that alters the consequences or promised consequences for the behaviour.</obo:IAO_0000115>
        <rdfs:label>behavioural consequence BCT</rdfs:label>
    </owl:Class>
    


    <!-- http://humanbehaviourchange.org/ontology/BCIO_007118 -->

    <owl:Class rdf:about="http://humanbehaviourchange.org/ontology/BCIO_007118">
        <rdfs:subClassOf rdf:resource="http://humanbehaviourchange.org/ontology/BCIO_007062"/>
        <obo:IAO_0000114>Published</obo:IAO_0000114>
        <obo:IAO_0000115>An increase awareness of consequences BCT that guides the person to imagine performing the unwanted behaviour in a real-life situation followed by experiencing an unpleasant consequence for performing that behaviour.</obo:IAO_0000115>
        <obo:IAO_0000118>covert sensitisation</obo:IAO_0000118>
        <rdfs:label>imagine punishment BCT</rdfs:label>
    </owl:Class>
    


    <!-- http://humanbehaviourchange.org/ontology/BCIO_007119 -->

    <owl:Class rdf:about="http://humanbehaviourchange.org/ontology/BCIO_007119">
        <rdfs:subClassOf rdf:resource="http://humanbehaviourchange.org/ontology/BCIO_007062"/>
        <obo:IAO_0000114>Published</obo:IAO_0000114>
        <obo:IAO_0000115>An increase awareness of consequences BCT that guides the person to imagine performing the wanted behaviour in a real-life situation followed by experiencing a pleasant consequence for performing that behaviour.</obo:IAO_0000115>
        <obo:IAO_0000118>covert conditioning</obo:IAO_0000118>
        <rdfs:label>imagine reward BCT</rdfs:label>
    </owl:Class>
    


    <!-- http://humanbehaviourchange.org/ontology/BCIO_007120 -->

    <owl:Class rdf:about="http://humanbehaviourchange.org/ontology/BCIO_007120">
        <rdfs:subClassOf rdf:resource="http://humanbehaviourchange.org/ontology/BCIO_007062"/>
        <obo:IAO_0000114>Published</obo:IAO_0000114>
        <obo:IAO_0000115>An increase awareness of consequences BCT that prompts observation of another person being rewarded when they perform the behaviour.</obo:IAO_0000115>
        <obo:IAO_0000118>vicarious reinforcement</obo:IAO_0000118>
        <rdfs:label>vicarious reward BCT</rdfs:label>
    </owl:Class>
    


    <!-- http://humanbehaviourchange.org/ontology/BCIO_007121 -->

    <owl:Class rdf:about="http://humanbehaviourchange.org/ontology/BCIO_007121">
        <rdfs:subClassOf rdf:resource="http://humanbehaviourchange.org/ontology/BCIO_007062"/>
        <obo:IAO_0000114>Published</obo:IAO_0000114>
        <obo:IAO_0000115>An increase awareness of consequences BCT that prompts observation of another person being punished when they perform the behaviour.</obo:IAO_0000115>
        <rdfs:label>vicarious punishment BCT</rdfs:label>
    </owl:Class>
    


    <!-- http://humanbehaviourchange.org/ontology/BCIO_007122 -->

    <owl:Class rdf:about="http://humanbehaviourchange.org/ontology/BCIO_007122">
        <rdfs:subClassOf rdf:resource="http://humanbehaviourchange.org/ontology/BCIO_007001"/>
        <obo:IAO_0000114>Published</obo:IAO_0000114>
        <obo:IAO_0000115>A goal directed BCT that involves the person communicating their intention to achieve a goal.</obo:IAO_0000115>
        <rdfs:comment>The goal being made public can be in terms of behaviour (e.g. to walk for 30 minutes a day) or an outcome of behaviour (e.g. to lose 5kg of body weight)</rdfs:comment>
        <rdfs:label>make a goal public BCT</rdfs:label>
    </owl:Class>
    


    <!-- http://humanbehaviourchange.org/ontology/BCIO_007134 -->

    <owl:Class rdf:about="http://humanbehaviourchange.org/ontology/BCIO_007134">
        <rdfs:subClassOf rdf:resource="http://humanbehaviourchange.org/ontology/BCIO_007185"/>
        <obo:IAO_0000112>Advise the person to carry food calorie information to reduce burden on memory when deciding what to eat.</obo:IAO_0000112>
        <obo:IAO_0000114>Published</obo:IAO_0000114>
        <obo:IAO_0000115>A manage mental processes BCT that advises a way to minimise demands on mental resources.</obo:IAO_0000115>
        <rdfs:label>conserve mental resources BCT</rdfs:label>
    </owl:Class>
    


    <!-- http://humanbehaviourchange.org/ontology/BCIO_007135 -->

    <owl:Class rdf:about="http://humanbehaviourchange.org/ontology/BCIO_007135">
        <rdfs:subClassOf rdf:resource="http://humanbehaviourchange.org/ontology/BCIO_007168"/>
        <obo:IAO_0000112>asking someone to smoke lots of cigarettes as a part of a quit smoking intervention.</obo:IAO_0000112>
        <obo:IAO_0000114>Published</obo:IAO_0000114>
        <obo:IAO_0000115>An advise specific behaviour BCT that advises the person to engage in an unwanted behaviour in a way that is aversive.</obo:IAO_0000115>
        <obo:IAO_0000118>paradoxical instructions</obo:IAO_0000118>
        <rdfs:label>advise paradoxical behaviour BCT</rdfs:label>
    </owl:Class>
    


    <!-- http://humanbehaviourchange.org/ontology/BCIO_007136 -->

    <owl:Class rdf:about="http://humanbehaviourchange.org/ontology/BCIO_007136">
        <rdfs:subClassOf rdf:resource="http://humanbehaviourchange.org/ontology/BCIO_033000"/>
        <obo:IAO_0000112> bariatric surgery meaning a person has to limit their food intake</obo:IAO_0000112>
        <obo:IAO_0000112>increasing physical strength or flexibility to facilitate walking outdoors</obo:IAO_0000112>
        <obo:IAO_0000114>Published</obo:IAO_0000114>
        <obo:IAO_0000115>A behaviour change technique that alters the structure or functioning of the person&apos;s body.</obo:IAO_0000115>
        <rdfs:label>change the body BCT</rdfs:label>
    </owl:Class>
    


    <!-- http://humanbehaviourchange.org/ontology/BCIO_007137 -->

    <owl:Class rdf:about="http://humanbehaviourchange.org/ontology/BCIO_007137">
        <rdfs:subClassOf rdf:resource="http://humanbehaviourchange.org/ontology/BCIO_007239"/>
        <obo:IAO_0000112> asserting that the person can and will succeed.</obo:IAO_0000112>
        <obo:IAO_0000112>Arguing against self-doubts</obo:IAO_0000112>
        <obo:IAO_0000114>Published</obo:IAO_0000114>
        <obo:IAO_0000115>A prompt thinking related to successful performance BCT that persuades the person that they can successfully perform the behaviour.</obo:IAO_0000115>
        <rdfs:label>persuade about personal capability BCT</rdfs:label>
    </owl:Class>
    


    <!-- http://humanbehaviourchange.org/ontology/BCIO_007138 -->

    <owl:Class rdf:about="http://humanbehaviourchange.org/ontology/BCIO_007138">
        <rdfs:subClassOf rdf:resource="http://humanbehaviourchange.org/ontology/BCIO_007239"/>
        <obo:IAO_0000114>Published</obo:IAO_0000114>
        <obo:IAO_0000115>A prompt thinking related to successful performance BCT that prompts the person to practise imagining performing the behaviour well in a relevant context.</obo:IAO_0000115>
        <rdfs:label>prompt mental rehearsal of successful performance BCT</rdfs:label>
    </owl:Class>
    


    <!-- http://humanbehaviourchange.org/ontology/BCIO_007139 -->

    <owl:Class rdf:about="http://humanbehaviourchange.org/ontology/BCIO_007139">
        <rdfs:subClassOf rdf:resource="http://humanbehaviourchange.org/ontology/BCIO_007239"/>
        <obo:IAO_0000114>Published</obo:IAO_0000114>
        <obo:IAO_0000115>A prompt thinking related to successful performance BCT that prompts the person to think about previous successful performance of the behaviour.</obo:IAO_0000115>
        <rdfs:label>prompt focus on past success BCT</rdfs:label>
    </owl:Class>
    


    <!-- http://humanbehaviourchange.org/ontology/BCIO_007140 -->

    <owl:Class rdf:about="http://humanbehaviourchange.org/ontology/BCIO_007140">
        <rdfs:subClassOf rdf:resource="http://humanbehaviourchange.org/ontology/BCIO_007239"/>
        <obo:IAO_0000114>Published</obo:IAO_0000114>
        <obo:IAO_0000115>A prompt thinking related to successful performance BCT that promotes the use of positive self-talk before or during the behaviour.</obo:IAO_0000115>
        <rdfs:comment>Self-talk could be about the behaviour or the context of the behaviour. Self-talk does not need to be spoken aloud</rdfs:comment>
        <rdfs:label>prompt self-talk BCT</rdfs:label>
    </owl:Class>
    


    <!-- http://humanbehaviourchange.org/ontology/BCIO_007141 -->

    <owl:Class rdf:about="http://humanbehaviourchange.org/ontology/BCIO_007141">
        <rdfs:subClassOf rdf:resource="http://humanbehaviourchange.org/ontology/BCIO_007001"/>
        <obo:IAO_0000114>Published</obo:IAO_0000114>
        <obo:IAO_0000115>A goal directed BCT that advises the person to find ways to remind themselves of their behavioural goal.</obo:IAO_0000115>
        <rdfs:label>advise to keep behaviour goal in mind BCT</rdfs:label>
    </owl:Class>
    


    <!-- http://humanbehaviourchange.org/ontology/BCIO_007142 -->

    <owl:Class rdf:about="http://humanbehaviourchange.org/ontology/BCIO_007142">
        <rdfs:subClassOf rdf:resource="http://humanbehaviourchange.org/ontology/BCIO_007001"/>
        <obo:IAO_0000114>Published</obo:IAO_0000114>
        <obo:IAO_0000115>A goal directed BCT that advises the person to find ways to remind themselves of their goal in terms of a desired outcome of performing the behaviour.</obo:IAO_0000115>
        <rdfs:label>advise to keep outcome goal in mind BCT</rdfs:label>
    </owl:Class>
    


    <!-- http://humanbehaviourchange.org/ontology/BCIO_007143 -->

    <owl:Class rdf:about="http://humanbehaviourchange.org/ontology/BCIO_007143">
        <rdfs:subClassOf rdf:resource="http://humanbehaviourchange.org/ontology/BCIO_007185"/>
        <obo:IAO_0000112> Training on the stop signal task</obo:IAO_0000112>
        <obo:IAO_0000112>Practising the Go/No-Go task</obo:IAO_0000112>
        <obo:IAO_0000114>Published</obo:IAO_0000114>
        <obo:IAO_0000115>A manage mental processes BCT that promotes a task that trains the person to control automatic responses.</obo:IAO_0000115>
        <rdfs:comment>Automatic responses can include impulses, habits or emotions that lead to the unwanted behaviour.</rdfs:comment>
        <rdfs:label>enable person to manage automatic responses BCT</rdfs:label>
    </owl:Class>
    


    <!-- http://humanbehaviourchange.org/ontology/BCIO_007144 -->

    <owl:Class rdf:about="http://humanbehaviourchange.org/ontology/BCIO_007144">
        <rdfs:subClassOf rdf:resource="http://humanbehaviourchange.org/ontology/BCIO_033000"/>
        <obo:IAO_0000114>Published</obo:IAO_0000114>
        <obo:IAO_0000115>A behaviour change technique promoting medicines or other drugs.</obo:IAO_0000115>
        <rdfs:comment>If pharmacological support to reduce negative emotions (i.e. anxiety) then also code &apos;advise how to reduce negative emotions BCT&apos;</rdfs:comment>
        <rdfs:label>promote pharmacological support BCT</rdfs:label>
    </owl:Class>
    


    <!-- http://humanbehaviourchange.org/ontology/BCIO_007145 -->

    <owl:Class rdf:about="http://humanbehaviourchange.org/ontology/BCIO_007145">
        <rdfs:subClassOf rdf:resource="http://humanbehaviourchange.org/ontology/BCIO_007144"/>
        <obo:IAO_0000114>Published</obo:IAO_0000114>
        <obo:IAO_0000115>A promote pharmacological support BCT that provides the person with medicines or other drugs.</obo:IAO_0000115>
        <rdfs:label>provide pharmacological support BCT</rdfs:label>
    </owl:Class>
    


    <!-- http://humanbehaviourchange.org/ontology/BCIO_007146 -->

    <owl:Class rdf:about="http://humanbehaviourchange.org/ontology/BCIO_007146">
        <rdfs:subClassOf rdf:resource="http://humanbehaviourchange.org/ontology/BCIO_007144"/>
        <obo:IAO_0000114>Published</obo:IAO_0000114>
        <obo:IAO_0000115>A promote pharmacological support BCT that encourages the person to use medicines or other drugs.</obo:IAO_0000115>
        <rdfs:label>encourage pharmacological support BCT</rdfs:label>
    </owl:Class>
    


    <!-- http://humanbehaviourchange.org/ontology/BCIO_007147 -->

    <owl:Class rdf:about="http://humanbehaviourchange.org/ontology/BCIO_007147">
        <rdfs:subClassOf rdf:resource="http://humanbehaviourchange.org/ontology/BCIO_033000"/>
        <obo:IAO_0000114>Published</obo:IAO_0000114>
        <obo:IAO_0000115>A behaviour change technique that suggests a method to alter emotions.</obo:IAO_0000115>
        <rdfs:comment>This is a broad category. It can include both advising people on ways to change emotions and directly intervening to change emotions.</rdfs:comment>
        <rdfs:label>advise how to change emotions BCT</rdfs:label>
    </owl:Class>
    


    <!-- http://humanbehaviourchange.org/ontology/BCIO_007150 -->

    <owl:Class rdf:about="http://humanbehaviourchange.org/ontology/BCIO_007150">
        <rdfs:subClassOf rdf:resource="http://humanbehaviourchange.org/ontology/BCIO_033000"/>
        <obo:IAO_0000114>Published</obo:IAO_0000114>
        <obo:IAO_0000115>A behaviour change technique that alters the environment in which the behaviour is, or would have been, performed in a way that facilitates or impedes the behaviour.</obo:IAO_0000115>
        <rdfs:label>restructure the environment BCT</rdfs:label>
    </owl:Class>
    


    <!-- http://humanbehaviourchange.org/ontology/BCIO_007151 -->

    <owl:Class rdf:about="http://humanbehaviourchange.org/ontology/BCIO_007151">
        <rdfs:subClassOf rdf:resource="http://humanbehaviourchange.org/ontology/BCIO_050348"/>
        <obo:IAO_0000112>Example 1: Changing meal portion size to reduce the amount people eat at a sitting.
Example 2: Removing unhealthy snacks from the till area in supermarkets to reduce impulse buying of these items.
Example 3: Organisation wide use of ‘red time’ notices that people can put on their door or desk to signal that they are not to be interrupted in order to increase productivity.</obo:IAO_0000112>
        <obo:IAO_0000114>Published</obo:IAO_0000114>
        <obo:IAO_0000115>A restructure the physical environment BCT that changes the person’s directly experienced environment at the time the behaviour is, or would have been, performed.</obo:IAO_0000115>
        <rdfs:label>directly restructure the physical environment BCT</rdfs:label>
    </owl:Class>
    


    <!-- http://humanbehaviourchange.org/ontology/BCIO_007152 -->

    <owl:Class rdf:about="http://humanbehaviourchange.org/ontology/BCIO_007152">
        <rdfs:subClassOf rdf:resource="http://humanbehaviourchange.org/ontology/BCIO_050348"/>
        <obo:IAO_0000112>Example 1: Putting cigarette packs out of sight in shops in order to promote smoking cessation or reduce smoking uptake
Example 2: Introducing safe cycle routes in residential neighbourhood to increase frequency of initiating journeys from home by bicycle.</obo:IAO_0000112>
        <obo:IAO_0000114>Published</obo:IAO_0000114>
        <obo:IAO_0000115>A restructure the physical environment BCT that changes the person&apos;s environment at a time or location other than when and where the behaviour is performed.</obo:IAO_0000115>
        <rdfs:label>indirectly restructure the physical environment BCT</rdfs:label>
    </owl:Class>
    


    <!-- http://humanbehaviourchange.org/ontology/BCIO_007153 -->

    <owl:Class rdf:about="http://humanbehaviourchange.org/ontology/BCIO_007153">
        <rdfs:subClassOf rdf:resource="http://humanbehaviourchange.org/ontology/BCIO_007079"/>
        <obo:IAO_0000114>Published</obo:IAO_0000114>
        <obo:IAO_0000115>An alter external stimulus BCT that reduces an external stimulus that signals the behaviour.</obo:IAO_0000115>
        <rdfs:comment>The reduction in exposure can be gradual, as in the technique of &quot;fading&quot; or not so gradual. This BCT is concerned with reducing the person&apos;s exposure to the cue, while the cue frequency may remain unchanged. In contrast, &quot;reduce cue frequency BCT&quot; is concerned with a reduction in the number of times with which the cue is presented. This BCT may also involve &apos;restructure the physical environment BCT&apos; and/or &apos;restructure the social environment BCT&apos;.</rdfs:comment>
        <rdfs:label>reduce exposure to cues for the behaviour BCT</rdfs:label>
    </owl:Class>
    


    <!-- http://humanbehaviourchange.org/ontology/BCIO_007154 -->

    <owl:Class rdf:about="http://humanbehaviourchange.org/ontology/BCIO_007154">
        <rdfs:subClassOf rdf:resource="http://humanbehaviourchange.org/ontology/BCIO_007185"/>
        <obo:IAO_0000114>Published</obo:IAO_0000114>
        <obo:IAO_0000115>An manage mental processes BCT that advises the person to find an alternative focus for attention in order to avoid internal or external states or events associated with an unwanted behaviour.</obo:IAO_0000115>
        <obo:IAO_0000118>attention shift</obo:IAO_0000118>
        <rdfs:label>advise distraction BCT</rdfs:label>
    </owl:Class>
    


    <!-- http://humanbehaviourchange.org/ontology/BCIO_007155 -->

    <owl:Class rdf:about="http://humanbehaviourchange.org/ontology/BCIO_007155">
        <rdfs:subClassOf rdf:resource="http://humanbehaviourchange.org/ontology/BCIO_050348"/>
        <obo:IAO_0000114>Published</obo:IAO_0000114>
        <obo:IAO_0000115>A restructure the physical environment BCT that organises an alternative focus for attention for the person to avoid internal or external states or events associated with an unwanted behaviour.</obo:IAO_0000115>
        <obo:IAO_0000118>attention shift</obo:IAO_0000118>
        <rdfs:label>provide distraction BCT</rdfs:label>
    </owl:Class>
    


    <!-- http://humanbehaviourchange.org/ontology/BCIO_007156 -->

    <owl:Class rdf:about="http://humanbehaviourchange.org/ontology/BCIO_007156">
        <rdfs:subClassOf rdf:resource="http://humanbehaviourchange.org/ontology/BCIO_050348"/>
        <obo:IAO_0000114>Published</obo:IAO_0000114>
        <obo:IAO_0000115>A restructure the physical environment BCT that adds objects to the person&apos;s physical surroundings.</obo:IAO_0000115>
        <rdfs:comment>Provision of information (e.g. written, verbal, visual) in a booklet or leaflet is insufficient. If this is accompanied by social support, also code &apos;social support BCT&apos; or one of its child classes. If the environment is changed beyond the addition of objects, also code &apos;directly restructure the physical environment BCT&apos; and/or &apos;indirectly restructure the physical environment BCT&apos;.</rdfs:comment>
        <rdfs:label>add objects to the environment BCT</rdfs:label>
    </owl:Class>
    


    <!-- http://humanbehaviourchange.org/ontology/BCIO_007157 -->

    <owl:Class rdf:about="http://humanbehaviourchange.org/ontology/BCIO_007157">
        <rdfs:subClassOf rdf:resource="http://humanbehaviourchange.org/ontology/BCIO_033000"/>
        <obo:IAO_0000114>Published</obo:IAO_0000114>
        <obo:IAO_0000115>A behaviour change technique that prompts the person to focus on their mental representation of themself.</obo:IAO_0000115>
        <obo:IAO_0000118>self-perception</obo:IAO_0000118>
        <rdfs:label>prompt focus on self-identity BCT</rdfs:label>
    </owl:Class>
    


    <!-- http://humanbehaviourchange.org/ontology/BCIO_007158 -->

    <owl:Class rdf:about="http://humanbehaviourchange.org/ontology/BCIO_007158">
        <rdfs:subClassOf rdf:resource="http://humanbehaviourchange.org/ontology/BCIO_007157"/>
        <obo:IAO_0000114>Published</obo:IAO_0000114>
        <obo:IAO_0000115>A prompt focus on self-identity BCT that informs the person that their behaviour may be an example to others.</obo:IAO_0000115>
        <rdfs:label>identify self as role model BCT</rdfs:label>
    </owl:Class>
    


    <!-- http://humanbehaviourchange.org/ontology/BCIO_007159 -->

    <owl:Class rdf:about="http://humanbehaviourchange.org/ontology/BCIO_007159">
        <rdfs:subClassOf rdf:resource="http://humanbehaviourchange.org/ontology/BCIO_007157"/>
        <obo:IAO_0000114>Published</obo:IAO_0000114>
        <obo:IAO_0000115>A prompt focus on self-identity BCT that advises engagement in activities that affirm the person&apos;s valued attributes.</obo:IAO_0000115>
        <obo:IAO_0000118>self-affirmation, personal affirmation</obo:IAO_0000118>
        <rdfs:label>affirm valued self-identity BCT</rdfs:label>
    </owl:Class>
    


    <!-- http://humanbehaviourchange.org/ontology/BCIO_007160 -->

    <owl:Class rdf:about="http://humanbehaviourchange.org/ontology/BCIO_007160">
        <rdfs:subClassOf rdf:resource="http://humanbehaviourchange.org/ontology/BCIO_007157"/>
        <obo:IAO_0000114>Published</obo:IAO_0000114>
        <obo:IAO_0000115>A prompt focus on self-identity BCT that promotes the adoption of a self-identity as someone who engages in the behaviour that is different from their previous behaviour.</obo:IAO_0000115>
        <rdfs:label>adopt changed self-identity BCT</rdfs:label>
    </owl:Class>
    


    <!-- http://humanbehaviourchange.org/ontology/BCIO_007161 -->

    <owl:Class rdf:about="http://humanbehaviourchange.org/ontology/BCIO_007161">
        <rdfs:subClassOf rdf:resource="http://humanbehaviourchange.org/ontology/BCIO_007157"/>
        <obo:IAO_0000114>Published</obo:IAO_0000114>
        <obo:IAO_0000115>A prompt focus on self-identity BCT that promotes the adoption of a positive self-identity as someone who currently engages in the behaviour.</obo:IAO_0000115>
        <rdfs:label>adopt positive self-identity BCT</rdfs:label>
    </owl:Class>
    


    <!-- http://humanbehaviourchange.org/ontology/BCIO_007163 -->

    <owl:Class rdf:about="http://humanbehaviourchange.org/ontology/BCIO_007163">
        <rdfs:subClassOf rdf:resource="http://humanbehaviourchange.org/ontology/BCIO_007156"/>
        <obo:IAO_0000114>Published</obo:IAO_0000114>
        <obo:IAO_0000115>An add objects to the environment BCT that adds an object to the person’s directly experienced environment at the time the behaviour is, or would have been, performed.</obo:IAO_0000115>
        <rdfs:label>add objects to the directly experienced environment BCT</rdfs:label>
    </owl:Class>
    


    <!-- http://humanbehaviourchange.org/ontology/BCIO_007164 -->

    <owl:Class rdf:about="http://humanbehaviourchange.org/ontology/BCIO_007164">
        <rdfs:subClassOf rdf:resource="http://humanbehaviourchange.org/ontology/BCIO_007156"/>
        <obo:IAO_0000114>Published</obo:IAO_0000114>
        <obo:IAO_0000115>An add objects to the environment BCT that adds an object to the person’s environment at a time or location other than when and where the behaviour is performed.</obo:IAO_0000115>
        <rdfs:label>add objects to the indirectly experienced environment BCT</rdfs:label>
    </owl:Class>
    


    <!-- http://humanbehaviourchange.org/ontology/BCIO_007165 -->

    <owl:Class rdf:about="http://humanbehaviourchange.org/ontology/BCIO_007165">
        <rdfs:subClassOf rdf:resource="http://humanbehaviourchange.org/ontology/BCIO_007147"/>
        <obo:IAO_0000114>Published</obo:IAO_0000114>
        <obo:IAO_0000115>An advise how to change emotions BCT that suggests the person perform a particular behaviour to change an emotion.</obo:IAO_0000115>
        <obo:IAO_0000118>behavioural activation in cognitive-behavioural therapy</obo:IAO_0000118>
        <rdfs:label>advise behavioural ways to change emotions BCT</rdfs:label>
    </owl:Class>
    


    <!-- http://humanbehaviourchange.org/ontology/BCIO_007166 -->

    <owl:Class rdf:about="http://humanbehaviourchange.org/ontology/BCIO_007166">
        <rdfs:subClassOf rdf:resource="http://humanbehaviourchange.org/ontology/BCIO_007147"/>
        <obo:IAO_0000114>Published</obo:IAO_0000114>
        <obo:IAO_0000115>An advise how to change emotions BCT that suggests the person deliberately use a particular mental process.</obo:IAO_0000115>
        <rdfs:comment>The target of the mental process advised by this BCT will be an emotion. If a BCT suggests adopting a different cognitive perspective on behaviour, which then changes emotions, use &quot;suggest different perspective on behaviour BCT&quot; or one of its child classes. A mental process is something that occurs in the brain, and that can of itself be conscious, or can give rise to a process that can of itself be conscious or can give rise to behaviour.</rdfs:comment>
        <rdfs:label>advise cognitive ways to change emotions BCT</rdfs:label>
    </owl:Class>
    


    <!-- http://humanbehaviourchange.org/ontology/BCIO_007167 -->

    <owl:Class rdf:about="http://humanbehaviourchange.org/ontology/BCIO_007167">
        <rdfs:subClassOf rdf:resource="http://humanbehaviourchange.org/ontology/BCIO_007147"/>
        <obo:IAO_0000114>Published</obo:IAO_0000114>
        <obo:IAO_0000115>An advise how to change emotions BCT that suggests the person use a method that stimulates one or more senses.</obo:IAO_0000115>
        <rdfs:comment> advise to use aromatherapy to reduce stress</rdfs:comment>
        <rdfs:comment>advise to listen to up-tempo music to increase happiness</rdfs:comment>
        <rdfs:label>advise sensory ways to change emotions BCT</rdfs:label>
    </owl:Class>
    


    <!-- http://humanbehaviourchange.org/ontology/BCIO_007168 -->

    <owl:Class rdf:about="http://humanbehaviourchange.org/ontology/BCIO_007168">
        <rdfs:subClassOf rdf:resource="http://humanbehaviourchange.org/ontology/BCIO_033000"/>
        <obo:IAO_0000114>Published</obo:IAO_0000114>
        <obo:IAO_0000115>A behaviour change technique that advises the person to perform a behaviour in a particular way to help change the target behaviour.</obo:IAO_0000115>
        <rdfs:comment>In this BCT, the behaviour the person is advised to perform may not necessarily be the target behaviour, but performing the advised behaviour is thought to help change the targeted behaviour.</rdfs:comment>
        <rdfs:label>advise specific behaviour BCT</rdfs:label>
    </owl:Class>
    


    <!-- http://humanbehaviourchange.org/ontology/BCIO_007169 -->

    <owl:Class rdf:about="http://humanbehaviourchange.org/ontology/BCIO_007169">
        <rdfs:subClassOf rdf:resource="http://humanbehaviourchange.org/ontology/BCIO_007168"/>
        <obo:IAO_0000114>Published</obo:IAO_0000114>
        <obo:IAO_0000115>An advise specific behaviour BCT that advises the person to refrain from engaging in the behaviour in a specified context.</obo:IAO_0000115>
        <rdfs:comment>For the purposes of this BCT, preceding behaviour can be considered part of the context</rdfs:comment>
        <rdfs:label>context-specific non-enactment of behaviour BCT</rdfs:label>
    </owl:Class>
    


    <!-- http://humanbehaviourchange.org/ontology/BCIO_007170 -->

    <owl:Class rdf:about="http://humanbehaviourchange.org/ontology/BCIO_007170">
        <rdfs:subClassOf rdf:resource="http://humanbehaviourchange.org/ontology/BCIO_007085"/>
        <obo:IAO_0000114>Published</obo:IAO_0000114>
        <obo:IAO_0000115>An expose to stimulus BCT that involves sustained exposure to an aversive stimulus to reduce the likelihood of the behaviour when encountering that stimulus.</obo:IAO_0000115>
        <obo:IAO_0000118>flooding</obo:IAO_0000118>
        <rdfs:label>expose to sustained aversive stimulus BCT</rdfs:label>
    </owl:Class>
    


    <!-- http://humanbehaviourchange.org/ontology/BCIO_007171 -->

    <owl:Class rdf:about="http://humanbehaviourchange.org/ontology/BCIO_007171">
        <rdfs:subClassOf rdf:resource="http://humanbehaviourchange.org/ontology/BCIO_007001"/>
        <obo:IAO_0000114>Published</obo:IAO_0000114>
        <obo:IAO_0000115>A goal directed BCT that enables the person to engage in an alternative rewarding behaviour that increases the likelihood of goal achievement.</obo:IAO_0000115>
        <rdfs:label>facilitate alternative goal-directed activity BCT</rdfs:label>
    </owl:Class>
    


    <!-- http://humanbehaviourchange.org/ontology/BCIO_007172 -->

    <owl:Class rdf:about="http://humanbehaviourchange.org/ontology/BCIO_007172">
        <rdfs:subClassOf rdf:resource="http://humanbehaviourchange.org/ontology/BCIO_007085"/>
        <obo:IAO_0000114>Published</obo:IAO_0000114>
        <obo:IAO_0000115>An expose to stimulus BCT that involves gradually increasing exposure to an aversive stimulus to reduce the likelihood of the behaviour when encountering that stimulus.</obo:IAO_0000115>
        <obo:IAO_0000118>graded exposure</obo:IAO_0000118>
        <rdfs:label>gradually increase exposure to aversive stimulus BCT</rdfs:label>
    </owl:Class>
    


    <!-- http://humanbehaviourchange.org/ontology/BCIO_007173 -->

    <owl:Class rdf:about="http://humanbehaviourchange.org/ontology/BCIO_007173">
        <rdfs:subClassOf rdf:resource="http://humanbehaviourchange.org/ontology/BCIO_033000"/>
        <obo:IAO_0000114>Published</obo:IAO_0000114>
        <obo:IAO_0000115>A behaviour change technique that draws attention to the behaviour.</obo:IAO_0000115>
        <rdfs:comment>This class concerns raising awareness of the behaviour itself.  Where a BCT increases awareness of the consequences of behaviour, rather than the behaviour itself, use &quot;increase awareness of consequences BCT&quot; or one of its child classes</rdfs:comment>
        <rdfs:label>increase awareness of behaviour BCT</rdfs:label>
    </owl:Class>
    


    <!-- http://humanbehaviourchange.org/ontology/BCIO_007174 -->

    <owl:Class rdf:about="http://humanbehaviourchange.org/ontology/BCIO_007174">
        <rdfs:subClassOf rdf:resource="http://humanbehaviourchange.org/ontology/BCIO_007173"/>
        <obo:IAO_0000114>Published</obo:IAO_0000114>
        <obo:IAO_0000115>An increase awareness of behaviour BCT that draws attention to the possibility of performing a novel behaviour.</obo:IAO_0000115>
        <rdfs:comment>This class concerns raising awareness of a novel behaviour that one might not have known was an option. If not a novel behaviour, consider &quot;suggest how to perform behaviour BCT&quot;.</rdfs:comment>
        <rdfs:label>increase awareness of option of novel behaviour BCT</rdfs:label>
    </owl:Class>
    


    <!-- http://humanbehaviourchange.org/ontology/BCIO_007175 -->

    <owl:Class rdf:about="http://humanbehaviourchange.org/ontology/BCIO_007175">
        <rdfs:subClassOf rdf:resource="http://humanbehaviourchange.org/ontology/BCIO_007173"/>
        <obo:IAO_0000112>Mask use at the start of the Covid pandemic through symbols/signs of masks in public spaces</obo:IAO_0000112>
        <obo:IAO_0000114>Published</obo:IAO_0000114>
        <obo:IAO_0000115>An increase awareness of behaviour BCT that makes the possibility of performing the behaviour more distinctive or prominent.</obo:IAO_0000115>
        <obo:IAO_0000118>salience of behaviour</obo:IAO_0000118>
        <rdfs:label>increase salience of behaviour BCT</rdfs:label>
    </owl:Class>
    


    <!-- http://humanbehaviourchange.org/ontology/BCIO_007176 -->

    <owl:Class rdf:about="http://humanbehaviourchange.org/ontology/BCIO_007176">
        <rdfs:subClassOf rdf:resource="http://humanbehaviourchange.org/ontology/BCIO_007062"/>
        <obo:IAO_0000114>Published</obo:IAO_0000114>
        <obo:IAO_0000115>An increase awareness of consequences BCT that provides information about the environmental consequences of performing or not performing the behaviour.</obo:IAO_0000115>
        <obo:IAO_0000118>environmental effects, ecological impacts</obo:IAO_0000118>
        <rdfs:comment> emphasising importance of consequences is not sufficient.</rdfs:comment>
        <rdfs:comment>Consequences can be for any target, not just the recipient(s) of the intervention</rdfs:comment>
        <rdfs:label>inform about environmental consequences BCT</rdfs:label>
    </owl:Class>
    


    <!-- http://humanbehaviourchange.org/ontology/BCIO_007177 -->

    <owl:Class rdf:about="http://humanbehaviourchange.org/ontology/BCIO_007177">
        <rdfs:subClassOf rdf:resource="http://humanbehaviourchange.org/ontology/BCIO_007065"/>
        <obo:IAO_0000114>Published</obo:IAO_0000114>
        <obo:IAO_0000115>An inform about emotional consequences BCT that provides information about the negative emotional consequences of performing or not performing the behaviour.</obo:IAO_0000115>
        <rdfs:label>inform about negative emotional consequences BCT</rdfs:label>
    </owl:Class>
    


    <!-- http://humanbehaviourchange.org/ontology/BCIO_007178 -->

    <owl:Class rdf:about="http://humanbehaviourchange.org/ontology/BCIO_007178">
        <rdfs:subClassOf rdf:resource="http://humanbehaviourchange.org/ontology/BCIO_007176"/>
        <obo:IAO_0000114>Published</obo:IAO_0000114>
        <obo:IAO_0000115>An inform about environmental consequences BCT that provides information about the negative environmental consequences of performing or not performing the behaviour.</obo:IAO_0000115>
        <rdfs:label>inform about negative environmental consequences BCT</rdfs:label>
    </owl:Class>
    


    <!-- http://humanbehaviourchange.org/ontology/BCIO_007179 -->

    <owl:Class rdf:about="http://humanbehaviourchange.org/ontology/BCIO_007179">
        <rdfs:subClassOf rdf:resource="http://humanbehaviourchange.org/ontology/BCIO_007063"/>
        <obo:IAO_0000114>Published</obo:IAO_0000114>
        <obo:IAO_0000115>An inform about health consequences BCT that provides information about the negative physical or mental health consequences of performing or not performing the behaviour.</obo:IAO_0000115>
        <rdfs:label>inform about negative health consequences BCT</rdfs:label>
    </owl:Class>
    


    <!-- http://humanbehaviourchange.org/ontology/BCIO_007180 -->

    <owl:Class rdf:about="http://humanbehaviourchange.org/ontology/BCIO_007180">
        <rdfs:subClassOf rdf:resource="http://humanbehaviourchange.org/ontology/BCIO_007064"/>
        <obo:IAO_0000114>Published</obo:IAO_0000114>
        <obo:IAO_0000115>An inform about social consequences BCT that provides information about the negative social consequences of performing or not performing the behaviour.</obo:IAO_0000115>
        <rdfs:label>inform about negative social consequences BCT</rdfs:label>
    </owl:Class>
    


    <!-- http://humanbehaviourchange.org/ontology/BCIO_007181 -->

    <owl:Class rdf:about="http://humanbehaviourchange.org/ontology/BCIO_007181">
        <rdfs:subClassOf rdf:resource="http://humanbehaviourchange.org/ontology/BCIO_007065"/>
        <obo:IAO_0000114>Published</obo:IAO_0000114>
        <obo:IAO_0000115>An inform about emotional consequences BCT that provides information about the positive emotional consequences of performing or not performing the behaviour.</obo:IAO_0000115>
        <rdfs:label>inform about positive emotional consequences BCT</rdfs:label>
    </owl:Class>
    


    <!-- http://humanbehaviourchange.org/ontology/BCIO_007182 -->

    <owl:Class rdf:about="http://humanbehaviourchange.org/ontology/BCIO_007182">
        <rdfs:subClassOf rdf:resource="http://humanbehaviourchange.org/ontology/BCIO_007176"/>
        <obo:IAO_0000114>Published</obo:IAO_0000114>
        <obo:IAO_0000115>An inform about environmental consequences BCT that provides information about the positive environmental consequences of performing or not performing the behaviour.</obo:IAO_0000115>
        <rdfs:label>inform about positive environmental consequences BCT</rdfs:label>
    </owl:Class>
    


    <!-- http://humanbehaviourchange.org/ontology/BCIO_007183 -->

    <owl:Class rdf:about="http://humanbehaviourchange.org/ontology/BCIO_007183">
        <rdfs:subClassOf rdf:resource="http://humanbehaviourchange.org/ontology/BCIO_007063"/>
        <obo:IAO_0000114>Published</obo:IAO_0000114>
        <obo:IAO_0000115>An inform about health consequences BCT that provides information about the positive physical or mental health consequences of performing or not performing the behaviour.</obo:IAO_0000115>
        <rdfs:label>inform about positive health consequences BCT</rdfs:label>
    </owl:Class>
    


    <!-- http://humanbehaviourchange.org/ontology/BCIO_007184 -->

    <owl:Class rdf:about="http://humanbehaviourchange.org/ontology/BCIO_007184">
        <rdfs:subClassOf rdf:resource="http://humanbehaviourchange.org/ontology/BCIO_007064"/>
        <obo:IAO_0000114>Published</obo:IAO_0000114>
        <obo:IAO_0000115>An inform about social consequences BCT that provides information about the positive social consequences of performing or not performing the behaviour.</obo:IAO_0000115>
        <rdfs:label>inform about positive social consequences BCT</rdfs:label>
    </owl:Class>
    


    <!-- http://humanbehaviourchange.org/ontology/BCIO_007185 -->

    <owl:Class rdf:about="http://humanbehaviourchange.org/ontology/BCIO_007185">
        <rdfs:subClassOf rdf:resource="http://humanbehaviourchange.org/ontology/BCIO_033000"/>
        <obo:IAO_0000114>Published</obo:IAO_0000114>
        <obo:IAO_0000115>A behaviour change technique that advises how to manage mental processes to facilitate the behaviour.</obo:IAO_0000115>
        <rdfs:comment>A mental process is something that occurs in the brain, and that can of itself be conscious, or can give rise to a process that can of itself be conscious or can give rise to behaviour.</rdfs:comment>
        <rdfs:label>manage mental processes BCT</rdfs:label>
    </owl:Class>
    


    <!-- http://humanbehaviourchange.org/ontology/BCIO_007186 -->

    <owl:Class rdf:about="http://humanbehaviourchange.org/ontology/BCIO_007186">
        <rdfs:subClassOf rdf:resource="http://humanbehaviourchange.org/ontology/BCIO_033000"/>
        <obo:IAO_0000114>Published</obo:IAO_0000114>
        <obo:IAO_0000115>A behaviour change technique that alters the consequences or promised consequences for an outcome that results from performing or not performing the behaviour.</obo:IAO_0000115>
        <rdfs:label>outcome consequence BCT</rdfs:label>
    </owl:Class>
    


    <!-- http://humanbehaviourchange.org/ontology/BCIO_007187 -->

    <owl:Class rdf:about="http://humanbehaviourchange.org/ontology/BCIO_007187">
        <rdfs:subClassOf rdf:resource="http://humanbehaviourchange.org/ontology/BCIO_007101"/>
        <obo:IAO_0000114>Published</obo:IAO_0000114>
        <obo:IAO_0000115>A behavioural consequence BCT that promises a future consequence contingent on performing or not performing the behaviour.</obo:IAO_0000115>
        <rdfs:comment>&quot;promises&quot; here means assuring someone that one will do something or that something will happen.</rdfs:comment>
        <rdfs:label>promise consequence for behaviour BCT</rdfs:label>
    </owl:Class>
    


    <!-- http://humanbehaviourchange.org/ontology/BCIO_007188 -->

    <owl:Class rdf:about="http://humanbehaviourchange.org/ontology/BCIO_007188">
        <rdfs:subClassOf rdf:resource="http://humanbehaviourchange.org/ontology/BCIO_007101"/>
        <obo:IAO_0000114>Published</obo:IAO_0000114>
        <obo:IAO_0000115>A behavioural consequence BCT that promises future removal of a consequence contingent on performing or not performing the behaviour.</obo:IAO_0000115>
        <rdfs:label>promise to remove consequence for behaviour BCT</rdfs:label>
    </owl:Class>
    


    <!-- http://humanbehaviourchange.org/ontology/BCIO_007189 -->

    <owl:Class rdf:about="http://humanbehaviourchange.org/ontology/BCIO_007189">
        <rdfs:subClassOf rdf:resource="http://humanbehaviourchange.org/ontology/BCIO_007187"/>
        <obo:IAO_0000114>Published</obo:IAO_0000114>
        <obo:IAO_0000115>A promise consequence for behaviour BCT where the consequence is aversive.</obo:IAO_0000115>
        <obo:IAO_0000118>threat, warning, disincentive</obo:IAO_0000118>
        <rdfs:comment>To qualify as aversive, the consequence should be aversively valued by the person receiving it.</rdfs:comment>
        <rdfs:label>promise aversive consequence for behaviour BCT</rdfs:label>
    </owl:Class>
    


    <!-- http://humanbehaviourchange.org/ontology/BCIO_007190 -->

    <owl:Class rdf:about="http://humanbehaviourchange.org/ontology/BCIO_007190">
        <rdfs:subClassOf rdf:resource="http://humanbehaviourchange.org/ontology/BCIO_007188"/>
        <obo:IAO_0000114>Published</obo:IAO_0000114>
        <obo:IAO_0000115>A promise to remove consequence for behaviour BCT where the consequence is aversive.</obo:IAO_0000115>
        <obo:IAO_0000118>incentive to remove punishment</obo:IAO_0000118>
        <rdfs:label>promise to remove aversive consequence for behaviour BCT</rdfs:label>
    </owl:Class>
    


    <!-- http://humanbehaviourchange.org/ontology/BCIO_007191 -->

    <owl:Class rdf:about="http://humanbehaviourchange.org/ontology/BCIO_007191">
        <rdfs:subClassOf rdf:resource="http://humanbehaviourchange.org/ontology/BCIO_007189"/>
        <obo:IAO_0000114>Published</obo:IAO_0000114>
        <obo:IAO_0000115>A promise aversive consequence for behaviour BCT that promises the consequence will be provided for the behaviour in one situation but not in another.</obo:IAO_0000115>
        <obo:IAO_0000118>threat for situation specific behaviour</obo:IAO_0000118>
        <rdfs:label>promise aversive consequence for situation specific behaviour BCT</rdfs:label>
    </owl:Class>
    


    <!-- http://humanbehaviourchange.org/ontology/BCIO_007192 -->

    <owl:Class rdf:about="http://humanbehaviourchange.org/ontology/BCIO_007192">
        <rdfs:subClassOf rdf:resource="http://humanbehaviourchange.org/ontology/BCIO_007189"/>
        <obo:IAO_0000114>Published</obo:IAO_0000114>
        <obo:IAO_0000115>A promise aversive consequence for behaviour BCT where the consequence is money, vouchers or other valued objects.</obo:IAO_0000115>
        <obo:IAO_0000118>material threat</obo:IAO_0000118>
        <rdfs:label>promise aversive material consequence for behaviour BCT</rdfs:label>
    </owl:Class>
    


    <!-- http://humanbehaviourchange.org/ontology/BCIO_007193 -->

    <owl:Class rdf:about="http://humanbehaviourchange.org/ontology/BCIO_007193">
        <rdfs:subClassOf rdf:resource="http://humanbehaviourchange.org/ontology/BCIO_007191"/>
        <obo:IAO_0000114>Published</obo:IAO_0000114>
        <obo:IAO_0000115>A promise aversive consequence for situation specific behaviour BCT in which the consequence is money, vouchers or other valued objects.</obo:IAO_0000115>
        <obo:IAO_0000118>material threat for situation specific behaviour</obo:IAO_0000118>
        <rdfs:label>promise aversive material consequence for situation specific behaviour BCT</rdfs:label>
    </owl:Class>
    


    <!-- http://humanbehaviourchange.org/ontology/BCIO_007194 -->

    <owl:Class rdf:about="http://humanbehaviourchange.org/ontology/BCIO_007194">
        <rdfs:subClassOf rdf:resource="http://humanbehaviourchange.org/ontology/BCIO_007195"/>
        <obo:IAO_0000114>Published</obo:IAO_0000114>
        <obo:IAO_0000115>A promise aversive consequence for outcome of behaviour BCT where the consequence is money, vouchers or other valued objects.</obo:IAO_0000115>
        <rdfs:label>promise aversive material consequence for outcome of behaviour</rdfs:label>
    </owl:Class>
    


    <!-- http://humanbehaviourchange.org/ontology/BCIO_007195 -->

    <owl:Class rdf:about="http://humanbehaviourchange.org/ontology/BCIO_007195">
        <rdfs:subClassOf rdf:resource="http://humanbehaviourchange.org/ontology/BCIO_007200"/>
        <obo:IAO_0000114>Published</obo:IAO_0000114>
        <obo:IAO_0000115>A promise consequence for outcome of behaviour BCT where the consequence is aversive.</obo:IAO_0000115>
        <obo:IAO_0000118>threat, warning, disincentive</obo:IAO_0000118>
        <rdfs:label>promise aversive consequence for outcome of behaviour BCT</rdfs:label>
    </owl:Class>
    


    <!-- http://humanbehaviourchange.org/ontology/BCIO_007196 -->

    <owl:Class rdf:about="http://humanbehaviourchange.org/ontology/BCIO_007196">
        <rdfs:subClassOf rdf:resource="http://humanbehaviourchange.org/ontology/BCIO_007201"/>
        <obo:IAO_0000114>Published</obo:IAO_0000114>
        <obo:IAO_0000115>A promise to remove consequence for outcome of behaviour BCT where the consequence is aversive.</obo:IAO_0000115>
        <obo:IAO_0000118>incentive to remove punishment</obo:IAO_0000118>
        <rdfs:label>promise to remove aversive consequence for outcome of behaviour BCT</rdfs:label>
    </owl:Class>
    


    <!-- http://humanbehaviourchange.org/ontology/BCIO_007197 -->

    <owl:Class rdf:about="http://humanbehaviourchange.org/ontology/BCIO_007197">
        <rdfs:subClassOf rdf:resource="http://humanbehaviourchange.org/ontology/BCIO_007189"/>
        <obo:IAO_0000114>Published</obo:IAO_0000114>
        <obo:IAO_0000115>A promise aversive consequence for behaviour BCT where the consequence is an interpersonal process or a proxy interpersonal process.</obo:IAO_0000115>
        <obo:IAO_0000118>social threat</obo:IAO_0000118>
        <rdfs:comment>A proxy interpersonal process is where the person interacts with a chatbot, digital assistant, or similar computer program designed to simulate and process human communication</rdfs:comment>
        <rdfs:label>promise aversive social consequence for behaviour BCT</rdfs:label>
    </owl:Class>
    


    <!-- http://humanbehaviourchange.org/ontology/BCIO_007198 -->

    <owl:Class rdf:about="http://humanbehaviourchange.org/ontology/BCIO_007198">
        <rdfs:subClassOf rdf:resource="http://humanbehaviourchange.org/ontology/BCIO_007191"/>
        <obo:IAO_0000114>Published</obo:IAO_0000114>
        <obo:IAO_0000115>A promise aversive consequence for situation specific behaviour BCT in which the consequence is an interpersonal process or a proxy interpersonal process.</obo:IAO_0000115>
        <obo:IAO_0000118>social threat for situation specific behaviour</obo:IAO_0000118>
        <rdfs:comment>A proxy interpersonal process is where the person interacts with a chatbot, digital assistant, or similar computer program designed to simulate and process human communication</rdfs:comment>
        <rdfs:label>promise aversive social consequence for situation specific behaviour BCT</rdfs:label>
    </owl:Class>
    


    <!-- http://humanbehaviourchange.org/ontology/BCIO_007199 -->

    <owl:Class rdf:about="http://humanbehaviourchange.org/ontology/BCIO_007199">
        <rdfs:subClassOf rdf:resource="http://humanbehaviourchange.org/ontology/BCIO_007195"/>
        <obo:IAO_0000114>Published</obo:IAO_0000114>
        <obo:IAO_0000115>A promise aversive consequence for outcome of behaviour BCT where the consequence is an interpersonal process or a proxy interpersonal process.</obo:IAO_0000115>
        <rdfs:comment>A proxy interpersonal process is where the person interacts with a chatbot, digital assistant, or similar computer program designed to simulate and process human communication</rdfs:comment>
        <rdfs:label>promise aversive social consequence for outcome of behaviour BCT</rdfs:label>
    </owl:Class>
    


    <!-- http://humanbehaviourchange.org/ontology/BCIO_007200 -->

    <owl:Class rdf:about="http://humanbehaviourchange.org/ontology/BCIO_007200">
        <rdfs:subClassOf rdf:resource="http://humanbehaviourchange.org/ontology/BCIO_007186"/>
        <obo:IAO_0000114>Published</obo:IAO_0000114>
        <obo:IAO_0000115>An outcome consequence BCT that promises a future consequence contingent on an outcome of performing or not performing the behaviour.</obo:IAO_0000115>
        <rdfs:comment>&quot;promises&quot; here means assuring someone that one will do something or that something will happen.</rdfs:comment>
        <rdfs:label>promise consequence for outcome of behaviour BCT</rdfs:label>
    </owl:Class>
    


    <!-- http://humanbehaviourchange.org/ontology/BCIO_007201 -->

    <owl:Class rdf:about="http://humanbehaviourchange.org/ontology/BCIO_007201">
        <rdfs:subClassOf rdf:resource="http://humanbehaviourchange.org/ontology/BCIO_007186"/>
        <obo:IAO_0000114>Published</obo:IAO_0000114>
        <obo:IAO_0000115>An outcome consequence BCT that promises future removal of a consequence contingent on an outcome of performing or not performing the behaviour.</obo:IAO_0000115>
        <rdfs:label>promise to remove consequence for outcome of behaviour BCT</rdfs:label>
    </owl:Class>
    


    <!-- http://humanbehaviourchange.org/ontology/BCIO_007202 -->

    <owl:Class rdf:about="http://humanbehaviourchange.org/ontology/BCIO_007202">
        <rdfs:subClassOf rdf:resource="http://humanbehaviourchange.org/ontology/BCIO_007187"/>
        <obo:IAO_0000114>Published</obo:IAO_0000114>
        <obo:IAO_0000115>A promise consequence for behaviour BCT where the consequence is positive.</obo:IAO_0000115>
        <obo:IAO_0000118>incentive</obo:IAO_0000118>
        <rdfs:comment>To qualify as positive, the consequence should be positively valued by the person receiving it. If consequence is delivered, also code &apos;provide positive consequence for behaviour BCT&apos; or one of its child classes.</rdfs:comment>
        <rdfs:label>promise positive consequence for behaviour BCT</rdfs:label>
    </owl:Class>
    


    <!-- http://humanbehaviourchange.org/ontology/BCIO_007203 -->

    <owl:Class rdf:about="http://humanbehaviourchange.org/ontology/BCIO_007203">
        <rdfs:subClassOf rdf:resource="http://humanbehaviourchange.org/ontology/BCIO_007188"/>
        <obo:IAO_0000114>Published</obo:IAO_0000114>
        <obo:IAO_0000115>A promise to remove consequence for behaviour BCT where the consequence is positive.</obo:IAO_0000115>
        <obo:IAO_0000118>threaten to remove reward</obo:IAO_0000118>
        <rdfs:label>promise to remove positive consequence for behaviour BCT</rdfs:label>
    </owl:Class>
    


    <!-- http://humanbehaviourchange.org/ontology/BCIO_007204 -->

    <owl:Class rdf:about="http://humanbehaviourchange.org/ontology/BCIO_007204">
        <rdfs:subClassOf rdf:resource="http://humanbehaviourchange.org/ontology/BCIO_007202"/>
        <obo:IAO_0000114>Published</obo:IAO_0000114>
        <obo:IAO_0000115>A promise positive consequence for behaviour BCT that promises the consequence will be provided for the behaviour that is different from the unwanted behaviour.</obo:IAO_0000115>
        <obo:IAO_0000118>incentive for alternative behaviour</obo:IAO_0000118>
        <rdfs:label>promise positive consequence for alternative behaviour BCT</rdfs:label>
    </owl:Class>
    


    <!-- http://humanbehaviourchange.org/ontology/BCIO_007205 -->

    <owl:Class rdf:about="http://humanbehaviourchange.org/ontology/BCIO_007205">
        <rdfs:subClassOf rdf:resource="http://humanbehaviourchange.org/ontology/BCIO_007202"/>
        <obo:IAO_0000114>Published</obo:IAO_0000114>
        <obo:IAO_0000115>A promise positive consequence for behaviour BCT where the consequence is provided as the performance gradually gets closer to the behaviour.</obo:IAO_0000115>
        <obo:IAO_0000118>incentive for approximating behaviour</obo:IAO_0000118>
        <rdfs:label>promise positive consequence for approximating behaviour BCT</rdfs:label>
    </owl:Class>
    


    <!-- http://humanbehaviourchange.org/ontology/BCIO_007206 -->

    <owl:Class rdf:about="http://humanbehaviourchange.org/ontology/BCIO_007206">
        <rdfs:subClassOf rdf:resource="http://humanbehaviourchange.org/ontology/BCIO_007202"/>
        <obo:IAO_0000114>Published</obo:IAO_0000114>
        <obo:IAO_0000115>A promise positive consequence for behaviour BCT in which the consequence will be provided for performing the final behaviour in a sequence of behaviours, followed by adding behaviours that occur earlier in the sequence.</obo:IAO_0000115>
        <obo:IAO_0000118>incentive for completion of behavioural sequence</obo:IAO_0000118>
        <rdfs:label>promise positive consequence for completion of behavioural sequence BCT</rdfs:label>
    </owl:Class>
    


    <!-- http://humanbehaviourchange.org/ontology/BCIO_007207 -->

    <owl:Class rdf:about="http://humanbehaviourchange.org/ontology/BCIO_007207">
        <rdfs:subClassOf rdf:resource="http://humanbehaviourchange.org/ontology/BCIO_007202"/>
        <obo:IAO_0000114>Published</obo:IAO_0000114>
        <obo:IAO_0000115>A promise positive consequence for behaviour BCT that promises the consequence will be provided for the behaviour that is incompatible with the unwanted behaviour.</obo:IAO_0000115>
        <obo:IAO_0000118>incentive for incompatible behaviour</obo:IAO_0000118>
        <rdfs:label>promise positive consequence for incompatible behaviour BCT</rdfs:label>
    </owl:Class>
    


    <!-- http://humanbehaviourchange.org/ontology/BCIO_007208 -->

    <owl:Class rdf:about="http://humanbehaviourchange.org/ontology/BCIO_007208">
        <rdfs:subClassOf rdf:resource="http://humanbehaviourchange.org/ontology/BCIO_007202"/>
        <obo:IAO_0000114>Published</obo:IAO_0000114>
        <obo:IAO_0000115>A promise positive consequence for behaviour BCT that promises the consequence will be provided for the behaviour in one situation but not in another.</obo:IAO_0000115>
        <obo:IAO_0000118>incentive for situation specific behaviour</obo:IAO_0000118>
        <rdfs:label>promise positive consequence for situation specific behaviour BCT</rdfs:label>
    </owl:Class>
    


    <!-- http://humanbehaviourchange.org/ontology/BCIO_007209 -->

    <owl:Class rdf:about="http://humanbehaviourchange.org/ontology/BCIO_007209">
        <rdfs:subClassOf rdf:resource="http://humanbehaviourchange.org/ontology/BCIO_007202"/>
        <obo:IAO_0000114>Published</obo:IAO_0000114>
        <obo:IAO_0000115>A promise positive consequence for behaviour BCT where the consequence is money, vouchers or other valued objects.</obo:IAO_0000115>
        <obo:IAO_0000118>material incentive</obo:IAO_0000118>
        <rdfs:label>promise positive material consequence for behaviour BCT</rdfs:label>
    </owl:Class>
    


    <!-- http://humanbehaviourchange.org/ontology/BCIO_007210 -->

    <owl:Class rdf:about="http://humanbehaviourchange.org/ontology/BCIO_007210">
        <rdfs:subClassOf rdf:resource="http://humanbehaviourchange.org/ontology/BCIO_007204"/>
        <obo:IAO_0000114>Published</obo:IAO_0000114>
        <obo:IAO_0000115>A promise positive consequence for alternative behaviour BCT in which the consequence is money, vouchers or other valued objects.</obo:IAO_0000115>
        <obo:IAO_0000118>material incentive for alternative behaviour</obo:IAO_0000118>
        <rdfs:label>promise positive material consequence for alternative behaviour BCT</rdfs:label>
    </owl:Class>
    


    <!-- http://humanbehaviourchange.org/ontology/BCIO_007211 -->

    <owl:Class rdf:about="http://humanbehaviourchange.org/ontology/BCIO_007211">
        <rdfs:subClassOf rdf:resource="http://humanbehaviourchange.org/ontology/BCIO_007205"/>
        <obo:IAO_0000114>Published</obo:IAO_0000114>
        <obo:IAO_0000115>A promise positive consequence for approximating behaviour BCT in which the consequence is money, vouchers or other valued objects.</obo:IAO_0000115>
        <obo:IAO_0000118>material incentive for approximating behaviour</obo:IAO_0000118>
        <rdfs:label>promise positive material consequence for approximating behaviour BCT</rdfs:label>
    </owl:Class>
    


    <!-- http://humanbehaviourchange.org/ontology/BCIO_007212 -->

    <owl:Class rdf:about="http://humanbehaviourchange.org/ontology/BCIO_007212">
        <rdfs:subClassOf rdf:resource="http://humanbehaviourchange.org/ontology/BCIO_007206"/>
        <obo:IAO_0000114>Published</obo:IAO_0000114>
        <obo:IAO_0000115>A promise positive consequence for completion of behavioural sequence BCT in which the consequence is money, vouchers or other valued objects.</obo:IAO_0000115>
        <obo:IAO_0000118>material incentive for completion of behavioural sequence</obo:IAO_0000118>
        <rdfs:label>promise positive material consequence for completion of behavioural sequence BCT</rdfs:label>
    </owl:Class>
    


    <!-- http://humanbehaviourchange.org/ontology/BCIO_007213 -->

    <owl:Class rdf:about="http://humanbehaviourchange.org/ontology/BCIO_007213">
        <rdfs:subClassOf rdf:resource="http://humanbehaviourchange.org/ontology/BCIO_007207"/>
        <obo:IAO_0000114>Published</obo:IAO_0000114>
        <obo:IAO_0000115>A promise positive consequence for incompatible behaviour BCT in which the consequence is money, vouchers or other valued objects.</obo:IAO_0000115>
        <obo:IAO_0000118>material incentive for incompatible behaviour</obo:IAO_0000118>
        <rdfs:label>promise positive material consequence for incompatible behaviour BCT</rdfs:label>
    </owl:Class>
    


    <!-- http://humanbehaviourchange.org/ontology/BCIO_007214 -->

    <owl:Class rdf:about="http://humanbehaviourchange.org/ontology/BCIO_007214">
        <rdfs:subClassOf rdf:resource="http://humanbehaviourchange.org/ontology/BCIO_007208"/>
        <obo:IAO_0000114>Published</obo:IAO_0000114>
        <obo:IAO_0000115>A promise positive consequence for situation specific behaviour BCT in which the consequence is money, vouchers or other valued objects.</obo:IAO_0000115>
        <obo:IAO_0000118>material incentive for situation specific behaviour</obo:IAO_0000118>
        <rdfs:label>promise positive material consequence for situation specific behaviour BCT</rdfs:label>
    </owl:Class>
    


    <!-- http://humanbehaviourchange.org/ontology/BCIO_007215 -->

    <owl:Class rdf:about="http://humanbehaviourchange.org/ontology/BCIO_007215">
        <rdfs:subClassOf rdf:resource="http://humanbehaviourchange.org/ontology/BCIO_007216"/>
        <obo:IAO_0000114>Published</obo:IAO_0000114>
        <obo:IAO_0000115>A promise positive consequence for outcome of behaviour BCT where the consequence is money, vouchers or other valued objects.</obo:IAO_0000115>
        <rdfs:label>promise positive material consequence for outcome of behaviour BCT</rdfs:label>
    </owl:Class>
    


    <!-- http://humanbehaviourchange.org/ontology/BCIO_007216 -->

    <owl:Class rdf:about="http://humanbehaviourchange.org/ontology/BCIO_007216">
        <rdfs:subClassOf rdf:resource="http://humanbehaviourchange.org/ontology/BCIO_007200"/>
        <obo:IAO_0000114>Published</obo:IAO_0000114>
        <obo:IAO_0000115>A promise consequence for outcome of behaviour BCT where the consequence is positive</obo:IAO_0000115>
        <obo:IAO_0000118>incentive</obo:IAO_0000118>
        <rdfs:label>promise positive consequence for outcome of behaviour BCT</rdfs:label>
    </owl:Class>
    


    <!-- http://humanbehaviourchange.org/ontology/BCIO_007217 -->

    <owl:Class rdf:about="http://humanbehaviourchange.org/ontology/BCIO_007217">
        <rdfs:subClassOf rdf:resource="http://humanbehaviourchange.org/ontology/BCIO_007201"/>
        <obo:IAO_0000114>Published</obo:IAO_0000114>
        <obo:IAO_0000115>A promise to remove consequence for outcome of behaviour BCT where the consequence is positive.</obo:IAO_0000115>
        <obo:IAO_0000118>threaten to remove reward</obo:IAO_0000118>
        <rdfs:label>promise to remove positive consequence for outcome of behaviour BCT</rdfs:label>
    </owl:Class>
    


    <!-- http://humanbehaviourchange.org/ontology/BCIO_007218 -->

    <owl:Class rdf:about="http://humanbehaviourchange.org/ontology/BCIO_007218">
        <rdfs:subClassOf rdf:resource="http://humanbehaviourchange.org/ontology/BCIO_007202"/>
        <obo:IAO_0000114>Published</obo:IAO_0000114>
        <obo:IAO_0000115>A promise positive consequence for behaviour BCT where the consequence is an interpersonal process or a proxy interpersonal process.</obo:IAO_0000115>
        <obo:IAO_0000118>social incentive</obo:IAO_0000118>
        <rdfs:comment>A proxy interpersonal process is where the person interacts with a chatbot, digital assistant, or similar computer program designed to simulate and process human communication</rdfs:comment>
        <rdfs:label>promise positive social consequence for behaviour BCT</rdfs:label>
    </owl:Class>
    


    <!-- http://humanbehaviourchange.org/ontology/BCIO_007219 -->

    <owl:Class rdf:about="http://humanbehaviourchange.org/ontology/BCIO_007219">
        <rdfs:subClassOf rdf:resource="http://humanbehaviourchange.org/ontology/BCIO_007204"/>
        <obo:IAO_0000114>Published</obo:IAO_0000114>
        <obo:IAO_0000115>A promise positive consequence for alternative behaviour BCT in which the consequence is an interpersonal process or a proxy interpersonal process.</obo:IAO_0000115>
        <obo:IAO_0000118>social incentive for alternative behaviour</obo:IAO_0000118>
        <rdfs:comment>A proxy interpersonal process is where the person interacts with a chatbot, digital assistant, or similar computer program designed to simulate and process human communication</rdfs:comment>
        <rdfs:label>promise positive social consequence for alternative behaviour BCT</rdfs:label>
    </owl:Class>
    


    <!-- http://humanbehaviourchange.org/ontology/BCIO_007220 -->

    <owl:Class rdf:about="http://humanbehaviourchange.org/ontology/BCIO_007220">
        <rdfs:subClassOf rdf:resource="http://humanbehaviourchange.org/ontology/BCIO_007205"/>
        <obo:IAO_0000114>Published</obo:IAO_0000114>
        <obo:IAO_0000115>A promise positive consequence for approximating behaviour BCT in which the consequence is an interpersonal process or a proxy interpersonal process.</obo:IAO_0000115>
        <obo:IAO_0000118>social incentive for approximating behaviour</obo:IAO_0000118>
        <rdfs:comment>A proxy interpersonal process is where the person interacts with a chatbot, digital assistant, or similar computer program designed to simulate and process human communication</rdfs:comment>
        <rdfs:label>promise positive social consequence for approximating behaviour BCT</rdfs:label>
    </owl:Class>
    


    <!-- http://humanbehaviourchange.org/ontology/BCIO_007221 -->

    <owl:Class rdf:about="http://humanbehaviourchange.org/ontology/BCIO_007221">
        <rdfs:subClassOf rdf:resource="http://humanbehaviourchange.org/ontology/BCIO_007206"/>
        <obo:IAO_0000114>Published</obo:IAO_0000114>
        <obo:IAO_0000115>A promise positive consequence for completion of behavioural sequence BCT in which the consequence is an interpersonal process or a proxy interpersonal process.</obo:IAO_0000115>
        <obo:IAO_0000118>social incentive for completion of behavioural sequence</obo:IAO_0000118>
        <rdfs:comment>A proxy interpersonal process is where the person interacts with a chatbot, digital assistant, or similar computer program designed to simulate and process human communication</rdfs:comment>
        <rdfs:label>promise positive social consequence for completion of behavioural sequence BCT</rdfs:label>
    </owl:Class>
    


    <!-- http://humanbehaviourchange.org/ontology/BCIO_007222 -->

    <owl:Class rdf:about="http://humanbehaviourchange.org/ontology/BCIO_007222">
        <rdfs:subClassOf rdf:resource="http://humanbehaviourchange.org/ontology/BCIO_007207"/>
        <obo:IAO_0000114>Published</obo:IAO_0000114>
        <obo:IAO_0000115>A promise positive consequence for incompatible behaviour BCT in which the consequence is an interpersonal process or a proxy interpersonal process.</obo:IAO_0000115>
        <obo:IAO_0000118>social incentive for incompatible behaviour</obo:IAO_0000118>
        <rdfs:comment>A proxy interpersonal process is where the person interacts with a chatbot, digital assistant, or similar computer program designed to simulate and process human communication</rdfs:comment>
        <rdfs:label>promise positive social consequence for incompatible behaviour BCT</rdfs:label>
    </owl:Class>
    


    <!-- http://humanbehaviourchange.org/ontology/BCIO_007223 -->

    <owl:Class rdf:about="http://humanbehaviourchange.org/ontology/BCIO_007223">
        <rdfs:subClassOf rdf:resource="http://humanbehaviourchange.org/ontology/BCIO_007208"/>
        <obo:IAO_0000114>Published</obo:IAO_0000114>
        <obo:IAO_0000115>A promise positive consequence for situation specific behaviour BCT in which the consequence is an interpersonal process or a proxy interpersonal process.</obo:IAO_0000115>
        <obo:IAO_0000118>social incentive for situation specific behaviour</obo:IAO_0000118>
        <rdfs:comment>A proxy interpersonal process is where the person interacts with a chatbot, digital assistant, or similar computer program designed to simulate and process human communication</rdfs:comment>
        <rdfs:label>promise positive social consequence for situation specific behaviour BCT</rdfs:label>
    </owl:Class>
    


    <!-- http://humanbehaviourchange.org/ontology/BCIO_007224 -->

    <owl:Class rdf:about="http://humanbehaviourchange.org/ontology/BCIO_007224">
        <rdfs:subClassOf rdf:resource="http://humanbehaviourchange.org/ontology/BCIO_007216"/>
        <obo:IAO_0000114>Published</obo:IAO_0000114>
        <obo:IAO_0000115>A promise positive consequence for outcome of behaviour BCT where the consequence is an interpersonal process or a proxy interpersonal process.</obo:IAO_0000115>
        <rdfs:comment>A proxy interpersonal process is where the person interacts with a chatbot, digital assistant, or similar computer program designed to simulate and process human communication</rdfs:comment>
        <rdfs:label>promise positive social consequence for outcome of behaviour BCT</rdfs:label>
    </owl:Class>
    


    <!-- http://humanbehaviourchange.org/ontology/BCIO_007225 -->

    <owl:Class rdf:about="http://humanbehaviourchange.org/ontology/BCIO_007225">
        <rdfs:subClassOf rdf:resource="http://humanbehaviourchange.org/ontology/BCIO_007189"/>
        <obo:IAO_0000114>Published</obo:IAO_0000114>
        <obo:IAO_0000115>A promise aversive consequence for behaviour BCT that promises to provide the consequence at increasingly less frequent intervals.</obo:IAO_0000115>
        <obo:IAO_0000118>reduce threat frequency</obo:IAO_0000118>
        <rdfs:label>promise reduced frequency of aversive consequence for behaviour BCT</rdfs:label>
    </owl:Class>
    


    <!-- http://humanbehaviourchange.org/ontology/BCIO_007226 -->

    <owl:Class rdf:about="http://humanbehaviourchange.org/ontology/BCIO_007226">
        <rdfs:subClassOf rdf:resource="http://humanbehaviourchange.org/ontology/BCIO_007225"/>
        <obo:IAO_0000114>Published</obo:IAO_0000114>
        <obo:IAO_0000115>A promise reduced frequency of aversive consequence for behaviour BCT in which the consequence is money, vouchers or other valued objects.</obo:IAO_0000115>
        <obo:IAO_0000118>reduce material threat frequency</obo:IAO_0000118>
        <rdfs:label>promise reduced frequency of aversive material consequence for behaviour BCT</rdfs:label>
    </owl:Class>
    


    <!-- http://humanbehaviourchange.org/ontology/BCIO_007227 -->

    <owl:Class rdf:about="http://humanbehaviourchange.org/ontology/BCIO_007227">
        <rdfs:subClassOf rdf:resource="http://humanbehaviourchange.org/ontology/BCIO_007225"/>
        <obo:IAO_0000114>Published</obo:IAO_0000114>
        <obo:IAO_0000115>A promise reduced frequency of aversive consequence for behaviour BCT in which the consequence is an interpersonal process or a proxy interpersonal process.</obo:IAO_0000115>
        <obo:IAO_0000118>reduce social threat frequency</obo:IAO_0000118>
        <rdfs:comment>A proxy interpersonal process is where the person interacts with a chatbot, digital assistant, or similar computer program designed to simulate and process human communication</rdfs:comment>
        <rdfs:label>promise reduced frequency of aversive social consequence for behaviour BCT</rdfs:label>
    </owl:Class>
    


    <!-- http://humanbehaviourchange.org/ontology/BCIO_007228 -->

    <owl:Class rdf:about="http://humanbehaviourchange.org/ontology/BCIO_007228">
        <rdfs:subClassOf rdf:resource="http://humanbehaviourchange.org/ontology/BCIO_007202"/>
        <obo:IAO_0000114>Published</obo:IAO_0000114>
        <obo:IAO_0000115>A promise positive consequence for behaviour BCT that promises to provide the consequence at increasingly less frequent intervals.</obo:IAO_0000115>
        <obo:IAO_0000118>reduce incentive frequency</obo:IAO_0000118>
        <rdfs:label>promise reduced frequency of positive consequence for behaviour BCT</rdfs:label>
    </owl:Class>
    


    <!-- http://humanbehaviourchange.org/ontology/BCIO_007229 -->

    <owl:Class rdf:about="http://humanbehaviourchange.org/ontology/BCIO_007229">
        <rdfs:subClassOf rdf:resource="http://humanbehaviourchange.org/ontology/BCIO_007228"/>
        <obo:IAO_0000114>Published</obo:IAO_0000114>
        <obo:IAO_0000115>A promise reduced frequency of positive consequence for behaviour BCT in which the consequence is money, vouchers or other valued objects.</obo:IAO_0000115>
        <obo:IAO_0000118>reduce material incentive frequency</obo:IAO_0000118>
        <rdfs:label>promise reduced frequency of positive material consequence for behaviour BCT</rdfs:label>
    </owl:Class>
    


    <!-- http://humanbehaviourchange.org/ontology/BCIO_007230 -->

    <owl:Class rdf:about="http://humanbehaviourchange.org/ontology/BCIO_007230">
        <rdfs:subClassOf rdf:resource="http://humanbehaviourchange.org/ontology/BCIO_007228"/>
        <obo:IAO_0000114>Published</obo:IAO_0000114>
        <obo:IAO_0000115>A promise reduced frequency of positive consequence for behaviour BCT in which the consequence is an interpersonal process or a proxy interpersonal process.</obo:IAO_0000115>
        <obo:IAO_0000118>reduce social incentive frequency</obo:IAO_0000118>
        <rdfs:comment>A proxy interpersonal process is where the person interacts with a chatbot, digital assistant, or similar computer program designed to simulate and process human communication</rdfs:comment>
        <rdfs:label>promise reduced frequency of positive social consequence for behaviour BCT</rdfs:label>
    </owl:Class>
    


    <!-- http://humanbehaviourchange.org/ontology/BCIO_007231 -->

    <owl:Class rdf:about="http://humanbehaviourchange.org/ontology/BCIO_007231">
        <rdfs:subClassOf rdf:resource="http://humanbehaviourchange.org/ontology/BCIO_007190"/>
        <obo:IAO_0000114>Published</obo:IAO_0000114>
        <obo:IAO_0000115>A promise to remove aversive consequence for behaviour BCT in which the consequence is money, vouchers or other valued objects.</obo:IAO_0000115>
        <obo:IAO_0000118>incentive to remove material punishment</obo:IAO_0000118>
        <rdfs:label>promise to remove aversive material consequence for behaviour BCT</rdfs:label>
    </owl:Class>
    


    <!-- http://humanbehaviourchange.org/ontology/BCIO_007232 -->

    <owl:Class rdf:about="http://humanbehaviourchange.org/ontology/BCIO_007232">
        <rdfs:subClassOf rdf:resource="http://humanbehaviourchange.org/ontology/BCIO_007196"/>
        <obo:IAO_0000114>Published</obo:IAO_0000114>
        <obo:IAO_0000115>A promise to remove aversive consequence for outcome of behaviour BCT where the consequence is money, vouchers or other valued objects.</obo:IAO_0000115>
        <obo:IAO_0000118>incentive to remove material punishment</obo:IAO_0000118>
        <rdfs:label>promise to remove aversive material consequence for outcome of behaviour BCT</rdfs:label>
    </owl:Class>
    


    <!-- http://humanbehaviourchange.org/ontology/BCIO_007233 -->

    <owl:Class rdf:about="http://humanbehaviourchange.org/ontology/BCIO_007233">
        <rdfs:subClassOf rdf:resource="http://humanbehaviourchange.org/ontology/BCIO_007190"/>
        <obo:IAO_0000114>Published</obo:IAO_0000114>
        <obo:IAO_0000115>A promise to remove aversive consequence for behaviour BCT in which the consequence is an interpersonal process or a proxy interpersonal process</obo:IAO_0000115>
        <obo:IAO_0000118>incentive to remove social punishment</obo:IAO_0000118>
        <rdfs:comment>A proxy interpersonal process is where the person interacts with a chatbot, digital assistant, or similar computer program designed to simulate and process human communication</rdfs:comment>
        <rdfs:label>promise to remove aversive social consequence for behaviour BCT</rdfs:label>
    </owl:Class>
    


    <!-- http://humanbehaviourchange.org/ontology/BCIO_007234 -->

    <owl:Class rdf:about="http://humanbehaviourchange.org/ontology/BCIO_007234">
        <rdfs:subClassOf rdf:resource="http://humanbehaviourchange.org/ontology/BCIO_007196"/>
        <obo:IAO_0000114>Published</obo:IAO_0000114>
        <obo:IAO_0000115>A promise to remove aversive consequence for outcome of behaviour BCT where the consequence is an interpersonal process or a proxy interpersonal process.</obo:IAO_0000115>
        <obo:IAO_0000118>incentive to remove social punishment</obo:IAO_0000118>
        <rdfs:comment>A proxy interpersonal process is where the person interacts with a chatbot, digital assistant, or similar computer program designed to simulate and process human communication</rdfs:comment>
        <rdfs:label>promise to remove aversive social consequence for outcome of behaviour BCT</rdfs:label>
    </owl:Class>
    


    <!-- http://humanbehaviourchange.org/ontology/BCIO_007235 -->

    <owl:Class rdf:about="http://humanbehaviourchange.org/ontology/BCIO_007235">
        <rdfs:subClassOf rdf:resource="http://humanbehaviourchange.org/ontology/BCIO_007203"/>
        <obo:IAO_0000114>Published</obo:IAO_0000114>
        <obo:IAO_0000115>A promise to remove positive consequence for behaviour BCT in which the consequence is money, vouchers or other valued objects.</obo:IAO_0000115>
        <obo:IAO_0000118>threaten to remove material reward</obo:IAO_0000118>
        <rdfs:label>promise to remove positive material consequence for behaviour BCT</rdfs:label>
    </owl:Class>
    


    <!-- http://humanbehaviourchange.org/ontology/BCIO_007236 -->

    <owl:Class rdf:about="http://humanbehaviourchange.org/ontology/BCIO_007236">
        <rdfs:subClassOf rdf:resource="http://humanbehaviourchange.org/ontology/BCIO_007217"/>
        <obo:IAO_0000114>Published</obo:IAO_0000114>
        <obo:IAO_0000115>A promise to remove positive consequence for outcome of behaviour BCT where the consequence is money, vouchers or other valued objects.</obo:IAO_0000115>
        <obo:IAO_0000118>threaten to remove material reward</obo:IAO_0000118>
        <rdfs:label>promise to remove positive material consequence for outcome of behaviour BCT</rdfs:label>
    </owl:Class>
    


    <!-- http://humanbehaviourchange.org/ontology/BCIO_007237 -->

    <owl:Class rdf:about="http://humanbehaviourchange.org/ontology/BCIO_007237">
        <rdfs:subClassOf rdf:resource="http://humanbehaviourchange.org/ontology/BCIO_007203"/>
        <obo:IAO_0000114>Published</obo:IAO_0000114>
        <obo:IAO_0000115>A promise to remove positive consequence for behaviour BCT in which the consequence is an interpersonal process or a proxy interpersonal process</obo:IAO_0000115>
        <obo:IAO_0000118>threaten to remove social reward</obo:IAO_0000118>
        <rdfs:comment>A proxy interpersonal process is where the person interacts with a chatbot, digital assistant, or similar computer program designed to simulate and process human communication</rdfs:comment>
        <rdfs:label>promise to remove positive social consequence for behaviour BCT</rdfs:label>
    </owl:Class>
    


    <!-- http://humanbehaviourchange.org/ontology/BCIO_007238 -->

    <owl:Class rdf:about="http://humanbehaviourchange.org/ontology/BCIO_007238">
        <rdfs:subClassOf rdf:resource="http://humanbehaviourchange.org/ontology/BCIO_007217"/>
        <obo:IAO_0000114>Published</obo:IAO_0000114>
        <obo:IAO_0000115>A promise to remove positive consequence for outcome of behaviour BCT where the consequence is an interpersonal process or a proxy interpersonal process.</obo:IAO_0000115>
        <obo:IAO_0000118>threaten to remove social reward</obo:IAO_0000118>
        <rdfs:comment>A proxy interpersonal process is where the person interacts with a chatbot, digital assistant, or similar computer program designed to simulate and process human communication</rdfs:comment>
        <rdfs:label>promise to remove positive social consequence for outcome of behaviour BCT</rdfs:label>
    </owl:Class>
    


    <!-- http://humanbehaviourchange.org/ontology/BCIO_007239 -->

    <owl:Class rdf:about="http://humanbehaviourchange.org/ontology/BCIO_007239">
        <rdfs:subClassOf rdf:resource="http://humanbehaviourchange.org/ontology/BCIO_033000"/>
        <obo:IAO_0000114>Published</obo:IAO_0000114>
        <obo:IAO_0000115>A behaviour change technique that prompts thinking relating to successful performance of the behaviour.</obo:IAO_0000115>
        <rdfs:label>prompt thinking related to successful performance BCT</rdfs:label>
    </owl:Class>
    


    <!-- http://humanbehaviourchange.org/ontology/BCIO_007240 -->

    <owl:Class rdf:about="http://humanbehaviourchange.org/ontology/BCIO_007240">
        <rdfs:subClassOf rdf:resource="http://humanbehaviourchange.org/ontology/BCIO_007101"/>
        <obo:IAO_0000114>Published</obo:IAO_0000114>
        <obo:IAO_0000115>A behavioural consequence BCT that provides a consequence for the behaviour.</obo:IAO_0000115>
        <rdfs:label>provide consequence for behaviour BCT</rdfs:label>
    </owl:Class>
    


    <!-- http://humanbehaviourchange.org/ontology/BCIO_007241 -->

    <owl:Class rdf:about="http://humanbehaviourchange.org/ontology/BCIO_007241">
        <rdfs:subClassOf rdf:resource="http://humanbehaviourchange.org/ontology/BCIO_007240"/>
        <obo:IAO_0000114>Published</obo:IAO_0000114>
        <obo:IAO_0000115>A provide consequence for behaviour BCT where the consequence is aversive.</obo:IAO_0000115>
        <obo:IAO_0000118>punishment</obo:IAO_0000118>
        <rdfs:comment>To qualify as aversive, the consequence should be aversively valued by the person receiving it.</rdfs:comment>
        <rdfs:label>provide aversive consequence for behaviour BCT</rdfs:label>
    </owl:Class>
    


    <!-- http://humanbehaviourchange.org/ontology/BCIO_007242 -->

    <owl:Class rdf:about="http://humanbehaviourchange.org/ontology/BCIO_007242">
        <rdfs:subClassOf rdf:resource="http://humanbehaviourchange.org/ontology/BCIO_007241"/>
        <obo:IAO_0000114>Published</obo:IAO_0000114>
        <obo:IAO_0000115>A provide aversive consequence for behaviour BCT that provides the consequence for the behaviour in one situation but not in another.</obo:IAO_0000115>
        <obo:IAO_0000118>punishment for situation specific behaviour</obo:IAO_0000118>
        <rdfs:label>provide aversive consequence for situation specific behaviour BCT</rdfs:label>
    </owl:Class>
    


    <!-- http://humanbehaviourchange.org/ontology/BCIO_007243 -->

    <owl:Class rdf:about="http://humanbehaviourchange.org/ontology/BCIO_007243">
        <rdfs:subClassOf rdf:resource="http://humanbehaviourchange.org/ontology/BCIO_007241"/>
        <obo:IAO_0000114>Published</obo:IAO_0000114>
        <obo:IAO_0000115>A provide aversive consequence for behaviour BCT where the consequence is money, vouchers or other valued objects.</obo:IAO_0000115>
        <obo:IAO_0000118>material punishment</obo:IAO_0000118>
        <rdfs:label>provide aversive material consequence for behaviour BCT</rdfs:label>
    </owl:Class>
    


    <!-- http://humanbehaviourchange.org/ontology/BCIO_007244 -->

    <owl:Class rdf:about="http://humanbehaviourchange.org/ontology/BCIO_007244">
        <rdfs:subClassOf rdf:resource="http://humanbehaviourchange.org/ontology/BCIO_007242"/>
        <obo:IAO_0000114>Published</obo:IAO_0000114>
        <obo:IAO_0000115>A provide aversive consequence for situation specific behaviour BCT where the consequence is money, vouchers or other valued objects.</obo:IAO_0000115>
        <obo:IAO_0000118>material punishment for situation specific behaviour</obo:IAO_0000118>
        <rdfs:label>provide aversive material consequence for situation specific behaviour BCT</rdfs:label>
    </owl:Class>
    


    <!-- http://humanbehaviourchange.org/ontology/BCIO_007245 -->

    <owl:Class rdf:about="http://humanbehaviourchange.org/ontology/BCIO_007245">
        <rdfs:subClassOf rdf:resource="http://humanbehaviourchange.org/ontology/BCIO_007246"/>
        <obo:IAO_0000114>Published</obo:IAO_0000114>
        <obo:IAO_0000115>A provide aversive consequence for outcome of behaviour BCT where the consequence is money, vouchers or other valued objects.</obo:IAO_0000115>
        <obo:IAO_0000118>material punishment</obo:IAO_0000118>
        <rdfs:label>provide aversive material consequence for outcome of behaviour BCT</rdfs:label>
    </owl:Class>
    


    <!-- http://humanbehaviourchange.org/ontology/BCIO_007246 -->

    <owl:Class rdf:about="http://humanbehaviourchange.org/ontology/BCIO_007246">
        <rdfs:subClassOf rdf:resource="http://humanbehaviourchange.org/ontology/BCIO_007250"/>
        <obo:IAO_0000114>Published</obo:IAO_0000114>
        <obo:IAO_0000115>A provide consequence for outcome of behaviour BCT where the consequence is aversive.</obo:IAO_0000115>
        <obo:IAO_0000118>punishment</obo:IAO_0000118>
        <rdfs:comment>To qualify as aversive, the consequence should be aversively valued by the person receiving it.</rdfs:comment>
        <rdfs:label>provide aversive consequence for outcome of behaviour BCT</rdfs:label>
    </owl:Class>
    


    <!-- http://humanbehaviourchange.org/ontology/BCIO_007247 -->

    <owl:Class rdf:about="http://humanbehaviourchange.org/ontology/BCIO_007247">
        <rdfs:subClassOf rdf:resource="http://humanbehaviourchange.org/ontology/BCIO_007241"/>
        <obo:IAO_0000114>Published</obo:IAO_0000114>
        <obo:IAO_0000115>A provide aversive consequence for behaviour BCT where the consequence is an interpersonal process or a proxy interpersonal process.</obo:IAO_0000115>
        <obo:IAO_0000118>social punishment</obo:IAO_0000118>
        <rdfs:comment>A proxy interpersonal process is where the person interacts with a chatbot, digital assistant, or similar computer program designed to simulate and process human communication</rdfs:comment>
        <rdfs:label>provide aversive social consequence for behaviour BCT</rdfs:label>
    </owl:Class>
    


    <!-- http://humanbehaviourchange.org/ontology/BCIO_007248 -->

    <owl:Class rdf:about="http://humanbehaviourchange.org/ontology/BCIO_007248">
        <rdfs:subClassOf rdf:resource="http://humanbehaviourchange.org/ontology/BCIO_007242"/>
        <obo:IAO_0000114>Published</obo:IAO_0000114>
        <obo:IAO_0000115>A provide aversive consequence for situation specific behaviour BCT where the consequence is an interpersonal process or a proxy interpersonal process.</obo:IAO_0000115>
        <obo:IAO_0000118>social punishment for situation specific behaviour</obo:IAO_0000118>
        <rdfs:comment>A proxy interpersonal process is where the person interacts with a chatbot, digital assistant, or similar computer program designed to simulate and process human communication</rdfs:comment>
        <rdfs:label>provide aversive social consequence for situation specific behaviour BCT</rdfs:label>
    </owl:Class>
    


    <!-- http://humanbehaviourchange.org/ontology/BCIO_007249 -->

    <owl:Class rdf:about="http://humanbehaviourchange.org/ontology/BCIO_007249">
        <rdfs:subClassOf rdf:resource="http://humanbehaviourchange.org/ontology/BCIO_007246"/>
        <obo:IAO_0000114>Published</obo:IAO_0000114>
        <obo:IAO_0000115>A provide aversive consequence for outcome of behaviour BCT where the consequence is an interpersonal process or a proxy interpersonal process.</obo:IAO_0000115>
        <obo:IAO_0000118>social punishment</obo:IAO_0000118>
        <rdfs:comment>A proxy interpersonal process is where the person interacts with a chatbot, digital assistant, or similar computer program designed to simulate and process human communication</rdfs:comment>
        <rdfs:label>provide aversive social consequence for outcome of behaviour BCT</rdfs:label>
    </owl:Class>
    


    <!-- http://humanbehaviourchange.org/ontology/BCIO_007250 -->

    <owl:Class rdf:about="http://humanbehaviourchange.org/ontology/BCIO_007250">
        <rdfs:subClassOf rdf:resource="http://humanbehaviourchange.org/ontology/BCIO_007186"/>
        <obo:IAO_0000114>Published</obo:IAO_0000114>
        <obo:IAO_0000115>An outcome consequence BCT that provides a consequence for an outcome resulting from performing or not performing the behaviour.</obo:IAO_0000115>
        <rdfs:label>provide consequence for outcome of behaviour BCT</rdfs:label>
    </owl:Class>
    


    <!-- http://humanbehaviourchange.org/ontology/BCIO_007251 -->

    <owl:Class rdf:about="http://humanbehaviourchange.org/ontology/BCIO_007251">
        <rdfs:subClassOf rdf:resource="http://humanbehaviourchange.org/ontology/BCIO_007252"/>
        <obo:IAO_0000112>Provide a reward for consuming low sugar food instead of high sugar food</obo:IAO_0000112>
        <obo:IAO_0000114>Published</obo:IAO_0000114>
        <obo:IAO_0000115>A provide positive consequence for behaviour BCT that provides the consequence for a behaviour that is different from the unwanted behaviour.</obo:IAO_0000115>
        <obo:IAO_0000118>differential reinforcement, reward for alternative behaviour</obo:IAO_0000118>
        <rdfs:label>provide positive consequence for alternative behaviour BCT</rdfs:label>
    </owl:Class>
    


    <!-- http://humanbehaviourchange.org/ontology/BCIO_007252 -->

    <owl:Class rdf:about="http://humanbehaviourchange.org/ontology/BCIO_007252">
        <rdfs:subClassOf rdf:resource="http://humanbehaviourchange.org/ontology/BCIO_007240"/>
        <obo:IAO_0000114>Published</obo:IAO_0000114>
        <obo:IAO_0000115>A provide consequence for behaviour BCT where the consequence is positive.</obo:IAO_0000115>
        <obo:IAO_0000118>positive reinforcement, reward</obo:IAO_0000118>
        <rdfs:comment>To qualify as positive, the consequence should be positively valued by the person receiving it. If informed of consequence in advance of rewarded behaviour, also code &apos;promise positive consequence for behaviour BCT&apos; or one of its child classses.</rdfs:comment>
        <rdfs:label>provide positive consequence for behaviour BCT</rdfs:label>
    </owl:Class>
    


    <!-- http://humanbehaviourchange.org/ontology/BCIO_007253 -->

    <owl:Class rdf:about="http://humanbehaviourchange.org/ontology/BCIO_007253">
        <rdfs:subClassOf rdf:resource="http://humanbehaviourchange.org/ontology/BCIO_007252"/>
        <obo:IAO_0000112>Reward a person who has recently had a stroke who is learning to use cutlery again</obo:IAO_0000112>
        <obo:IAO_0000114>Published</obo:IAO_0000114>
        <obo:IAO_0000115>A provide positive consequence for behaviour BCT where the consequence is provided as the performance gradually gets closer to the behaviour.</obo:IAO_0000115>
        <obo:IAO_0000118>shaping, reward for approximating behaviour</obo:IAO_0000118>
        <rdfs:label>provide positive consequence for approximating behaviour BCT</rdfs:label>
    </owl:Class>
    


    <!-- http://humanbehaviourchange.org/ontology/BCIO_007254 -->

    <owl:Class rdf:about="http://humanbehaviourchange.org/ontology/BCIO_007254">
        <rdfs:subClassOf rdf:resource="http://humanbehaviourchange.org/ontology/BCIO_007252"/>
        <obo:IAO_0000114>Published</obo:IAO_0000114>
        <obo:IAO_0000115>A provide positive consequence for behaviour BCT where the consequence is provided for performing the final behaviour in a sequence of behaviours, followed by adding behaviours that occur earlier in the sequence.</obo:IAO_0000115>
        <obo:IAO_0000118>backward chaining, reward for completion of behavoural sequence</obo:IAO_0000118>
        <rdfs:label>provide positive consequence for completion of behavioural sequence BCT</rdfs:label>
    </owl:Class>
    


    <!-- http://humanbehaviourchange.org/ontology/BCIO_007255 -->

    <owl:Class rdf:about="http://humanbehaviourchange.org/ontology/BCIO_007255">
        <rdfs:subClassOf rdf:resource="http://humanbehaviourchange.org/ontology/BCIO_007252"/>
        <obo:IAO_0000112>Provide a reward when a person folds their arms or sits on their hands instead of touching their face.</obo:IAO_0000112>
        <obo:IAO_0000114>Published</obo:IAO_0000114>
        <obo:IAO_0000115>A provide positive consequence for behaviour BCT that provides the consequence for a behaviour that is incompatible with the unwanted behaviour.</obo:IAO_0000115>
        <obo:IAO_0000118>counter-conditioning, reward for incompatible behaviour</obo:IAO_0000118>
        <rdfs:label>provide positive consequence for incompatible behaviour BCT</rdfs:label>
    </owl:Class>
    


    <!-- http://humanbehaviourchange.org/ontology/BCIO_007256 -->

    <owl:Class rdf:about="http://humanbehaviourchange.org/ontology/BCIO_007256">
        <rdfs:subClassOf rdf:resource="http://humanbehaviourchange.org/ontology/BCIO_007252"/>
        <obo:IAO_0000114>Published</obo:IAO_0000114>
        <obo:IAO_0000115>A provide positive consequence for behaviour BCT that provides the consequence for the behaviour in one situation but not in another.</obo:IAO_0000115>
        <obo:IAO_0000118>discrimination training, reward for situation specific behaviour</obo:IAO_0000118>
        <rdfs:label>provide positive consequence for situation specific behaviour BCT</rdfs:label>
    </owl:Class>
    


    <!-- http://humanbehaviourchange.org/ontology/BCIO_007257 -->

    <owl:Class rdf:about="http://humanbehaviourchange.org/ontology/BCIO_007257">
        <rdfs:subClassOf rdf:resource="http://humanbehaviourchange.org/ontology/BCIO_007252"/>
        <obo:IAO_0000114>Published</obo:IAO_0000114>
        <obo:IAO_0000115>A provide positive consequence for behaviour BCT where the consequence is money, vouchers or other valued objects.</obo:IAO_0000115>
        <obo:IAO_0000118>material reward, tangible reinforcement</obo:IAO_0000118>
        <rdfs:label>provide positive material consequence for behaviour BCT</rdfs:label>
    </owl:Class>
    


    <!-- http://humanbehaviourchange.org/ontology/BCIO_007258 -->

    <owl:Class rdf:about="http://humanbehaviourchange.org/ontology/BCIO_007258">
        <rdfs:subClassOf rdf:resource="http://humanbehaviourchange.org/ontology/BCIO_007251"/>
        <obo:IAO_0000114>Published</obo:IAO_0000114>
        <obo:IAO_0000115>A provide positive consequence for alternative behaviour BCT where the consequence is money, vouchers or other valued objects.</obo:IAO_0000115>
        <obo:IAO_0000118>material reward for alternative behaviour</obo:IAO_0000118>
        <rdfs:label>provide positive material consequence for alternative behaviour BCT</rdfs:label>
    </owl:Class>
    


    <!-- http://humanbehaviourchange.org/ontology/BCIO_007259 -->

    <owl:Class rdf:about="http://humanbehaviourchange.org/ontology/BCIO_007259">
        <rdfs:subClassOf rdf:resource="http://humanbehaviourchange.org/ontology/BCIO_007253"/>
        <obo:IAO_0000114>Published</obo:IAO_0000114>
        <obo:IAO_0000115>A provide positive consequence for approximating behaviour BCT where the consequence is money, vouchers or other valued objects.</obo:IAO_0000115>
        <obo:IAO_0000118>material reward for approximating behaviour</obo:IAO_0000118>
        <rdfs:label>provide positive material consequence for approximating behaviour BCT</rdfs:label>
    </owl:Class>
    


    <!-- http://humanbehaviourchange.org/ontology/BCIO_007260 -->

    <owl:Class rdf:about="http://humanbehaviourchange.org/ontology/BCIO_007260">
        <rdfs:subClassOf rdf:resource="http://humanbehaviourchange.org/ontology/BCIO_007254"/>
        <obo:IAO_0000114>Published</obo:IAO_0000114>
        <obo:IAO_0000115>A provide positive consequence for completion of behavioural sequence BCT where the consequence is money, vouchers or other valued objects.</obo:IAO_0000115>
        <obo:IAO_0000118>material reward for completion of behavoural sequence</obo:IAO_0000118>
        <rdfs:label>provide positive material consequence for completion of behavioural sequence BCT</rdfs:label>
    </owl:Class>
    


    <!-- http://humanbehaviourchange.org/ontology/BCIO_007261 -->

    <owl:Class rdf:about="http://humanbehaviourchange.org/ontology/BCIO_007261">
        <rdfs:subClassOf rdf:resource="http://humanbehaviourchange.org/ontology/BCIO_007255"/>
        <obo:IAO_0000114>Published</obo:IAO_0000114>
        <obo:IAO_0000115>A provide positive consequence for incompatible behaviour BCT where the consequence is money, vouchers or other valued objects.</obo:IAO_0000115>
        <obo:IAO_0000118>material reward for incompatible behaviour</obo:IAO_0000118>
        <rdfs:label>provide positive material consequence for incompatible behaviour BCT</rdfs:label>
    </owl:Class>
    


    <!-- http://humanbehaviourchange.org/ontology/BCIO_007262 -->

    <owl:Class rdf:about="http://humanbehaviourchange.org/ontology/BCIO_007262">
        <rdfs:subClassOf rdf:resource="http://humanbehaviourchange.org/ontology/BCIO_007256"/>
        <obo:IAO_0000114>Published</obo:IAO_0000114>
        <obo:IAO_0000115>A provide positive consequence for situation specific behaviour BCT where the consequence is money, vouchers or other valued objects.</obo:IAO_0000115>
        <obo:IAO_0000118>material reward for situation specific behaviour</obo:IAO_0000118>
        <rdfs:label>provide positive material consequence for situation specific behaviour BCT</rdfs:label>
    </owl:Class>
    


    <!-- http://humanbehaviourchange.org/ontology/BCIO_007263 -->

    <owl:Class rdf:about="http://humanbehaviourchange.org/ontology/BCIO_007263">
        <rdfs:subClassOf rdf:resource="http://humanbehaviourchange.org/ontology/BCIO_007264"/>
        <obo:IAO_0000114>Published</obo:IAO_0000114>
        <obo:IAO_0000115>A provide positive consequence for outcome of behaviour BCT where the consequence is money, vouchers or other valued objects.</obo:IAO_0000115>
        <obo:IAO_0000118>material reward, tangible reinforcement</obo:IAO_0000118>
        <rdfs:label>provide positive material consequence for outcome of behaviour BCT</rdfs:label>
    </owl:Class>
    


    <!-- http://humanbehaviourchange.org/ontology/BCIO_007264 -->

    <owl:Class rdf:about="http://humanbehaviourchange.org/ontology/BCIO_007264">
        <rdfs:subClassOf rdf:resource="http://humanbehaviourchange.org/ontology/BCIO_007250"/>
        <obo:IAO_0000114>Published</obo:IAO_0000114>
        <obo:IAO_0000115>A provide consequence for outcome of behaviour BCT where the consequence is positive.</obo:IAO_0000115>
        <obo:IAO_0000118>positive reinforcement, reward</obo:IAO_0000118>
        <rdfs:comment>To qualify as positive, the consequence should be positively valued by the person receiving it.</rdfs:comment>
        <rdfs:label>provide positive consequence for outcome of behaviour BCT</rdfs:label>
    </owl:Class>
    


    <!-- http://humanbehaviourchange.org/ontology/BCIO_007265 -->

    <owl:Class rdf:about="http://humanbehaviourchange.org/ontology/BCIO_007265">
        <rdfs:subClassOf rdf:resource="http://humanbehaviourchange.org/ontology/BCIO_007252"/>
        <obo:IAO_0000114>Published</obo:IAO_0000114>
        <obo:IAO_0000115>A provide positive consequence for behaviour BCT where the consequence is an interpersonal process or a proxy interpersonal process.</obo:IAO_0000115>
        <obo:IAO_0000118>social reward</obo:IAO_0000118>
        <rdfs:comment>A proxy interpersonal process is where the person interacts with a chatbot, digital assistant, or similar computer program designed to simulate and process human communication</rdfs:comment>
        <rdfs:label>provide positive social consequence for behaviour BCT</rdfs:label>
    </owl:Class>
    


    <!-- http://humanbehaviourchange.org/ontology/BCIO_007266 -->

    <owl:Class rdf:about="http://humanbehaviourchange.org/ontology/BCIO_007266">
        <rdfs:subClassOf rdf:resource="http://humanbehaviourchange.org/ontology/BCIO_007251"/>
        <obo:IAO_0000114>Published</obo:IAO_0000114>
        <obo:IAO_0000115>A provide positive consequence for alternative behaviour BCT where the consequence is an interpersonal process or a proxy interpersonal process.</obo:IAO_0000115>
        <obo:IAO_0000118>social reward for alternative behaviour</obo:IAO_0000118>
        <rdfs:comment>A proxy interpersonal process is where the person interacts with a chatbot, digital assistant, or similar computer program designed to simulate and process human communication</rdfs:comment>
        <rdfs:label>provide positive social consequence for alternative behaviour BCT</rdfs:label>
    </owl:Class>
    


    <!-- http://humanbehaviourchange.org/ontology/BCIO_007267 -->

    <owl:Class rdf:about="http://humanbehaviourchange.org/ontology/BCIO_007267">
        <rdfs:subClassOf rdf:resource="http://humanbehaviourchange.org/ontology/BCIO_007253"/>
        <obo:IAO_0000114>Published</obo:IAO_0000114>
        <obo:IAO_0000115>A provide positive consequence for approximating behaviour BCT where the consequence is an interpersonal process or a proxy interpersonal process.</obo:IAO_0000115>
        <obo:IAO_0000118>social reward for approximating behaviour</obo:IAO_0000118>
        <rdfs:comment>A proxy interpersonal process is where the person interacts with a chatbot, digital assistant, or similar computer program designed to simulate and process human communication</rdfs:comment>
        <rdfs:label>provide positive social consequence for approximating behaviour BCT</rdfs:label>
    </owl:Class>
    


    <!-- http://humanbehaviourchange.org/ontology/BCIO_007268 -->

    <owl:Class rdf:about="http://humanbehaviourchange.org/ontology/BCIO_007268">
        <rdfs:subClassOf rdf:resource="http://humanbehaviourchange.org/ontology/BCIO_007254"/>
        <obo:IAO_0000114>Published</obo:IAO_0000114>
        <obo:IAO_0000115>A provide positive consequence for completion of behavioural sequence BCT where the consequence is an interpersonal process or a proxy interpersonal process.</obo:IAO_0000115>
        <obo:IAO_0000118>social reward for completion of behavoural sequence</obo:IAO_0000118>
        <rdfs:comment>A proxy interpersonal process is where the person interacts with a chatbot, digital assistant, or similar computer program designed to simulate and process human communication</rdfs:comment>
        <rdfs:label>provide positive social consequence for completion of behavioural sequence BCT</rdfs:label>
    </owl:Class>
    


    <!-- http://humanbehaviourchange.org/ontology/BCIO_007269 -->

    <owl:Class rdf:about="http://humanbehaviourchange.org/ontology/BCIO_007269">
        <rdfs:subClassOf rdf:resource="http://humanbehaviourchange.org/ontology/BCIO_007255"/>
        <obo:IAO_0000114>Published</obo:IAO_0000114>
        <obo:IAO_0000115>A provide positive consequence for incompatible behaviour BCT where the consequence is an interpersonal process or a proxy interpersonal process.</obo:IAO_0000115>
        <obo:IAO_0000118>social reward for incompatible behaviour</obo:IAO_0000118>
        <rdfs:comment>A proxy interpersonal process is where the person interacts with a chatbot, digital assistant, or similar computer program designed to simulate and process human communication</rdfs:comment>
        <rdfs:label>provide positive social consequence for incompatible behaviour BCT</rdfs:label>
    </owl:Class>
    


    <!-- http://humanbehaviourchange.org/ontology/BCIO_007270 -->

    <owl:Class rdf:about="http://humanbehaviourchange.org/ontology/BCIO_007270">
        <rdfs:subClassOf rdf:resource="http://humanbehaviourchange.org/ontology/BCIO_007256"/>
        <obo:IAO_0000114>Published</obo:IAO_0000114>
        <obo:IAO_0000115>A provide positive consequence for  situation specific behaviour BCT where the consequence is an interpersonal process or a proxy interpersonal process.</obo:IAO_0000115>
        <obo:IAO_0000118>social reward for situation specific behaviour</obo:IAO_0000118>
        <rdfs:comment>A proxy interpersonal process is where the person interacts with a chatbot, digital assistant, or similar computer program designed to simulate and process human communication</rdfs:comment>
        <rdfs:label>provide positive social consequence for situation specific behaviour BCT</rdfs:label>
    </owl:Class>
    


    <!-- http://humanbehaviourchange.org/ontology/BCIO_007271 -->

    <owl:Class rdf:about="http://humanbehaviourchange.org/ontology/BCIO_007271">
        <rdfs:subClassOf rdf:resource="http://humanbehaviourchange.org/ontology/BCIO_007264"/>
        <obo:IAO_0000114>Published</obo:IAO_0000114>
        <obo:IAO_0000115>A provide positive consequence for outcome of behaviour BCT where the consequence is an interpersonal process or a proxy interpersonal process.</obo:IAO_0000115>
        <obo:IAO_0000118>social reward</obo:IAO_0000118>
        <rdfs:comment>A proxy interpersonal process is where the person interacts with a chatbot, digital assistant, or similar computer program designed to simulate and process human communication</rdfs:comment>
        <rdfs:label>provide positive social consequence for outcome of behaviour BCT</rdfs:label>
    </owl:Class>
    


    <!-- http://humanbehaviourchange.org/ontology/BCIO_007272 -->

    <owl:Class rdf:about="http://humanbehaviourchange.org/ontology/BCIO_007272">
        <rdfs:subClassOf rdf:resource="http://humanbehaviourchange.org/ontology/BCIO_007281"/>
        <obo:IAO_0000114>Published</obo:IAO_0000114>
        <obo:IAO_0000115>A provide reduced frequency of positive consequence for outcome of behaviour BCT where the consequence is money, vouchers or other valued objects.</obo:IAO_0000115>
        <obo:IAO_0000118>reduce material reward frequency</obo:IAO_0000118>
        <rdfs:label>provide reduced frequency of positive material consequence for outcome of behaviour BCT</rdfs:label>
    </owl:Class>
    


    <!-- http://humanbehaviourchange.org/ontology/BCIO_007273 -->

    <owl:Class rdf:about="http://humanbehaviourchange.org/ontology/BCIO_007273">
        <rdfs:subClassOf rdf:resource="http://humanbehaviourchange.org/ontology/BCIO_007241"/>
        <obo:IAO_0000114>Published</obo:IAO_0000114>
        <obo:IAO_0000115>A provide aversive consequence for behaviour BCT that provides the consequence at increasingly less frequent intervals.</obo:IAO_0000115>
        <obo:IAO_0000118>reduce punishment frequency</obo:IAO_0000118>
        <rdfs:label>provide reduced frequency of aversive consequence for behaviour BCT</rdfs:label>
    </owl:Class>
    


    <!-- http://humanbehaviourchange.org/ontology/BCIO_007274 -->

    <owl:Class rdf:about="http://humanbehaviourchange.org/ontology/BCIO_007274">
        <rdfs:subClassOf rdf:resource="http://humanbehaviourchange.org/ontology/BCIO_007273"/>
        <obo:IAO_0000114>Published</obo:IAO_0000114>
        <obo:IAO_0000115>A provide reduced frequency of aversive consequence for behaviour BCT where the consequence is money, vouchers or other valued objects.</obo:IAO_0000115>
        <obo:IAO_0000118>reduce material punishment frequency</obo:IAO_0000118>
        <rdfs:label>provide reduced frequency of aversive material consequence for behaviour BCT</rdfs:label>
    </owl:Class>
    


    <!-- http://humanbehaviourchange.org/ontology/BCIO_007275 -->

    <owl:Class rdf:about="http://humanbehaviourchange.org/ontology/BCIO_007275">
        <rdfs:subClassOf rdf:resource="http://humanbehaviourchange.org/ontology/BCIO_007276"/>
        <obo:IAO_0000114>Published</obo:IAO_0000114>
        <obo:IAO_0000115>A provide reduced frequency of aversive consequence for outcome of behaviour BCT where the consequence is money, vouchers or other valued objects.</obo:IAO_0000115>
        <obo:IAO_0000118>reduce material punishment frequency</obo:IAO_0000118>
        <rdfs:label>provide reduced frequency of aversive material consequence for outcome of behaviour BCT</rdfs:label>
    </owl:Class>
    


    <!-- http://humanbehaviourchange.org/ontology/BCIO_007276 -->

    <owl:Class rdf:about="http://humanbehaviourchange.org/ontology/BCIO_007276">
        <rdfs:subClassOf rdf:resource="http://humanbehaviourchange.org/ontology/BCIO_007246"/>
        <obo:IAO_0000114>Published</obo:IAO_0000114>
        <obo:IAO_0000115>A provide aversive consequence for outcome of behaviour BCT that provides the consequence at increasingly less frequent intervals.</obo:IAO_0000115>
        <obo:IAO_0000118>reduce punishment frequency</obo:IAO_0000118>
        <rdfs:label>provide reduced frequency of aversive consequence for outcome of behaviour BCT</rdfs:label>
    </owl:Class>
    


    <!-- http://humanbehaviourchange.org/ontology/BCIO_007277 -->

    <owl:Class rdf:about="http://humanbehaviourchange.org/ontology/BCIO_007277">
        <rdfs:subClassOf rdf:resource="http://humanbehaviourchange.org/ontology/BCIO_007273"/>
        <obo:IAO_0000114>Published</obo:IAO_0000114>
        <obo:IAO_0000115>A provide reduced frequency of aversive consequence for behaviour BCT where the consequence is an interpersonal process or a proxy interpersonal process.</obo:IAO_0000115>
        <obo:IAO_0000118>reduce social punishment frequency</obo:IAO_0000118>
        <rdfs:comment>A proxy interpersonal process is where the person interacts with a chatbot, digital assistant, or similar computer program designed to simulate and process human communication</rdfs:comment>
        <rdfs:label>provide reduced frequency of aversive social consequence for behaviour BCT</rdfs:label>
    </owl:Class>
    


    <!-- http://humanbehaviourchange.org/ontology/BCIO_007278 -->

    <owl:Class rdf:about="http://humanbehaviourchange.org/ontology/BCIO_007278">
        <rdfs:subClassOf rdf:resource="http://humanbehaviourchange.org/ontology/BCIO_007276"/>
        <obo:IAO_0000114>Published</obo:IAO_0000114>
        <obo:IAO_0000115>A provide reduced frequency of aversive consequence for outcome of behaviour BCT where the consequence is an interpersonal process or a proxy interpersonal process.</obo:IAO_0000115>
        <obo:IAO_0000118>reduce social punishment frequency</obo:IAO_0000118>
        <rdfs:comment>A proxy interpersonal process is where the person interacts with a chatbot, digital assistant, or similar computer program designed to simulate and process human communication</rdfs:comment>
        <rdfs:label>provide reduced frequency of aversive social consequence for outcome of behaviour BCT</rdfs:label>
    </owl:Class>
    


    <!-- http://humanbehaviourchange.org/ontology/BCIO_007279 -->

    <owl:Class rdf:about="http://humanbehaviourchange.org/ontology/BCIO_007279">
        <rdfs:subClassOf rdf:resource="http://humanbehaviourchange.org/ontology/BCIO_007252"/>
        <obo:IAO_0000114>Published</obo:IAO_0000114>
        <obo:IAO_0000115>A provide positive consequence for behaviour BCT that provides the consequence at increasingly less frequent intervals.</obo:IAO_0000115>
        <obo:IAO_0000118>thinning, reduce reward frequency</obo:IAO_0000118>
        <rdfs:label>provide reduced frequency of positive consequence for behaviour BCT</rdfs:label>
    </owl:Class>
    


    <!-- http://humanbehaviourchange.org/ontology/BCIO_007280 -->

    <owl:Class rdf:about="http://humanbehaviourchange.org/ontology/BCIO_007280">
        <rdfs:subClassOf rdf:resource="http://humanbehaviourchange.org/ontology/BCIO_007279"/>
        <obo:IAO_0000114>Published</obo:IAO_0000114>
        <obo:IAO_0000115>A provide reduced frequency of positive consequence for behaviour BCT where the consequence is money, vouchers or other valued objects.</obo:IAO_0000115>
        <obo:IAO_0000118>reduce material reward frequency</obo:IAO_0000118>
        <rdfs:label>provide reduced frequency of positive material consequence for behaviour BCT</rdfs:label>
    </owl:Class>
    


    <!-- http://humanbehaviourchange.org/ontology/BCIO_007281 -->

    <owl:Class rdf:about="http://humanbehaviourchange.org/ontology/BCIO_007281">
        <rdfs:subClassOf rdf:resource="http://humanbehaviourchange.org/ontology/BCIO_007264"/>
        <obo:IAO_0000114>Published</obo:IAO_0000114>
        <obo:IAO_0000115>A provide positive consequence for outcome of behaviour BCT that provides the consequence at increasingly less frequent intervals.</obo:IAO_0000115>
        <obo:IAO_0000118>thinning, reduce reward frequency</obo:IAO_0000118>
        <rdfs:label>provide reduced frequency of positive consequence for outcome of behaviour BCT</rdfs:label>
    </owl:Class>
    


    <!-- http://humanbehaviourchange.org/ontology/BCIO_007282 -->

    <owl:Class rdf:about="http://humanbehaviourchange.org/ontology/BCIO_007282">
        <rdfs:subClassOf rdf:resource="http://humanbehaviourchange.org/ontology/BCIO_007279"/>
        <obo:IAO_0000114>Published</obo:IAO_0000114>
        <obo:IAO_0000115>A provide reduced frequency of positive consequence for behaviour BCT where the consequence is an interpersonal process or a proxy interpersonal process.</obo:IAO_0000115>
        <obo:IAO_0000118>reduce social reward frequency</obo:IAO_0000118>
        <rdfs:comment>A proxy interpersonal process is where the person interacts with a chatbot, digital assistant, or similar computer program designed to simulate and process human communication</rdfs:comment>
        <rdfs:label>provide reduced frequency of positive social consequence for behaviour BCT</rdfs:label>
    </owl:Class>
    


    <!-- http://humanbehaviourchange.org/ontology/BCIO_007283 -->

    <owl:Class rdf:about="http://humanbehaviourchange.org/ontology/BCIO_007283">
        <rdfs:subClassOf rdf:resource="http://humanbehaviourchange.org/ontology/BCIO_007281"/>
        <obo:IAO_0000114>Published</obo:IAO_0000114>
        <obo:IAO_0000115>A provide reduced frequency of positive consequence for outcome of behaviour BCT where the consequence is an interpersonal process or a proxy interpersonal process.</obo:IAO_0000115>
        <obo:IAO_0000118>reduce social reward frequency</obo:IAO_0000118>
        <rdfs:comment>A proxy interpersonal process is where the person interacts with a chatbot, digital assistant, or similar computer program designed to simulate and process human communication</rdfs:comment>
        <rdfs:label>provide reduced frequency of positive social consequence for outcome of behaviour BCT</rdfs:label>
    </owl:Class>
    


    <!-- http://humanbehaviourchange.org/ontology/BCIO_007284 -->

    <owl:Class rdf:about="http://humanbehaviourchange.org/ontology/BCIO_007284">
        <rdfs:subClassOf rdf:resource="http://humanbehaviourchange.org/ontology/BCIO_050348"/>
        <obo:IAO_0000114>Published</obo:IAO_0000114>
        <obo:IAO_0000115>A restructure the physical environment BCT that reduces an alternative focus for attention for the person to concentrate on internal or external states or events associated with the behaviour.</obo:IAO_0000115>
        <rdfs:comment>Reducing a distraction to zero is equivalent to removing a distraction</rdfs:comment>
        <rdfs:label>reduce distraction BCT</rdfs:label>
    </owl:Class>
    


    <!-- http://humanbehaviourchange.org/ontology/BCIO_007285 -->

    <owl:Class rdf:about="http://humanbehaviourchange.org/ontology/BCIO_007285">
        <rdfs:subClassOf rdf:resource="http://humanbehaviourchange.org/ontology/BCIO_007101"/>
        <obo:IAO_0000114>Published</obo:IAO_0000114>
        <obo:IAO_0000115>A behavioural consequence BCT that removes a previously provided consequence for performing the behaviour.</obo:IAO_0000115>
        <rdfs:label>remove consequence for behaviour BCT</rdfs:label>
    </owl:Class>
    


    <!-- http://humanbehaviourchange.org/ontology/BCIO_007286 -->

    <owl:Class rdf:about="http://humanbehaviourchange.org/ontology/BCIO_007286">
        <rdfs:subClassOf rdf:resource="http://humanbehaviourchange.org/ontology/BCIO_007285"/>
        <obo:IAO_0000114>Published</obo:IAO_0000114>
        <obo:IAO_0000115>A remove consequence for behaviour BCT where the consequence is aversive.</obo:IAO_0000115>
        <obo:IAO_0000118>negative reinforcement, remove punishment</obo:IAO_0000118>
        <rdfs:comment>To qualify as aversive, the consequence should have been aversively valued by the person receiving it.</rdfs:comment>
        <rdfs:label>remove aversive consequence for behaviour BCT</rdfs:label>
    </owl:Class>
    


    <!-- http://humanbehaviourchange.org/ontology/BCIO_007287 -->

    <owl:Class rdf:about="http://humanbehaviourchange.org/ontology/BCIO_007287">
        <rdfs:subClassOf rdf:resource="http://humanbehaviourchange.org/ontology/BCIO_007286"/>
        <obo:IAO_0000114>Published</obo:IAO_0000114>
        <obo:IAO_0000115>A remove aversive consequence for behaviour BCT where the consequence is money, vouchers or other valued objects.</obo:IAO_0000115>
        <obo:IAO_0000118>remove material punishment</obo:IAO_0000118>
        <rdfs:label>remove aversive material consequence for behaviour BCT</rdfs:label>
    </owl:Class>
    


    <!-- http://humanbehaviourchange.org/ontology/BCIO_007288 -->

    <owl:Class rdf:about="http://humanbehaviourchange.org/ontology/BCIO_007288">
        <rdfs:subClassOf rdf:resource="http://humanbehaviourchange.org/ontology/BCIO_007289"/>
        <obo:IAO_0000114>Published</obo:IAO_0000114>
        <obo:IAO_0000115>A remove aversive consequence for outcome of behaviour BCT in which the consequence is money, vouchers or other valued objects.</obo:IAO_0000115>
        <obo:IAO_0000118>remove material punishment</obo:IAO_0000118>
        <rdfs:label>remove aversive material consequence for outcome of behaviour BCT</rdfs:label>
    </owl:Class>
    


    <!-- http://humanbehaviourchange.org/ontology/BCIO_007289 -->

    <owl:Class rdf:about="http://humanbehaviourchange.org/ontology/BCIO_007289">
        <rdfs:subClassOf rdf:resource="http://humanbehaviourchange.org/ontology/BCIO_007292"/>
        <obo:IAO_0000114>Published</obo:IAO_0000114>
        <obo:IAO_0000115>A remove consequence for outcome of behaviour BCT in which the consequence is aversive.</obo:IAO_0000115>
        <obo:IAO_0000118>negative reinforcement, remove punishment</obo:IAO_0000118>
        <rdfs:comment>To qualify as aversive, the consequence should have been aversively valued by the person receiving it.</rdfs:comment>
        <rdfs:label>remove aversive consequence for outcome of behaviour BCT</rdfs:label>
    </owl:Class>
    


    <!-- http://humanbehaviourchange.org/ontology/BCIO_007290 -->

    <owl:Class rdf:about="http://humanbehaviourchange.org/ontology/BCIO_007290">
        <rdfs:subClassOf rdf:resource="http://humanbehaviourchange.org/ontology/BCIO_007286"/>
        <obo:IAO_0000114>Published</obo:IAO_0000114>
        <obo:IAO_0000115>A remove aversive consequence for behaviour BCT where the consequence is an interpersonal process or a proxy interpersonal process.</obo:IAO_0000115>
        <obo:IAO_0000118>remove social punishment</obo:IAO_0000118>
        <rdfs:comment>A proxy interpersonal process is where the person interacts with a chatbot, digital assistant, or similar computer program designed to simulate and process human communication</rdfs:comment>
        <rdfs:label>remove aversive social consequence for behaviour BCT</rdfs:label>
    </owl:Class>
    


    <!-- http://humanbehaviourchange.org/ontology/BCIO_007291 -->

    <owl:Class rdf:about="http://humanbehaviourchange.org/ontology/BCIO_007291">
        <rdfs:subClassOf rdf:resource="http://humanbehaviourchange.org/ontology/BCIO_007289"/>
        <obo:IAO_0000114>Published</obo:IAO_0000114>
        <obo:IAO_0000115>A remove aversive consequence for outcome of behaviour BCT in which the consequence is an interpersonal process or a proxy interpersonal process.</obo:IAO_0000115>
        <obo:IAO_0000118>remove social punishment</obo:IAO_0000118>
        <rdfs:comment>A proxy interpersonal process is where the person interacts with a chatbot, digital assistant, or similar computer program designed to simulate and process human communication</rdfs:comment>
        <rdfs:label>remove aversive social consequence for outcome of behaviour BCT</rdfs:label>
    </owl:Class>
    


    <!-- http://humanbehaviourchange.org/ontology/BCIO_007292 -->

    <owl:Class rdf:about="http://humanbehaviourchange.org/ontology/BCIO_007292">
        <rdfs:subClassOf rdf:resource="http://humanbehaviourchange.org/ontology/BCIO_007186"/>
        <obo:IAO_0000114>Published</obo:IAO_0000114>
        <obo:IAO_0000115>An outcome consequence BCT that removes a previously provided consequence for an outcome resulting from performing or not performing the behaviour.</obo:IAO_0000115>
        <rdfs:label>remove consequence for outcome of behaviour BCT</rdfs:label>
    </owl:Class>
    


    <!-- http://humanbehaviourchange.org/ontology/BCIO_007293 -->

    <owl:Class rdf:about="http://humanbehaviourchange.org/ontology/BCIO_007293">
        <rdfs:subClassOf rdf:resource="http://humanbehaviourchange.org/ontology/BCIO_007285"/>
        <obo:IAO_0000114>Published</obo:IAO_0000114>
        <obo:IAO_0000115>A remove consequence for behaviour BCT where the consequence is positive.</obo:IAO_0000115>
        <obo:IAO_0000118>time out, response cost, extinction, remove reward</obo:IAO_0000118>
        <rdfs:comment>To qualify as positive, the consequence should have been positively valued by the person receiving it.</rdfs:comment>
        <rdfs:label>remove positive consequence for behaviour BCT</rdfs:label>
    </owl:Class>
    


    <!-- http://humanbehaviourchange.org/ontology/BCIO_007294 -->

    <owl:Class rdf:about="http://humanbehaviourchange.org/ontology/BCIO_007294">
        <rdfs:subClassOf rdf:resource="http://humanbehaviourchange.org/ontology/BCIO_007293"/>
        <obo:IAO_0000114>Published</obo:IAO_0000114>
        <obo:IAO_0000115>A remove positive consequence for behaviour BCT where the consequence is money, vouchers or other valued objects.</obo:IAO_0000115>
        <obo:IAO_0000118>remove material reward</obo:IAO_0000118>
        <rdfs:label>remove positive material consequence for behaviour BCT</rdfs:label>
    </owl:Class>
    


    <!-- http://humanbehaviourchange.org/ontology/BCIO_007295 -->

    <owl:Class rdf:about="http://humanbehaviourchange.org/ontology/BCIO_007295">
        <rdfs:subClassOf rdf:resource="http://humanbehaviourchange.org/ontology/BCIO_007296"/>
        <obo:IAO_0000114>Published</obo:IAO_0000114>
        <obo:IAO_0000115>A remove positive consequence for outcome of behaviour BCT in which the consequence is money, vouchers or other valued objects.</obo:IAO_0000115>
        <obo:IAO_0000118>remove material reward</obo:IAO_0000118>
        <rdfs:label>remove positive material consequence for outcome of behaviour BCT</rdfs:label>
    </owl:Class>
    


    <!-- http://humanbehaviourchange.org/ontology/BCIO_007296 -->

    <owl:Class rdf:about="http://humanbehaviourchange.org/ontology/BCIO_007296">
        <rdfs:subClassOf rdf:resource="http://humanbehaviourchange.org/ontology/BCIO_007292"/>
        <obo:IAO_0000114>Published</obo:IAO_0000114>
        <obo:IAO_0000115>A remove consequence for outcome of behaviour BCT in which the consequence is positive.</obo:IAO_0000115>
        <obo:IAO_0000118>remove reward</obo:IAO_0000118>
        <rdfs:comment>To qualify as positive, the consequence should have been positively valued by the person receiving it.</rdfs:comment>
        <rdfs:label>remove positive consequence for outcome of behaviour BCT</rdfs:label>
    </owl:Class>
    


    <!-- http://humanbehaviourchange.org/ontology/BCIO_007297 -->

    <owl:Class rdf:about="http://humanbehaviourchange.org/ontology/BCIO_007297">
        <rdfs:subClassOf rdf:resource="http://humanbehaviourchange.org/ontology/BCIO_007293"/>
        <obo:IAO_0000114>Published</obo:IAO_0000114>
        <obo:IAO_0000115>A remove positive consequence for behaviour BCT where the consequence is an interpersonal process or a proxy interpersonal process.</obo:IAO_0000115>
        <obo:IAO_0000118>remove social reward</obo:IAO_0000118>
        <rdfs:comment>A proxy interpersonal process is where the person interacts with a chatbot, digital assistant, or similar computer program designed to simulate and process human communication</rdfs:comment>
        <rdfs:label>remove positive social consequence for behaviour BCT</rdfs:label>
    </owl:Class>
    


    <!-- http://humanbehaviourchange.org/ontology/BCIO_007298 -->

    <owl:Class rdf:about="http://humanbehaviourchange.org/ontology/BCIO_007298">
        <rdfs:subClassOf rdf:resource="http://humanbehaviourchange.org/ontology/BCIO_007296"/>
        <obo:IAO_0000114>Published</obo:IAO_0000114>
        <obo:IAO_0000115>A remove positive consequence for outcome of behaviour BCT in which the consequence is an interpersonal process or a proxy interpersonal process.</obo:IAO_0000115>
        <obo:IAO_0000118>remove social reward</obo:IAO_0000118>
        <rdfs:comment>A proxy interpersonal process is where the person interacts with a chatbot, digital assistant, or similar computer program designed to simulate and process human communication</rdfs:comment>
        <rdfs:label>remove positive social consequence for outcome of behaviour BCT</rdfs:label>
    </owl:Class>
    


    <!-- http://humanbehaviourchange.org/ontology/BCIO_007299 -->

    <owl:Class rdf:about="http://humanbehaviourchange.org/ontology/BCIO_007299">
        <rdfs:subClassOf rdf:resource="http://humanbehaviourchange.org/ontology/BCIO_007001"/>
        <obo:IAO_0000114>Published</obo:IAO_0000114>
        <obo:IAO_0000115>A goal directed BCT that reviews progress towards a behavioural goal and considers modifying the plan to achieve the goal.</obo:IAO_0000115>
        <rdfs:comment>A goal is a cognitive representation of an end state towards which one is striving.</rdfs:comment>
        <rdfs:label>review behaviour goal plan BCT</rdfs:label>
    </owl:Class>
    


    <!-- http://humanbehaviourchange.org/ontology/BCIO_007300 -->

    <owl:Class rdf:about="http://humanbehaviourchange.org/ontology/BCIO_007300">
        <rdfs:subClassOf rdf:resource="http://humanbehaviourchange.org/ontology/BCIO_007003"/>
        <obo:IAO_0000114>Published</obo:IAO_0000114>
        <obo:IAO_0000115>A set behaviour goal BCT that describes the behaviour to be achieved in terms of a measurable target.</obo:IAO_0000115>
        <rdfs:comment>A behaviour goal might be set in general terms e.g. &quot;to do more physical activity&quot; or in measurable terms e.g. &quot;to do 30 minutes of physical activity five times a week&quot; or &quot;to walk 8000 steps a day.&quot; Use this class for measurable behaviour goals</rdfs:comment>
        <rdfs:label>set measurable behaviour goal BCT</rdfs:label>
    </owl:Class>
    


    <!-- http://humanbehaviourchange.org/ontology/BCIO_007301 -->

    <owl:Class rdf:about="http://humanbehaviourchange.org/ontology/BCIO_007301">
        <rdfs:subClassOf rdf:resource="http://humanbehaviourchange.org/ontology/BCIO_007005"/>
        <obo:IAO_0000114>Published</obo:IAO_0000114>
        <obo:IAO_0000115>A set outcome goal BCT that describes the behavioural outcome to be achieved in terms of a measurable target.</obo:IAO_0000115>
        <rdfs:comment>An outcome goal might be set in general terms - e.g. &quot;to lose weight&quot; or in measurable terms - e.g. &quot;to lose 5kg of weight&quot; or &quot;to lose 10% of my body weight&quot;. Use this class for measurable outcome goals</rdfs:comment>
        <rdfs:label>set measurable outcome goal BCT</rdfs:label>
    </owl:Class>
    


    <!-- http://humanbehaviourchange.org/ontology/BCIO_007302 -->

    <owl:Class rdf:about="http://humanbehaviourchange.org/ontology/BCIO_007302">
        <rdfs:subClassOf rdf:resource="http://humanbehaviourchange.org/ontology/BCIO_033000"/>
        <obo:IAO_0000114>Published</obo:IAO_0000114>
        <obo:IAO_0000115>A behaviour change technique that suggests the deliberate adoption of a new perspective on the behaviour.</obo:IAO_0000115>
        <obo:IAO_0000118>cognitive reframing</obo:IAO_0000118>
        <rdfs:label>suggest different perspective on behaviour BCT</rdfs:label>
    </owl:Class>
    


    <!-- http://humanbehaviourchange.org/ontology/BCIO_007303 -->

    <owl:Class rdf:about="http://humanbehaviourchange.org/ontology/BCIO_007303">
        <rdfs:subClassOf rdf:resource="http://humanbehaviourchange.org/ontology/BCIO_007050"/>
        <obo:IAO_0000114>Published</obo:IAO_0000114>
        <obo:IAO_0000115>A guide how to perform behaviour BCT that provides a suggestion regarding how to perform the behaviour.</obo:IAO_0000115>
        <rdfs:label>suggest how to perform behaviour BCT</rdfs:label>
    </owl:Class>
    


    <!-- http://humanbehaviourchange.org/ontology/BCIO_033000 -->

    <owl:Class rdf:about="http://humanbehaviourchange.org/ontology/BCIO_033000">
        <rdfs:subClassOf rdf:resource="http://purl.obolibrary.org/obo/COB_0000082"/>
        <obo:IAO_0000114>Published</obo:IAO_0000114>
        <obo:IAO_0000115>A planned process that is the smallest part of BCI content that is observable, replicable and on its own has the potential to bring about behaviour change</obo:IAO_0000115>
        <rdfs:label>behaviour change technique</rdfs:label>
    </owl:Class>
    


    <!-- http://humanbehaviourchange.org/ontology/BCIO_050330 -->

    <owl:Class rdf:about="http://humanbehaviourchange.org/ontology/BCIO_050330">
        <rdfs:subClassOf rdf:resource="http://humanbehaviourchange.org/ontology/BCIO_007050"/>
        <obo:IAO_0000114>Published</obo:IAO_0000114>
        <obo:IAO_0000115>A guide how to perform behaviour BCT that involves suggesting the person avoid spending time with others who do a behaviour that the person wants to reduce or stop.</obo:IAO_0000115>
        <rdfs:label>advise to avoid people who do an unwanted behaviour BCT</rdfs:label>
    </owl:Class>
    


    <!-- http://humanbehaviourchange.org/ontology/BCIO_050331 -->

    <owl:Class rdf:about="http://humanbehaviourchange.org/ontology/BCIO_050331">
        <rdfs:subClassOf rdf:resource="http://humanbehaviourchange.org/ontology/BCIO_007079"/>
        <obo:IAO_0000114>Published</obo:IAO_0000114>
        <obo:IAO_0000115>An alter external stimulus BCT that involves removing an aversive stimulus to bring about behaviour change.</obo:IAO_0000115>
        <obo:IAO_0000118>escape learning</obo:IAO_0000118>
        <rdfs:label>remove aversive stimulus BCT</rdfs:label>
    </owl:Class>
    


    <!-- http://humanbehaviourchange.org/ontology/BCIO_050332 -->

    <owl:Class rdf:about="http://humanbehaviourchange.org/ontology/BCIO_050332">
        <rdfs:subClassOf rdf:resource="http://humanbehaviourchange.org/ontology/BCIO_007165"/>
        <obo:IAO_0000114>Published</obo:IAO_0000114>
        <obo:IAO_0000115>An advise behavioural ways to change emotions BCT suggesting the person perform a particular behaviour to enhance negative emotions.</obo:IAO_0000115>
        <rdfs:label>advise behavioural ways to increase negative emotions BCT</rdfs:label>
    </owl:Class>
    


    <!-- http://humanbehaviourchange.org/ontology/BCIO_050333 -->

    <owl:Class rdf:about="http://humanbehaviourchange.org/ontology/BCIO_050333">
        <rdfs:subClassOf rdf:resource="http://humanbehaviourchange.org/ontology/BCIO_007165"/>
        <obo:IAO_0000114>Published</obo:IAO_0000114>
        <obo:IAO_0000115>An advise behavioural ways to change emotions BCT suggesting the person perform a particular behaviour to decrease negative emotions.</obo:IAO_0000115>
        <rdfs:label>advise behavioural ways to reduce negative emotions BCT</rdfs:label>
    </owl:Class>
    


    <!-- http://humanbehaviourchange.org/ontology/BCIO_050334 -->

    <owl:Class rdf:about="http://humanbehaviourchange.org/ontology/BCIO_050334">
        <rdfs:subClassOf rdf:resource="http://humanbehaviourchange.org/ontology/BCIO_007166"/>
        <obo:IAO_0000114>Published</obo:IAO_0000114>
        <obo:IAO_0000115>An advise cognitive ways to change emotions BCT suggesting the person deliberately use a particular mental process to enhance positive emotions.</obo:IAO_0000115>
        <rdfs:label>advise cognitive ways to increase positive emotions BCT</rdfs:label>
    </owl:Class>
    


    <!-- http://humanbehaviourchange.org/ontology/BCIO_050335 -->

    <owl:Class rdf:about="http://humanbehaviourchange.org/ontology/BCIO_050335">
        <rdfs:subClassOf rdf:resource="http://humanbehaviourchange.org/ontology/BCIO_007166"/>
        <obo:IAO_0000114>Published</obo:IAO_0000114>
        <obo:IAO_0000115>An advise cognitive ways to change emotions BCT suggesting the person deliberately use a particular mental process to decrease positive emotions.</obo:IAO_0000115>
        <rdfs:label>advise cognitive ways to reduce positive emotions BCT</rdfs:label>
    </owl:Class>
    


    <!-- http://humanbehaviourchange.org/ontology/BCIO_050336 -->

    <owl:Class rdf:about="http://humanbehaviourchange.org/ontology/BCIO_050336">
        <rdfs:subClassOf rdf:resource="http://humanbehaviourchange.org/ontology/BCIO_007166"/>
        <obo:IAO_0000114>Published</obo:IAO_0000114>
        <obo:IAO_0000115>An advise cognitive ways to change emotions BCT suggesting the person deliberately use a particular mental process to enhance negative emotions.</obo:IAO_0000115>
        <rdfs:label>advise cognitive ways to increase negative emotions BCT</rdfs:label>
    </owl:Class>
    


    <!-- http://humanbehaviourchange.org/ontology/BCIO_050337 -->

    <owl:Class rdf:about="http://humanbehaviourchange.org/ontology/BCIO_050337">
        <rdfs:subClassOf rdf:resource="http://humanbehaviourchange.org/ontology/BCIO_007166"/>
        <obo:IAO_0000114>Published</obo:IAO_0000114>
        <obo:IAO_0000115>An advise cognitive ways to change emotions BCT suggesting the person deliberately use a particular mental process to decrease negative emotions.</obo:IAO_0000115>
        <rdfs:label>advise cognitive ways to reduce negative emotions BCT</rdfs:label>
    </owl:Class>
    


    <!-- http://humanbehaviourchange.org/ontology/BCIO_050338 -->

    <owl:Class rdf:about="http://humanbehaviourchange.org/ontology/BCIO_050338">
        <rdfs:subClassOf rdf:resource="http://humanbehaviourchange.org/ontology/BCIO_007167"/>
        <obo:IAO_0000114>Published</obo:IAO_0000114>
        <obo:IAO_0000115>An advise sensory ways to change emotions BCT suggesting the person use a method that stimulates one or more senses to enhance positive emotions.</obo:IAO_0000115>
        <rdfs:label>advise sensory ways to increase positive emotions BCT</rdfs:label>
    </owl:Class>
    


    <!-- http://humanbehaviourchange.org/ontology/BCIO_050339 -->

    <owl:Class rdf:about="http://humanbehaviourchange.org/ontology/BCIO_050339">
        <rdfs:subClassOf rdf:resource="http://humanbehaviourchange.org/ontology/BCIO_007167"/>
        <obo:IAO_0000114>Published</obo:IAO_0000114>
        <obo:IAO_0000115>An advise sensory ways to change emotions BCT suggesting the person use a method that stimulates one or more senses to decrease positive emotions.</obo:IAO_0000115>
        <rdfs:label>advise sensory ways to reduce positive emotions BCT</rdfs:label>
    </owl:Class>
    


    <!-- http://humanbehaviourchange.org/ontology/BCIO_050340 -->

    <owl:Class rdf:about="http://humanbehaviourchange.org/ontology/BCIO_050340">
        <rdfs:subClassOf rdf:resource="http://humanbehaviourchange.org/ontology/BCIO_007167"/>
        <obo:IAO_0000114>Published</obo:IAO_0000114>
        <obo:IAO_0000115>An advise sensory ways to change emotions BCT suggesting the person use a method that stimulates one or more senses to enhance negative emotions.</obo:IAO_0000115>
        <rdfs:label>advise sensory ways to increase negative emotions BCT</rdfs:label>
    </owl:Class>
    


    <!-- http://humanbehaviourchange.org/ontology/BCIO_050341 -->

    <owl:Class rdf:about="http://humanbehaviourchange.org/ontology/BCIO_050341">
        <rdfs:subClassOf rdf:resource="http://humanbehaviourchange.org/ontology/BCIO_007167"/>
        <obo:IAO_0000114>Published</obo:IAO_0000114>
        <obo:IAO_0000115>An advise sensory ways to change emotions BCT suggesting the person use a method that stimulates one or more senses to decrease negative emotions.</obo:IAO_0000115>
        <rdfs:label>advise sensory ways to reduce negative emotions BCT</rdfs:label>
    </owl:Class>
    


    <!-- http://humanbehaviourchange.org/ontology/BCIO_050342 -->

    <owl:Class rdf:about="http://humanbehaviourchange.org/ontology/BCIO_050342">
        <rdfs:subClassOf rdf:resource="http://humanbehaviourchange.org/ontology/BCIO_007147"/>
        <obo:IAO_0000114>Published</obo:IAO_0000114>
        <obo:IAO_0000115>An advise how to change emotions BCT suggesting a method to enhance negative emotions.</obo:IAO_0000115>
        <rdfs:label>advise how to increase negative emotions BCT</rdfs:label>
    </owl:Class>
    


    <!-- http://humanbehaviourchange.org/ontology/BCIO_050343 -->

    <owl:Class rdf:about="http://humanbehaviourchange.org/ontology/BCIO_050343">
        <rdfs:subClassOf rdf:resource="http://humanbehaviourchange.org/ontology/BCIO_007147"/>
        <obo:IAO_0000114>Published</obo:IAO_0000114>
        <obo:IAO_0000115>An advise how to change emotions BCT suggesting a method to enhance positive emotions.</obo:IAO_0000115>
        <rdfs:label>advise how to increase positive emotions BCT</rdfs:label>
    </owl:Class>
    


    <!-- http://humanbehaviourchange.org/ontology/BCIO_050344 -->

    <owl:Class rdf:about="http://humanbehaviourchange.org/ontology/BCIO_050344">
        <rdfs:subClassOf rdf:resource="http://humanbehaviourchange.org/ontology/BCIO_007147"/>
        <obo:IAO_0000114>Published</obo:IAO_0000114>
        <obo:IAO_0000115>An advise how to change emotions BCT suggesting a method to decrease negative emotions.</obo:IAO_0000115>
        <obo:IAO_0000118>stress management</obo:IAO_0000118>
        <rdfs:comment>If includes analysing the behavioural problem, also code &apos;goal strategising BCT&apos;</rdfs:comment>
        <rdfs:label>advise how to reduce negative emotions BCT</rdfs:label>
    </owl:Class>
    


    <!-- http://humanbehaviourchange.org/ontology/BCIO_050345 -->

    <owl:Class rdf:about="http://humanbehaviourchange.org/ontology/BCIO_050345">
        <rdfs:subClassOf rdf:resource="http://humanbehaviourchange.org/ontology/BCIO_007147"/>
        <obo:IAO_0000114>Published</obo:IAO_0000114>
        <obo:IAO_0000115>An advise how to change emotions BCT suggesting a method to decrease positive emotions.</obo:IAO_0000115>
        <rdfs:label>advise how to reduce positive emotions BCT</rdfs:label>
    </owl:Class>
    


    <!-- http://humanbehaviourchange.org/ontology/BCIO_050346 -->

    <owl:Class rdf:about="http://humanbehaviourchange.org/ontology/BCIO_050346">
        <rdfs:subClassOf rdf:resource="http://humanbehaviourchange.org/ontology/BCIO_050349"/>
        <obo:IAO_0000114>Published</obo:IAO_0000114>
        <obo:IAO_0000115>A restructure the social environment BCT that changes the person&apos;s directly experienced environment at the time the behaviour is, or would have been, performed.</obo:IAO_0000115>
        <rdfs:label>directly restructure the social environment BCT</rdfs:label>
    </owl:Class>
    


    <!-- http://humanbehaviourchange.org/ontology/BCIO_050347 -->

    <owl:Class rdf:about="http://humanbehaviourchange.org/ontology/BCIO_050347">
        <rdfs:subClassOf rdf:resource="http://humanbehaviourchange.org/ontology/BCIO_050349"/>
        <obo:IAO_0000114>Published</obo:IAO_0000114>
        <obo:IAO_0000115>A restructure the social environment BCT that changes the person&apos;s environment at a time or location other than when and where the behaviour is performed.</obo:IAO_0000115>
        <rdfs:label>indirectly restructure the social environment BCT</rdfs:label>
    </owl:Class>
    


    <!-- http://humanbehaviourchange.org/ontology/BCIO_050348 -->

    <owl:Class rdf:about="http://humanbehaviourchange.org/ontology/BCIO_050348">
        <rdfs:subClassOf rdf:resource="http://humanbehaviourchange.org/ontology/BCIO_007150"/>
        <obo:IAO_0000114>Published</obo:IAO_0000114>
        <obo:IAO_0000115>A restructure the environment BCT that alters the physical environment in which the behaviour is, or would have been, performed in a way that facilitates or impedes the behaviour.</obo:IAO_0000115>
        <obo:IAO_0000118>physical space reorganisation, environmental modification</obo:IAO_0000118>
        <rdfs:comment>This may also involve &apos;reduce exposure to cues for the behaviour BCT&apos;</rdfs:comment>
        <rdfs:label>restructure the physical environment BCT</rdfs:label>
    </owl:Class>
    


    <!-- http://humanbehaviourchange.org/ontology/BCIO_050349 -->

    <owl:Class rdf:about="http://humanbehaviourchange.org/ontology/BCIO_050349">
        <rdfs:subClassOf rdf:resource="http://humanbehaviourchange.org/ontology/BCIO_007150"/>
        <obo:IAO_0000112> Instructing schoolchildren to form a single file queue rather than mingle in a crowd.</obo:IAO_0000112>
        <obo:IAO_0000112>Instructing people in a smoking cessation group to sit in a circle rather than in rows</obo:IAO_0000112>
        <obo:IAO_0000114>Published</obo:IAO_0000114>
        <obo:IAO_0000115>A restructure the environment BCT that alters the social environment in which the behaviour is, or would have been, performed in a way that facilitates or impedes the behaviour.</obo:IAO_0000115>
        <obo:IAO_0000118>interpersonal environment restructuring, social context modification</obo:IAO_0000118>
        <rdfs:comment>This may also involve &apos;reduce exposure to cues for the behaviour BCT&apos;</rdfs:comment>
        <rdfs:label>restructure the social environment BCT</rdfs:label>
    </owl:Class>
    


    <!-- http://humanbehaviourchange.org/ontology/BCIO_050350 -->

    <owl:Class rdf:about="http://humanbehaviourchange.org/ontology/BCIO_050350">
        <rdfs:subClassOf rdf:resource="http://humanbehaviourchange.org/ontology/BCIO_007165"/>
        <obo:IAO_0000114>Published</obo:IAO_0000114>
        <obo:IAO_0000115>An advise behavioural ways to change emotions BCT suggesting the person perform a particular behaviour to enhance positive emotions.</obo:IAO_0000115>
        <rdfs:label>advise behavioural ways to increase positive emotions BCT</rdfs:label>
    </owl:Class>
    


    <!-- http://humanbehaviourchange.org/ontology/BCIO_050351 -->

    <owl:Class rdf:about="http://humanbehaviourchange.org/ontology/BCIO_050351">
        <rdfs:subClassOf rdf:resource="http://humanbehaviourchange.org/ontology/BCIO_007165"/>
        <obo:IAO_0000114>Published</obo:IAO_0000114>
        <obo:IAO_0000115>An advise behavioural ways to change emotions BCT suggesting the person perform a particular behaviour to decrease positive emotions.</obo:IAO_0000115>
        <rdfs:label>advise behavioural ways to reduce positive emotions BCT</rdfs:label>
    </owl:Class>
    


    <!-- http://humanbehaviourchange.org/ontology/BCIO_050445 -->

    <owl:Class rdf:about="http://humanbehaviourchange.org/ontology/BCIO_050445">
        <rdfs:subClassOf rdf:resource="http://humanbehaviourchange.org/ontology/BCIO_007001"/>
        <obo:IAO_0000114>Proposed</obo:IAO_0000114>
        <obo:IAO_0000115>A goal directed BCT that changes an existing goal for the behaviour to be achieved.</obo:IAO_0000115>
        <rdfs:comment>A goal is a cognitive representation of an end state towards which one is striving.</rdfs:comment>
        <rdfs:label>change behaviour goal BCT</rdfs:label>
    </owl:Class>
    


    <!-- http://humanbehaviourchange.org/ontology/BCIO_050446 -->

    <owl:Class rdf:about="http://humanbehaviourchange.org/ontology/BCIO_050446">
        <rdfs:subClassOf rdf:resource="http://humanbehaviourchange.org/ontology/BCIO_007001"/>
        <obo:IAO_0000114>Proposed</obo:IAO_0000114>
        <obo:IAO_0000115>A goal directed BCT that changes an existing goal for the outcome to be achieved.</obo:IAO_0000115>
        <rdfs:comment>A goal is a cognitive representation of an end state towards which one is striving.</rdfs:comment>
        <rdfs:label>change outcome goal BCT</rdfs:label>
    </owl:Class>
</rdf:RDF>



<!-- Generated by the OWL API (version 4.5.26) https://github.com/owlcs/owlapi -->

