<?xml version="1.0"?>
<rdf:RDF xmlns="http://humanbehaviourchange.org/ontology/bcio_mode_of_delivery.owl#"
     xml:base="http://humanbehaviourchange.org/ontology/bcio_mode_of_delivery.owl"
     xmlns:dc="http://purl.org/dc/elements/1.1/"
     xmlns:obo="http://purl.obolibrary.org/obo/"
     xmlns:owl="http://www.w3.org/2002/07/owl#"
     xmlns:rdf="http://www.w3.org/1999/02/22-rdf-syntax-ns#"
     xmlns:xml="http://www.w3.org/XML/1998/namespace"
     xmlns:xsd="http://www.w3.org/2001/XMLSchema#"
     xmlns:foaf="http://xmlns.com/foaf/0.1/"
     xmlns:rdfs="http://www.w3.org/2000/01/rdf-schema#"
     xmlns:sssom="https://w3id.org/sssom/"
     xmlns:terms="http://purl.org/dc/terms/"
     xmlns:schema="https://schema.org/"
     xmlns:Property="https://www.wikidata.org/wiki/Property:"
     xmlns:oboInOwl="http://www.geneontology.org/formats/oboInOwl#"
     xmlns:owlready_ontology="http://www.lesfleursdunormal.fr/static/_downloads/owlready_ontology.owl#">
    <owl:Ontology rdf:about="http://humanbehaviourchange.org/ontology/bcio_mode_of_delivery.owl">
        <owl:imports rdf:resource="http://humanbehaviourchange.org/ontology/bcio_external.owl"/>
        <owl:imports rdf:resource="http://humanbehaviourchange.org/ontology/bcio_upper_level.owl"/>
    </owl:Ontology>
    


    <!-- 
    ///////////////////////////////////////////////////////////////////////////////////////
    //
    // Classes
    //
    ///////////////////////////////////////////////////////////////////////////////////////
     -->

    


    <!-- http://humanbehaviourchange.org/ontology/BCIO_011000 -->

    <owl:Class rdf:about="http://humanbehaviourchange.org/ontology/BCIO_011000">
        <rdfs:subClassOf rdf:resource="http://humanbehaviourchange.org/ontology/BCIO_043000"/>
        <obo:IAO_0000114>Published</obo:IAO_0000114>
        <obo:IAO_0000115>An attribute of a BCI delivery that is the physical or informational medium through which a BCI is provided.</obo:IAO_0000115>
        <obo:IAO_0000118>BCI mode of delivery</obo:IAO_0000118>
        <rdfs:label>behaviour change intervention mode of delivery</rdfs:label>
    </owl:Class>
    


    <!-- http://humanbehaviourchange.org/ontology/BCIO_011001 -->

    <owl:Class rdf:about="http://humanbehaviourchange.org/ontology/BCIO_011001">
        <rdfs:subClassOf rdf:resource="http://humanbehaviourchange.org/ontology/BCIO_011000"/>
        <obo:IAO_0000114>Published</obo:IAO_0000114>
        <obo:IAO_0000115>Mode of delivery that involves intentional transmission of a representation of the world to an intervention recipient with the aim of changing that person&apos;s representation of the world.</obo:IAO_0000115>
        <rdfs:comment>This includes delivery of rewards, prompts, and cues that result in learning and information about the environment and environmental contingencies.</rdfs:comment>
        <rdfs:label>informational mode of delivery</rdfs:label>
    </owl:Class>
    


    <!-- http://humanbehaviourchange.org/ontology/BCIO_011002 -->

    <owl:Class rdf:about="http://humanbehaviourchange.org/ontology/BCIO_011002">
        <rdfs:subClassOf rdf:resource="http://humanbehaviourchange.org/ontology/BCIO_011001"/>
        <obo:IAO_0000114>Published</obo:IAO_0000114>
        <obo:IAO_0000115>Informational mode of delivery that involves a person as intervention source who interacts with an intervention recipient in real time.</obo:IAO_0000115>
        <rdfs:label>human interactional mode of delivery</rdfs:label>
    </owl:Class>
    


    <!-- http://humanbehaviourchange.org/ontology/BCIO_011003 -->

    <owl:Class rdf:about="http://humanbehaviourchange.org/ontology/BCIO_011003">
        <rdfs:subClassOf rdf:resource="http://humanbehaviourchange.org/ontology/BCIO_011002"/>
        <obo:IAO_0000114>Published</obo:IAO_0000114>
        <obo:IAO_0000115>Human interactional mode of delivery that involves an intervention source and recipient being together in the same location and communicating directly.</obo:IAO_0000115>
        <rdfs:label>face to face mode of delivery</rdfs:label>
    </owl:Class>
    


    <!-- http://humanbehaviourchange.org/ontology/BCIO_011004 -->

    <owl:Class rdf:about="http://humanbehaviourchange.org/ontology/BCIO_011004">
        <rdfs:subClassOf rdf:resource="http://humanbehaviourchange.org/ontology/BCIO_011002"/>
        <obo:IAO_0000114>Published</obo:IAO_0000114>
        <obo:IAO_0000115>Human interactional mode of delivery that involves an intervention source and recipient being in different locations and communicating through a communication channel.</obo:IAO_0000115>
        <rdfs:label>at-a-distance mode of delivery</rdfs:label>
    </owl:Class>
    


    <!-- http://humanbehaviourchange.org/ontology/BCIO_011005 -->

    <owl:Class rdf:about="http://humanbehaviourchange.org/ontology/BCIO_011005">
        <rdfs:subClassOf rdf:resource="http://humanbehaviourchange.org/ontology/BCIO_011001"/>
        <obo:IAO_0000114>Published</obo:IAO_0000114>
        <obo:IAO_0000115>Informational mode of delivery that involves use of printed material.</obo:IAO_0000115>
        <rdfs:comment>Can include paper, acetate, text, diagrams and photographic images.</rdfs:comment>
        <rdfs:label>printed material mode of delivery</rdfs:label>
    </owl:Class>
    


    <!-- http://humanbehaviourchange.org/ontology/BCIO_011006 -->

    <owl:Class rdf:about="http://humanbehaviourchange.org/ontology/BCIO_011006">
        <rdfs:subClassOf rdf:resource="http://humanbehaviourchange.org/ontology/BCIO_011005"/>
        <obo:IAO_0000114>Published</obo:IAO_0000114>
        <obo:IAO_0000115>Printed material mode of delivery that involves a letter or postcard that can be sent through the post or handed directly to the recipient</obo:IAO_0000115>
        <rdfs:label>letter mode of delivery</rdfs:label>
    </owl:Class>
    


    <!-- http://humanbehaviourchange.org/ontology/BCIO_011007 -->

    <owl:Class rdf:about="http://humanbehaviourchange.org/ontology/BCIO_011007">
        <rdfs:subClassOf rdf:resource="http://humanbehaviourchange.org/ontology/BCIO_011005"/>
        <obo:IAO_0000114>Published</obo:IAO_0000114>
        <obo:IAO_0000115>Printed material mode of delivery that involves display of a poster, sign or notice in a public location.</obo:IAO_0000115>
        <rdfs:label>public notice mode of delivery</rdfs:label>
    </owl:Class>
    


    <!-- http://humanbehaviourchange.org/ontology/BCIO_011008 -->

    <owl:Class rdf:about="http://humanbehaviourchange.org/ontology/BCIO_011008">
        <rdfs:subClassOf rdf:resource="http://humanbehaviourchange.org/ontology/BCIO_011005"/>
        <obo:IAO_0000114>Published</obo:IAO_0000114>
        <obo:IAO_0000115>Printed material mode of delivery that involves use of of a printed publication.</obo:IAO_0000115>
        <rdfs:comment>Includes leaflets, brochures, newspapers, newsletter, booklets, mazazines, manuals or worksheets.</rdfs:comment>
        <rdfs:label>printed publication mode of delivery</rdfs:label>
    </owl:Class>
    


    <!-- http://humanbehaviourchange.org/ontology/BCIO_011009 -->

    <owl:Class rdf:about="http://humanbehaviourchange.org/ontology/BCIO_011009">
        <rdfs:subClassOf rdf:resource="http://humanbehaviourchange.org/ontology/BCIO_011005"/>
        <obo:IAO_0000114>Published</obo:IAO_0000114>
        <obo:IAO_0000115>Printed material mode of delivery that involves information printed on a product or its packaging, or a label attached to or included with, a product or its packaging, and aims to convey information about that product.</obo:IAO_0000115>
        <rdfs:label>labelling mode of delivery</rdfs:label>
    </owl:Class>
    


    <!-- http://humanbehaviourchange.org/ontology/BCIO_011010 -->

    <owl:Class rdf:about="http://humanbehaviourchange.org/ontology/BCIO_011010">
        <rdfs:subClassOf rdf:resource="http://humanbehaviourchange.org/ontology/BCIO_011001"/>
        <obo:IAO_0000114>Published</obo:IAO_0000114>
        <obo:IAO_0000115>Informational mode of delivery that involves electronic technology in the presentation of information to an intervention recipient.</obo:IAO_0000115>
        <obo:IAO_0000232>Electronic has been used rather than digital because not all of the content may involve digital encoding - some may be analogue. Also, it is the electronic nature that is central not the means of encoding.</obo:IAO_0000232>
        <rdfs:label>electronic mode of delivery</rdfs:label>
    </owl:Class>
    


    <!-- http://humanbehaviourchange.org/ontology/BCIO_011011 -->

    <owl:Class rdf:about="http://humanbehaviourchange.org/ontology/BCIO_011011">
        <rdfs:subClassOf rdf:resource="http://humanbehaviourchange.org/ontology/BCIO_011010"/>
        <obo:IAO_0000114>Published</obo:IAO_0000114>
        <obo:IAO_0000115>Electronic mode of delivery that involves presentation of information that is broadcast and displayed by television.</obo:IAO_0000115>
        <rdfs:comment>Includes internet and satellite television.</rdfs:comment>
        <rdfs:label>television mode of delivery</rdfs:label>
    </owl:Class>
    


    <!-- http://humanbehaviourchange.org/ontology/BCIO_011012 -->

    <owl:Class rdf:about="http://humanbehaviourchange.org/ontology/BCIO_011012">
        <rdfs:subClassOf rdf:resource="http://humanbehaviourchange.org/ontology/BCIO_011010"/>
        <obo:IAO_0000114>Published</obo:IAO_0000114>
        <obo:IAO_0000115>Electronic mode of delivery that involves presentation of information by a handheld mobile digital device that can store, retrieve and process data.</obo:IAO_0000115>
        <rdfs:label>mobile digital device mode of delivery</rdfs:label>
    </owl:Class>
    


    <!-- http://humanbehaviourchange.org/ontology/BCIO_011013 -->

    <owl:Class rdf:about="http://humanbehaviourchange.org/ontology/BCIO_011013">
        <rdfs:subClassOf rdf:resource="http://humanbehaviourchange.org/ontology/BCIO_011010"/>
        <obo:IAO_0000114>Published</obo:IAO_0000114>
        <obo:IAO_0000115>Electronic mode of delivery that involves presentation of information by a desktop or laptop computer.</obo:IAO_0000115>
        <rdfs:label>computer mode of delivery</rdfs:label>
    </owl:Class>
    


    <!-- http://humanbehaviourchange.org/ontology/BCIO_011014 -->

    <owl:Class rdf:about="http://humanbehaviourchange.org/ontology/BCIO_011014">
        <rdfs:subClassOf rdf:resource="http://humanbehaviourchange.org/ontology/BCIO_011010"/>
        <obo:IAO_0000114>Published</obo:IAO_0000114>
        <obo:IAO_0000115>Electronic mode of delivery that involves presentation of information by an electronic screen positioned in a public location.</obo:IAO_0000115>
        <rdfs:label>electronic billboard mode of delivery</rdfs:label>
    </owl:Class>
    


    <!-- http://humanbehaviourchange.org/ontology/BCIO_011015 -->

    <owl:Class rdf:about="http://humanbehaviourchange.org/ontology/BCIO_011015">
        <rdfs:subClassOf rdf:resource="http://humanbehaviourchange.org/ontology/BCIO_011010"/>
        <obo:IAO_0000114>Published</obo:IAO_0000114>
        <obo:IAO_0000115>Electronic mode of delivery that involves presentation of information by an electronic device that is worn or carried on the body.</obo:IAO_0000115>
        <rdfs:comment>Includes a watch, clip-on device, spectacles, in-ear devfice, vibrating device.</rdfs:comment>
        <rdfs:label>wearable electronic device mode of delivery</rdfs:label>
    </owl:Class>
    


    <!-- http://humanbehaviourchange.org/ontology/BCIO_011016 -->

    <owl:Class rdf:about="http://humanbehaviourchange.org/ontology/BCIO_011016">
        <rdfs:subClassOf rdf:resource="http://humanbehaviourchange.org/ontology/BCIO_011010"/>
        <obo:IAO_0000114>Published</obo:IAO_0000114>
        <obo:IAO_0000115>Electronic mode of delivery that involves an electronic device positioned in the environment of the intervention recipient that can gather information and respond to commands.</obo:IAO_0000115>
        <rdfs:comment>Includes robots, and &apos;internet of things&apos;.</rdfs:comment>
        <rdfs:label>electronic environmental object mode of delivery</rdfs:label>
    </owl:Class>
    


    <!-- http://humanbehaviourchange.org/ontology/BCIO_011017 -->

    <owl:Class rdf:about="http://humanbehaviourchange.org/ontology/BCIO_011017">
        <rdfs:subClassOf rdf:resource="http://humanbehaviourchange.org/ontology/BCIO_011010"/>
        <obo:IAO_0000114>Published</obo:IAO_0000114>
        <obo:IAO_0000115>Electronic mode of delivery that involves presentation of a 3-D image.</obo:IAO_0000115>
        <rdfs:comment>Includes hologram but does not include virtual reality headsets.</rdfs:comment>
        <rdfs:label>3-D projection mode of delivery</rdfs:label>
    </owl:Class>
    


    <!-- http://humanbehaviourchange.org/ontology/BCIO_011018 -->

    <owl:Class rdf:about="http://humanbehaviourchange.org/ontology/BCIO_011018">
        <rdfs:subClassOf rdf:resource="http://humanbehaviourchange.org/ontology/BCIO_011010"/>
        <obo:IAO_0000114>Published</obo:IAO_0000114>
        <obo:IAO_0000115>Electronic mode of delivery that involves use of virtual reality through a virtual reality headset and optionally body movement sensors.</obo:IAO_0000115>
        <rdfs:label>virtual reality mode of delivery</rdfs:label>
    </owl:Class>
    


    <!-- http://humanbehaviourchange.org/ontology/BCIO_011019 -->

    <owl:Class rdf:about="http://humanbehaviourchange.org/ontology/BCIO_011019">
        <rdfs:subClassOf rdf:resource="http://humanbehaviourchange.org/ontology/BCIO_011010"/>
        <obo:IAO_0000114>Published</obo:IAO_0000114>
        <obo:IAO_0000115>Electronic mode of delivery that involves presentation of information stored on an object that is inserted into a playing device.</obo:IAO_0000115>
        <rdfs:comment>Includes cassettes, video tapes, DVDs, CDs.</rdfs:comment>
        <rdfs:label>playable electronic storage mode of delivery</rdfs:label>
    </owl:Class>
    


    <!-- http://humanbehaviourchange.org/ontology/BCIO_011020 -->

    <owl:Class rdf:about="http://humanbehaviourchange.org/ontology/BCIO_011020">
        <rdfs:subClassOf rdf:resource="http://humanbehaviourchange.org/ontology/BCIO_011010"/>
        <obo:IAO_0000114>Published</obo:IAO_0000114>
        <obo:IAO_0000115>Electronic mode of delivery that involves presentation of audio information that is broadcast and received by a radio receiver.</obo:IAO_0000115>
        <rdfs:comment>Includes digital radio and audio that is streamed as a podcast.</rdfs:comment>
        <rdfs:label>radio broadcast mode of delivery</rdfs:label>
    </owl:Class>
    


    <!-- http://humanbehaviourchange.org/ontology/BCIO_011021 -->

    <owl:Class rdf:about="http://humanbehaviourchange.org/ontology/BCIO_011021">
        <rdfs:subClassOf rdf:resource="http://humanbehaviourchange.org/ontology/BCIO_011010"/>
        <obo:IAO_0000114>Published</obo:IAO_0000114>
        <obo:IAO_0000115>Electronic mode of delivery that involves a communication process in which a signal is sent by a caller to a recipient to alert them of the communication intent, giving the recipient the opportunity to enage with the communication.</obo:IAO_0000115>
        <obo:IAO_0000232>Added in order to be able to capture the concept of a &apos;call&apos;.</obo:IAO_0000232>
        <rdfs:label>call mode of delivery</rdfs:label>
    </owl:Class>
    


    <!-- http://humanbehaviourchange.org/ontology/BCIO_011022 -->

    <owl:Class rdf:about="http://humanbehaviourchange.org/ontology/BCIO_011022">
        <rdfs:subClassOf rdf:resource="http://humanbehaviourchange.org/ontology/BCIO_011021"/>
        <obo:IAO_0000114>Published</obo:IAO_0000114>
        <obo:IAO_0000115>Call mode of delivery that involves only audio information in the communication.</obo:IAO_0000115>
        <rdfs:comment>Includes automated calls and audio messaging.</rdfs:comment>
        <rdfs:label>audio call mode of delivery</rdfs:label>
    </owl:Class>
    


    <!-- http://humanbehaviourchange.org/ontology/BCIO_011023 -->

    <owl:Class rdf:about="http://humanbehaviourchange.org/ontology/BCIO_011023">
        <rdfs:subClassOf rdf:resource="http://humanbehaviourchange.org/ontology/BCIO_011021"/>
        <obo:IAO_0000114>Published</obo:IAO_0000114>
        <obo:IAO_0000115>Call mode of delivery that involves video and audio information in the communication.</obo:IAO_0000115>
        <rdfs:label>video call mode of delivery</rdfs:label>
    </owl:Class>
    


    <!-- http://humanbehaviourchange.org/ontology/BCIO_011024 -->

    <owl:Class rdf:about="http://humanbehaviourchange.org/ontology/BCIO_011024">
        <rdfs:subClassOf rdf:resource="http://humanbehaviourchange.org/ontology/BCIO_011021"/>
        <obo:IAO_0000114>Published</obo:IAO_0000114>
        <obo:IAO_0000115>Call mode of delivery that involves textual information in the communication.</obo:IAO_0000115>
        <rdfs:comment>Text message can include emojis, and additional audio and pictorial material. Includes SMS, WhatsApp and other messaging services.</rdfs:comment>
        <rdfs:label>messaging mode of delivery</rdfs:label>
    </owl:Class>
    


    <!-- http://humanbehaviourchange.org/ontology/BCIO_011025 -->

    <owl:Class rdf:about="http://humanbehaviourchange.org/ontology/BCIO_011025">
        <rdfs:subClassOf rdf:resource="http://humanbehaviourchange.org/ontology/BCIO_011010"/>
        <obo:IAO_0000114>Published</obo:IAO_0000114>
        <obo:IAO_0000115>Electronic mode of delivery that involves communication by email.</obo:IAO_0000115>
        <rdfs:label>email mode of delivery</rdfs:label>
    </owl:Class>
    


    <!-- http://humanbehaviourchange.org/ontology/BCIO_011026 -->

    <owl:Class rdf:about="http://humanbehaviourchange.org/ontology/BCIO_011026">
        <rdfs:subClassOf rdf:resource="http://humanbehaviourchange.org/ontology/BCIO_011010"/>
        <obo:IAO_0000114>Published</obo:IAO_0000114>
        <obo:IAO_0000115>Electronic mode of delivery that involves the intervention recipient playing a computer game.</obo:IAO_0000115>
        <rdfs:label>video game mode of delivery</rdfs:label>
    </owl:Class>
    


    <!-- http://humanbehaviourchange.org/ontology/BCIO_011027 -->

    <owl:Class rdf:about="http://humanbehaviourchange.org/ontology/BCIO_011027">
        <rdfs:subClassOf rdf:resource="http://humanbehaviourchange.org/ontology/BCIO_011010"/>
        <obo:IAO_0000114>Published</obo:IAO_0000114>
        <obo:IAO_0000115>Electronic mode of delivery that involves the intervention recipient interacting with a website.</obo:IAO_0000115>
        <rdfs:label>website mode of delivery</rdfs:label>
    </owl:Class>
    


    <!-- http://humanbehaviourchange.org/ontology/BCIO_011028 -->

    <owl:Class rdf:about="http://humanbehaviourchange.org/ontology/BCIO_011028">
        <rdfs:subClassOf rdf:resource="http://humanbehaviourchange.org/ontology/BCIO_011010"/>
        <obo:IAO_0000114>Published</obo:IAO_0000114>
        <obo:IAO_0000115>Electronic mode of delivery that involves the intervention recipient interacting with a mobile application.</obo:IAO_0000115>
        <obo:IAO_0000232>The distinction between websites and mobile applications has become blurred with the advent of webapps.</obo:IAO_0000232>
        <rdfs:label>mobile application mode of delivery</rdfs:label>
    </owl:Class>
    


    <!-- http://humanbehaviourchange.org/ontology/BCIO_011029 -->

    <owl:Class rdf:about="http://humanbehaviourchange.org/ontology/BCIO_011029">
        <rdfs:subClassOf rdf:resource="http://humanbehaviourchange.org/ontology/BCIO_011010"/>
        <obo:IAO_0000114>Published</obo:IAO_0000114>
        <obo:IAO_0000115>Electronic mode of delivery that involves the intervention recipient being given access to an e-book.</obo:IAO_0000115>
        <rdfs:label>e-book mode of delivery</rdfs:label>
    </owl:Class>
    


    <!-- http://humanbehaviourchange.org/ontology/BCIO_011030 -->

    <owl:Class rdf:about="http://humanbehaviourchange.org/ontology/BCIO_011030">
        <rdfs:subClassOf rdf:resource="http://humanbehaviourchange.org/ontology/BCIO_011001"/>
        <obo:IAO_0000114>Published</obo:IAO_0000114>
        <obo:IAO_0000115>Informational mode of delivery that involves sound.</obo:IAO_0000115>
        <rdfs:label>audio informational mode of delivery</rdfs:label>
    </owl:Class>
    


    <!-- http://humanbehaviourchange.org/ontology/BCIO_011031 -->

    <owl:Class rdf:about="http://humanbehaviourchange.org/ontology/BCIO_011031">
        <rdfs:subClassOf rdf:resource="http://humanbehaviourchange.org/ontology/BCIO_011001"/>
        <obo:IAO_0000114>Published</obo:IAO_0000114>
        <obo:IAO_0000115>Informational mode of delivery that involves visual images.</obo:IAO_0000115>
        <rdfs:label>visual informational mode of delivery</rdfs:label>
    </owl:Class>
    


    <!-- http://humanbehaviourchange.org/ontology/BCIO_011032 -->

    <owl:Class rdf:about="http://humanbehaviourchange.org/ontology/BCIO_011032">
        <rdfs:subClassOf rdf:resource="http://humanbehaviourchange.org/ontology/BCIO_011001"/>
        <obo:IAO_0000114>Published</obo:IAO_0000114>
        <obo:IAO_0000115>Informational mode of delivery that involves written text.</obo:IAO_0000115>
        <rdfs:label>textual mode of delivery</rdfs:label>
    </owl:Class>
    


    <!-- http://humanbehaviourchange.org/ontology/BCIO_011033 -->

    <owl:Class rdf:about="http://humanbehaviourchange.org/ontology/BCIO_011033">
        <rdfs:subClassOf rdf:resource="http://humanbehaviourchange.org/ontology/BCIO_011000"/>
        <obo:IAO_0000114>Published</obo:IAO_0000114>
        <obo:IAO_0000115>Mode of delivery that involves changing the physical shape, size, structure or appearance of objects in the environment of the intervention recipient.</obo:IAO_0000115>
        <obo:IAO_0000232>This is a very heterogeneous class that will need to be further subdivided.</obo:IAO_0000232>
        <rdfs:comment>This does not include use of textual or pictorial information. It includes lighting, speed humps, use of music, shape and size of containers of consumables.</rdfs:comment>
        <rdfs:label>environmental change mode of delivery</rdfs:label>
    </owl:Class>
    


    <!-- http://humanbehaviourchange.org/ontology/BCIO_011034 -->

    <owl:Class rdf:about="http://humanbehaviourchange.org/ontology/BCIO_011034">
        <rdfs:subClassOf rdf:resource="http://humanbehaviourchange.org/ontology/BCIO_011000"/>
        <obo:IAO_0000114>Published</obo:IAO_0000114>
        <obo:IAO_0000115>Mode of delivery that involves devices or substances that alter bodily processes or structure.</obo:IAO_0000115>
        <obo:IAO_0000232>Is intended to be disjoint from informational mode of delivery.</obo:IAO_0000232>
        <rdfs:label>somatic mode of delivery</rdfs:label>
    </owl:Class>
    


    <!-- http://humanbehaviourchange.org/ontology/BCIO_011035 -->

    <owl:Class rdf:about="http://humanbehaviourchange.org/ontology/BCIO_011035">
        <rdfs:subClassOf rdf:resource="http://humanbehaviourchange.org/ontology/BCIO_011034"/>
        <obo:IAO_0000114>Published</obo:IAO_0000114>
        <obo:IAO_0000115>Somatic mode of delivery that involves ingestion of a chemical into the body.</obo:IAO_0000115>
        <rdfs:label>ingestion mode of delivery</rdfs:label>
    </owl:Class>
    


    <!-- http://humanbehaviourchange.org/ontology/BCIO_011036 -->

    <owl:Class rdf:about="http://humanbehaviourchange.org/ontology/BCIO_011036">
        <rdfs:subClassOf rdf:resource="http://humanbehaviourchange.org/ontology/BCIO_011035"/>
        <obo:IAO_0000114>Published</obo:IAO_0000114>
        <obo:IAO_0000115>Ingestion mode of delivery that involves ingestion of a chemical through the skin.</obo:IAO_0000115>
        <rdfs:label>transdermal mode of delivery</rdfs:label>
    </owl:Class>
    


    <!-- http://humanbehaviourchange.org/ontology/BCIO_011037 -->

    <owl:Class rdf:about="http://humanbehaviourchange.org/ontology/BCIO_011037">
        <rdfs:subClassOf rdf:resource="http://humanbehaviourchange.org/ontology/BCIO_011035"/>
        <obo:IAO_0000114>Published</obo:IAO_0000114>
        <obo:IAO_0000115>Somatic mode of delivery that involves ingestion of a chemical through the stomach or intestine.</obo:IAO_0000115>
        <rdfs:label>alimentary mode of delivery</rdfs:label>
    </owl:Class>
    


    <!-- http://humanbehaviourchange.org/ontology/BCIO_011038 -->

    <owl:Class rdf:about="http://humanbehaviourchange.org/ontology/BCIO_011038">
        <rdfs:subClassOf rdf:resource="http://humanbehaviourchange.org/ontology/BCIO_011037"/>
        <obo:IAO_0000114>Published</obo:IAO_0000114>
        <obo:IAO_0000115>Alimentary mode of delivery that involves swallowing of a pill or oral capsule.</obo:IAO_0000115>
        <rdfs:label>pill mode of delivery</rdfs:label>
    </owl:Class>
    


    <!-- http://humanbehaviourchange.org/ontology/BCIO_011039 -->

    <owl:Class rdf:about="http://humanbehaviourchange.org/ontology/BCIO_011039">
        <rdfs:subClassOf rdf:resource="http://humanbehaviourchange.org/ontology/BCIO_011037"/>
        <obo:IAO_0000114>Published</obo:IAO_0000114>
        <obo:IAO_0000115>Alimentary mode of delivery that involves swallowing of a liquid.</obo:IAO_0000115>
        <rdfs:label>ingestable liquid mode of delivery</rdfs:label>
    </owl:Class>
    


    <!-- http://humanbehaviourchange.org/ontology/BCIO_011040 -->

    <owl:Class rdf:about="http://humanbehaviourchange.org/ontology/BCIO_011040">
        <rdfs:subClassOf rdf:resource="http://humanbehaviourchange.org/ontology/BCIO_011035"/>
        <obo:IAO_0000114>Published</obo:IAO_0000114>
        <obo:IAO_0000115>Ingestion mode of delivery that involves absorption of a chemical through the lining of the buccal cavity.</obo:IAO_0000115>
        <rdfs:label>buccal mode of delivery</rdfs:label>
    </owl:Class>
    


    <!-- http://humanbehaviourchange.org/ontology/BCIO_011041 -->

    <owl:Class rdf:about="http://humanbehaviourchange.org/ontology/BCIO_011041">
        <rdfs:subClassOf rdf:resource="http://humanbehaviourchange.org/ontology/BCIO_011035"/>
        <obo:IAO_0000114>Published</obo:IAO_0000114>
        <obo:IAO_0000115>Ingestion mode of delivery that involves absorption of a chemical through  the upper airways or lungs by inspiration.</obo:IAO_0000115>
        <rdfs:label>inhalation mode of delivery</rdfs:label>
    </owl:Class>
    


    <!-- http://humanbehaviourchange.org/ontology/BCIO_011042 -->

    <owl:Class rdf:about="http://humanbehaviourchange.org/ontology/BCIO_011042">
        <rdfs:subClassOf rdf:resource="http://humanbehaviourchange.org/ontology/BCIO_011035"/>
        <obo:IAO_0000114>Published</obo:IAO_0000114>
        <obo:IAO_0000115>Ingestion mode of delivery that involves a chemical being introduced into body tissue through a hollow needle that punctures the skin.</obo:IAO_0000115>
        <rdfs:label>injection mode of delivery</rdfs:label>
    </owl:Class>
    


    <!-- http://humanbehaviourchange.org/ontology/BCIO_011043 -->

    <owl:Class rdf:about="http://humanbehaviourchange.org/ontology/BCIO_011043">
        <rdfs:subClassOf rdf:resource="http://humanbehaviourchange.org/ontology/BCIO_011042"/>
        <obo:IAO_0000114>Published</obo:IAO_0000114>
        <obo:IAO_0000115>Injection mode of delivery in which the tissue receiving the chemical is subcutaneous tissue.</obo:IAO_0000115>
        <rdfs:label>subcutaneous injection mode of delivery</rdfs:label>
    </owl:Class>
    


    <!-- http://humanbehaviourchange.org/ontology/BCIO_011044 -->

    <owl:Class rdf:about="http://humanbehaviourchange.org/ontology/BCIO_011044">
        <rdfs:subClassOf rdf:resource="http://humanbehaviourchange.org/ontology/BCIO_011042"/>
        <obo:IAO_0000114>Published</obo:IAO_0000114>
        <obo:IAO_0000115>Injection mode of delivery in which the tissue receiving the chemical is venous blood.</obo:IAO_0000115>
        <rdfs:label>intravenous injection mode of delivery</rdfs:label>
    </owl:Class>
    


    <!-- http://humanbehaviourchange.org/ontology/BCIO_011045 -->

    <owl:Class rdf:about="http://humanbehaviourchange.org/ontology/BCIO_011045">
        <rdfs:subClassOf rdf:resource="http://humanbehaviourchange.org/ontology/BCIO_011042"/>
        <obo:IAO_0000114>Published</obo:IAO_0000114>
        <obo:IAO_0000115>Injection mode of delivery in which the tissue receiving the chemical is muscle.</obo:IAO_0000115>
        <rdfs:label>intramuscular injection mode of delivery</rdfs:label>
    </owl:Class>
    


    <!-- http://humanbehaviourchange.org/ontology/BCIO_011046 -->

    <owl:Class rdf:about="http://humanbehaviourchange.org/ontology/BCIO_011046">
        <rdfs:subClassOf rdf:resource="http://humanbehaviourchange.org/ontology/BCIO_011035"/>
        <obo:IAO_0000114>Published</obo:IAO_0000114>
        <obo:IAO_0000115>Ingestion mode of delivery that involves a device that is worn on the body.</obo:IAO_0000115>
        <rdfs:comment>Includes insulin pump.</rdfs:comment>
        <rdfs:label>wearable ingestion mode of delivery</rdfs:label>
    </owl:Class>
    


    <!-- http://humanbehaviourchange.org/ontology/BCIO_011047 -->

    <owl:Class rdf:about="http://humanbehaviourchange.org/ontology/BCIO_011047">
        <rdfs:subClassOf rdf:resource="http://humanbehaviourchange.org/ontology/BCIO_011034"/>
        <obo:IAO_0000114>Published</obo:IAO_0000114>
        <obo:IAO_0000115>Ingestion mode of delivery that involves chewing of a soft material.</obo:IAO_0000115>
        <rdfs:comment>This includes chewing gum. often involves ingestion of a chemical that is released by chewing and absorbed through the lining of the buccal cavity, but this is not necessary.</rdfs:comment>
        <rdfs:label>chewable substance mode of delivery</rdfs:label>
    </owl:Class>
    


    <!-- http://humanbehaviourchange.org/ontology/BCIO_011048 -->

    <owl:Class rdf:about="http://humanbehaviourchange.org/ontology/BCIO_011048">
        <rdfs:subClassOf rdf:resource="http://humanbehaviourchange.org/ontology/BCIO_011034"/>
        <obo:IAO_0000114>Published</obo:IAO_0000114>
        <obo:IAO_0000115>A mode of delivery that involves application of a physical stimulus to the body.</obo:IAO_0000115>
        <rdfs:label>physical stimulus mode of delivery</rdfs:label>
    </owl:Class>
    


    <!-- http://humanbehaviourchange.org/ontology/BCIO_011049 -->

    <owl:Class rdf:about="http://humanbehaviourchange.org/ontology/BCIO_011049">
        <rdfs:subClassOf rdf:resource="http://humanbehaviourchange.org/ontology/BCIO_011048"/>
        <obo:IAO_0000114>Published</obo:IAO_0000114>
        <obo:IAO_0000115>Physical stimulus mode of delivery that involves exposure of light to the body</obo:IAO_0000115>
        <obo:IAO_0000118>Includes photo therapy</obo:IAO_0000118>
        <rdfs:label>light exposure mode of delivery</rdfs:label>
    </owl:Class>
    


    <!-- http://humanbehaviourchange.org/ontology/BCIO_011050 -->

    <owl:Class rdf:about="http://humanbehaviourchange.org/ontology/BCIO_011050">
        <rdfs:subClassOf rdf:resource="http://humanbehaviourchange.org/ontology/BCIO_011048"/>
        <obo:IAO_0000114>Published</obo:IAO_0000114>
        <obo:IAO_0000115>Physical stimulius mode of delivery that involves application of heat or cold to the body.</obo:IAO_0000115>
        <rdfs:label>temperature mode of delivery</rdfs:label>
    </owl:Class>
    


    <!-- http://humanbehaviourchange.org/ontology/BCIO_011051 -->

    <owl:Class rdf:about="http://humanbehaviourchange.org/ontology/BCIO_011051">
        <rdfs:subClassOf rdf:resource="http://humanbehaviourchange.org/ontology/BCIO_011048"/>
        <obo:IAO_0000114>Published</obo:IAO_0000114>
        <obo:IAO_0000115>Physical stimulus mode of delivery that involves application of electrical stimulation to the body.</obo:IAO_0000115>
        <rdfs:label>electrical stimulation mode of delivery</rdfs:label>
    </owl:Class>
    


    <!-- http://humanbehaviourchange.org/ontology/BCIO_011052 -->

    <owl:Class rdf:about="http://humanbehaviourchange.org/ontology/BCIO_011052">
        <rdfs:subClassOf rdf:resource="http://humanbehaviourchange.org/ontology/BCIO_011048"/>
        <obo:IAO_0000114>Published</obo:IAO_0000114>
        <obo:IAO_0000115>Physical stimulus mode of delivery that involves application of physical pressure to the outside of the body.</obo:IAO_0000115>
        <rdfs:comment>Includes massage.</rdfs:comment>
        <rdfs:label>physical pressure mode of delivery</rdfs:label>
    </owl:Class>
    


    <!-- http://humanbehaviourchange.org/ontology/BCIO_011053 -->

    <owl:Class rdf:about="http://humanbehaviourchange.org/ontology/BCIO_011053">
        <rdfs:subClassOf rdf:resource="http://humanbehaviourchange.org/ontology/BCIO_011048"/>
        <obo:IAO_0000114>Published</obo:IAO_0000114>
        <obo:IAO_0000115>Physical stimulus mode of delivery that involves a device that is worn on the body.</obo:IAO_0000115>
        <rdfs:label>wearable stimulus mode of delivery</rdfs:label>
    </owl:Class>
    


    <!-- http://humanbehaviourchange.org/ontology/BCIO_011054 -->

    <owl:Class rdf:about="http://humanbehaviourchange.org/ontology/BCIO_011054">
        <rdfs:subClassOf rdf:resource="http://humanbehaviourchange.org/ontology/BCIO_011000"/>
        <obo:IAO_0000114>Published</obo:IAO_0000114>
        <obo:IAO_0000115>Mode of of delivery that involves modifying the structure of the body of the recipient of the intervention.</obo:IAO_0000115>
        <rdfs:comment>Includes surgery.</rdfs:comment>
        <rdfs:label>somatic alteration mode of delivery</rdfs:label>
    </owl:Class>
    


    <!-- http://humanbehaviourchange.org/ontology/BCIO_011055 -->

    <owl:Class rdf:about="http://humanbehaviourchange.org/ontology/BCIO_011055">
        <rdfs:subClassOf rdf:resource="http://humanbehaviourchange.org/ontology/BCIO_011000"/>
        <obo:IAO_0000114>Published</obo:IAO_0000114>
        <obo:IAO_0000115>Mode of delivery that involves one recipient in the location where the intervention is delivered.</obo:IAO_0000115>
        <rdfs:label>individual-based mode of delivery</rdfs:label>
    </owl:Class>
    


    <!-- http://humanbehaviourchange.org/ontology/BCIO_011056 -->

    <owl:Class rdf:about="http://humanbehaviourchange.org/ontology/BCIO_011056">
        <rdfs:subClassOf rdf:resource="http://humanbehaviourchange.org/ontology/BCIO_011000"/>
        <obo:IAO_0000114>Published</obo:IAO_0000114>
        <obo:IAO_0000115>Mode of delivery that involves two recipients in the location where the intervention is delivered who have an interpersonal relationship.</obo:IAO_0000115>
        <rdfs:label>pair-based mode of delivery</rdfs:label>
    </owl:Class>
    


    <!-- http://humanbehaviourchange.org/ontology/BCIO_011057 -->

    <owl:Class rdf:about="http://humanbehaviourchange.org/ontology/BCIO_011057">
        <rdfs:subClassOf rdf:resource="http://humanbehaviourchange.org/ontology/BCIO_011000"/>
        <obo:IAO_0000114>Published</obo:IAO_0000114>
        <obo:IAO_0000115>Mode of delivery that involves three or more people in the location where the intervention is delivered.</obo:IAO_0000115>
        <rdfs:label>group-based mode of delivery</rdfs:label>
    </owl:Class>
    


    <!-- http://humanbehaviourchange.org/ontology/BCIO_011058 -->

    <owl:Class rdf:about="http://humanbehaviourchange.org/ontology/BCIO_011058">
        <rdfs:subClassOf rdf:resource="http://humanbehaviourchange.org/ontology/BCIO_011000"/>
        <obo:IAO_0000114>Published</obo:IAO_0000114>
        <obo:IAO_0000115>Mode of delivery in which the only causal influence is from the intervention source to the recipient.</obo:IAO_0000115>
        <rdfs:label>uni-directional mode of delivery</rdfs:label>
    </owl:Class>
    


    <!-- http://humanbehaviourchange.org/ontology/BCIO_011059 -->

    <owl:Class rdf:about="http://humanbehaviourchange.org/ontology/BCIO_011059">
        <rdfs:subClassOf rdf:resource="http://humanbehaviourchange.org/ontology/BCIO_011000"/>
        <obo:IAO_0000114>Published</obo:IAO_0000114>
        <obo:IAO_0000115>Mode of delivery in which there is causal influence from the intervention source to the recipient and from the recipient to the source.</obo:IAO_0000115>
        <rdfs:label>interactional mode of delivery</rdfs:label>
    </owl:Class>
    


    <!-- http://humanbehaviourchange.org/ontology/BCIO_011060 -->

    <owl:Class rdf:about="http://humanbehaviourchange.org/ontology/BCIO_011060">
        <rdfs:subClassOf rdf:resource="http://humanbehaviourchange.org/ontology/BCIO_011000"/>
        <obo:IAO_0000114>Published</obo:IAO_0000114>
        <obo:IAO_0000115>Mode of delivery that involves delivery and receipt of the intervention or its components occurring at the same time or very close in time.</obo:IAO_0000115>
        <rdfs:label>synchronous mode of delivery</rdfs:label>
    </owl:Class>
    


    <!-- http://humanbehaviourchange.org/ontology/BCIO_011061 -->

    <owl:Class rdf:about="http://humanbehaviourchange.org/ontology/BCIO_011061">
        <rdfs:subClassOf rdf:resource="http://humanbehaviourchange.org/ontology/BCIO_011000"/>
        <obo:IAO_0000114>Published</obo:IAO_0000114>
        <obo:IAO_0000115>Mode of delivery that involves receipt of the intervention or its components taking place a significant period of time after delivery.</obo:IAO_0000115>
        <rdfs:label>asynchronous mode of delivery</rdfs:label>
    </owl:Class>
    


    <!-- http://humanbehaviourchange.org/ontology/BCIO_011062 -->

    <owl:Class rdf:about="http://humanbehaviourchange.org/ontology/BCIO_011062">
        <rdfs:subClassOf rdf:resource="http://humanbehaviourchange.org/ontology/BCIO_011000"/>
        <obo:IAO_0000114>Published</obo:IAO_0000114>
        <obo:IAO_0000115>Mode of delivery that is not dependent on actions on the part of the intervention recipient.</obo:IAO_0000115>
        <rdfs:label>push mode of delivery</rdfs:label>
    </owl:Class>
    


    <!-- http://humanbehaviourchange.org/ontology/BCIO_011063 -->

    <owl:Class rdf:about="http://humanbehaviourchange.org/ontology/BCIO_011063">
        <rdfs:subClassOf rdf:resource="http://humanbehaviourchange.org/ontology/BCIO_011000"/>
        <obo:IAO_0000114>Published</obo:IAO_0000114>
        <obo:IAO_0000115>Mode of delivery that requires some action on the part of the recipient.</obo:IAO_0000115>
        <rdfs:label>pull mode of delivery</rdfs:label>
    </owl:Class>
    


    <!-- http://humanbehaviourchange.org/ontology/BCIO_011064 -->

    <owl:Class rdf:about="http://humanbehaviourchange.org/ontology/BCIO_011064">
        <rdfs:subClassOf rdf:resource="http://humanbehaviourchange.org/ontology/BCIO_011000"/>
        <obo:IAO_0000114>Published</obo:IAO_0000114>
        <obo:IAO_0000115>Mode of delivery that involves application of typical elements of game playing  to other areas of activity, typically as an online marketing technique to encourage engagement with a product or service.</obo:IAO_0000115>
        <obo:IAO_0000119>https://www.lexico.com/en/definition/gamification</obo:IAO_0000119>
        <rdfs:comment>Includes point scoring, competition with others, and rules of play.</rdfs:comment>
        <rdfs:label>gamification mode of delivery</rdfs:label>
    </owl:Class>
    


    <!-- http://humanbehaviourchange.org/ontology/BCIO_011065 -->

    <owl:Class rdf:about="http://humanbehaviourchange.org/ontology/BCIO_011065">
        <rdfs:subClassOf rdf:resource="http://humanbehaviourchange.org/ontology/BCIO_011000"/>
        <obo:IAO_0000114>Published</obo:IAO_0000114>
        <obo:IAO_0000115>Mode of delivery that involves application of creativity on the part of the intervention recipient.</obo:IAO_0000115>
        <rdfs:comment>Includes art therapy, music therapy, dance and acting.</rdfs:comment>
        <rdfs:label>arts feature mode of delivery</rdfs:label>
    </owl:Class>
    


    <!-- http://humanbehaviourchange.org/ontology/BCIO_043000 -->

    <owl:Class rdf:about="http://humanbehaviourchange.org/ontology/BCIO_043000"/>
</rdf:RDF>



<!-- Generated by the OWL API (version 4.5.26) https://github.com/owlcs/owlapi -->

